Merge branch 'universal' into dd/dev/abpcomp_func_ex
# Conflicts:
#	CaseStudies/ABP/ABP_TSPS.thy

CaseStudies/ABP/ABP_TSPS.thy
@@ -10,7 +10,7 @@ theory ABP_TSPS
 
 begin
 
-  default_sort countable
+default_sort countable
 
 
 (* ----------------------------------------------------------------------- *)
@@ -19,13 +19,13 @@ section \<open>Datatype Definition\<close>
 
 
 datatype 'a::countable MABP = BoolPair "('a * bool)" | Bool bool | Data 'a
+print_theorems
 
 instantiation MABP ::  (countable) countable
 begin
 instance
    by (countable_datatype)
 end
-
 
 instantiation MABP ::  (countable) message
 begin
@@ -42,17 +42,6 @@ fun ctype_MABP :: "channel \<Rightarrow> 'a MABP set" where
   instance ..
 end
 
-(*
-instantiation MABP ::  (countable) message
-begin
-function ctype_MABP :: "channel \<Rightarrow> 'a MABP set" where
-  "ctype_MABP (\<C> ''abpIn'') = range Data" |
-  "ctype_MABP (\<C> ''abpOut'') = range Data" |
-  "other \<noteq> (\<C> ''abpOut'') \<Longrightarrow> other \<noteq> (\<C> ''abpIn'') \<Longrightarrow> ctype_MABP other = undefined"
-        apply simp_all
-  sorry 
-  instance ..
-end*)
 
 declare [[show_types]]
 declare [[show_sorts]]
@@ -77,9 +66,11 @@ abbreviation invData :: "'a MABP \<Rightarrow> 'a" where
 
 
 (* ----------------------------------------------------------------------- *)
-section \<open>Helper Definitions\<close>
+section \<open>Component Helper Definitions\<close>
 (* ----------------------------------------------------------------------- *)
 
+
+subsection \<open>receiver\<close>
 
 
 abbreviation recvAbb where
@@ -88,39 +79,39 @@ let recRes = (\<lambda> x. tsRec\<cdot>((tsMap invBoolPair)\<cdot>(x . c_dr)))
 in (\<lambda> x. (ubclDom\<cdot>x = {c_dr}) \<leadsto> Abs_ubundle([c_ar    \<mapsto> tsMap Bool\<cdot>(fst (recRes x)),
                                         c_abpOut \<mapsto> tsMap Data\<cdot>(snd (recRes x))]))"
 
-
-subsection \<open>receiver\<close>
 definition recvTSPF :: "('a MABP tstream\<^sup>\<Omega>) ufun" where
 "recvTSPF \<equiv> Abs_cufun (\<lambda> x. (ubclDom\<cdot>x = {c_dr}) \<leadsto> Abs_ubundle([c_ar    \<mapsto> (tsMap::(bool \<Rightarrow> 'a MABP) \<Rightarrow> bool tstream \<rightarrow> 'a MABP tstream) Bool\<cdot>(fst ( tsRec\<cdot>((tsMap invBoolPair)\<cdot>(x . c_dr)))),
                                         c_abpOut \<mapsto> (tsMap::('a \<Rightarrow> 'a MABP) \<Rightarrow> 'a tstream \<rightarrow> 'a MABP tstream) Data\<cdot>(snd ( tsRec\<cdot>((tsMap invBoolPair)\<cdot>(x . c_dr))))]))"
 
-subsection \<open>medium_rs\<close>
-  (* medium from receiver to sender *)
-  (* input: c_ar, output: c_as, transport booleans *)
 
-definition medRS_TSPF :: "bool stream \<Rightarrow> ('a MABP tstream\<^sup>\<Omega>) ufun" where
-"medRS_TSPF bst\<equiv> Abs_cufun (\<lambda> x. (ubclDom\<cdot>x = {c_ar})
-                           \<leadsto> Abs_ubundle([c_as \<mapsto> (tsMap::(bool \<Rightarrow> 'a MABP) \<Rightarrow> bool tstream \<rightarrow> 'a MABP tstream) Bool\<cdot>(tsMed\<cdot>(tsMap invBool\<cdot>(x . c_ar))\<cdot>bst)]))"
+subsection \<open>medium\<close>
 
-abbreviation tsMedRSAbb  :: "bool stream \<Rightarrow> 'a MABP tstream\<^sup>\<Omega> \<Rightarrow> ('a MABP tstream\<^sup>\<Omega>) option" where
-"tsMedRSAbb bst x \<equiv> ((ubclDom\<cdot>x = {c_ar})
-                            \<leadsto> Abs_ubundle([c_as \<mapsto> (tsMap::(bool \<Rightarrow> 'a MABP) \<Rightarrow> bool tstream \<rightarrow> 'a MABP tstream) Bool\<cdot>(tsMed\<cdot>(tsMap invBool\<cdot>(x . c_ar))\<cdot>bst)]))"
+
+definition med_TSPF :: "bool stream \<Rightarrow> channel \<Rightarrow> channel \<Rightarrow> ('b \<Rightarrow> 'a MABP) \<Rightarrow> ('a MABP tstream\<^sup>\<Omega>)ufun" where
+"med_TSPF bst In Out f \<equiv> Abs_cufun (\<lambda> x. (ubDom\<cdot>x = {In})
+                           \<leadsto> Abs_ubundle([Out \<mapsto> tsMap f\<cdot>(tsMed\<cdot>(tsMap (inv f)\<cdot>(x . In))\<cdot>bst)]))"
+
+abbreviation tsMedAbb  :: "bool stream \<Rightarrow> channel \<Rightarrow> channel \<Rightarrow> ('b \<Rightarrow> 'a MABP) \<Rightarrow> 'a MABP tstream\<^sup>\<Omega> \<Rightarrow> ('a MABP tstream\<^sup>\<Omega>) option" where
+"tsMedAbb bst In Out f x \<equiv> ((ubDom\<cdot>x = {In})
+                           \<leadsto> Abs_ubundle([Out \<mapsto> tsMap f\<cdot>(tsMed\<cdot>(tsMap (inv f)\<cdot>(x . In))\<cdot>bst)]))"
+
 
 subsection \<open>medium_sr\<close>
   (* medium from sender to receiver *)
   (* input: c_ds, output: c_dr, transport (data, bool) tuples *)
+abbreviation medSR_TSPF :: "bool stream \<Rightarrow>('a MABP tstream\<^sup>\<Omega>)ufun" where
+"medSR_TSPF bst\<equiv> med_TSPF bst c_ds c_dr BoolPair"
 
-definition medSR_TSPF :: "bool stream \<Rightarrow> ('a MABP tstream\<^sup>\<Omega>) ufun" where
-"medSR_TSPF bst\<equiv> Abs_cufun (\<lambda> x. (ubclDom\<cdot>x = {c_ds})
-  \<leadsto> Abs_ubundle([c_dr \<mapsto> (tsMap:: ('a \<times> bool \<Rightarrow> 'a MABP) \<Rightarrow> ('a \<times> bool) tstream \<rightarrow> 'a MABP tstream) 
-            BoolPair\<cdot>(tsMed\<cdot>(tsMap invBoolPair\<cdot>(x . c_ds))\<cdot>bst)]))"
 
-abbreviation medSR_TSPFAbb  :: "bool stream \<Rightarrow> 'a MABP tstream\<^sup>\<Omega> \<Rightarrow> ('a MABP tstream\<^sup>\<Omega>) option" where
-"medSR_TSPFAbb bst x \<equiv> ((ubclDom\<cdot>x = {c_ds})
-  \<leadsto> Abs_ubundle([c_dr \<mapsto> (tsMap:: ('a \<times> bool \<Rightarrow> 'a MABP) \<Rightarrow> ('a \<times> bool) tstream \<rightarrow> 'a MABP tstream) 
-            BoolPair\<cdot>(tsMed\<cdot>(tsMap invBoolPair\<cdot>(x . c_ds))\<cdot>bst)]))"
+subsection \<open>medium_rs\<close>
+  (* medium from receiver to sender *)
+  (* input: c_ar, output: c_as, transport booleans *)
+abbreviation medRS_TSPF :: "bool stream \<Rightarrow>('a MABP tstream\<^sup>\<Omega>)ufun" where
+"medRS_TSPF bst\<equiv> med_TSPF bst c_ar c_as Bool"
+
 
 subsection \<open>sender\<close>
+
 
   (* lift a sender function to a TSPF *)
 definition senderTSPF :: "'a sender \<Rightarrow> ('a MABP tstream\<^sup>\<Omega>) ufun" where
@@ -128,237 +119,23 @@ definition senderTSPF :: "'a sender \<Rightarrow> ('a MABP tstream\<^sup>\<Omega
                 \<leadsto> Abs_ubundle([c_ds \<mapsto> tsMap BoolPair\<cdot>(se\<cdot>(tsMap invData\<cdot>(x . c_abpIn))\<cdot>(tsMap invBool\<cdot>(x . c_as)))]))"
 
 
-
 subsection \<open>id\<close>
 
 
-definition id_TSPF :: "('a MABP tstream\<^sup>\<Omega>) ufun" where
-"id_TSPF \<equiv> Abs_cufun (\<lambda> x. (ubDom\<cdot>x = {c_abpOut}) \<leadsto> Abs_ubundle [c_idOut \<mapsto> x . c_abpOut])"
+definition idTSPF :: "('a MABP tstream\<^sup>\<Omega>) ufun" where
+"idTSPF \<equiv> Abs_cufun (\<lambda> x. (ubDom\<cdot>x = {c_abpOut}) \<leadsto> x)"
 
-
-
-(* ----------------------------------------------------------------------- *)
-section \<open>Components\<close>
-(* ----------------------------------------------------------------------- *)
-
-
-lift_definition SND :: "(('a MABP tstream\<^sup>\<Omega>) ufun) uspec" is
-"Rev {senderTSPF s | s. s \<in> tsSender}"
-  sorry
-
-lift_definition RCV :: "(('a MABP tstream\<^sup>\<Omega>) ufun) uspec" is
-"Rev {recvTSPF}"
-  sorry
-
-lift_definition MEDSR :: "(('a MABP tstream\<^sup>\<Omega>) ufun) uspec" is
-"Rev {medSR_TSPF ora | ora. #({True} \<ominus> ora)=\<infinity>}"
-  sorry
-
-lift_definition MEDRS :: "(('a MABP tstream\<^sup>\<Omega>) ufun) uspec" is
-"Rev {medRS_TSPF ora | ora. #({True} \<ominus> ora)=\<infinity>}"
-  sorry
-
-lift_definition ID :: "(('a MABP tstream\<^sup>\<Omega>) ufun) uspec" is
-"Rev {id_TSPF}"
-  sorry    
-
-abbreviation gencompABP :: "(('a MABP tstream\<^sup>\<Omega>) ufun) uspec" where
-"gencompABP \<equiv> ((SND \<Otimes> MEDSR) \<Otimes> RCV) \<Otimes> MEDRS"
-
-abbreviation speccompABP :: "(('a MABP tstream\<^sup>\<Omega>) ufun) uspec" where
-"speccompABP \<equiv> uspecFeedbackComp(((SND \<circle> MEDSR) \<circle> RCV) \<circle> (MEDRS \<parallel> ID))"
-
-
-(* ----------------------------------------------------------------------- *)
-section \<open>Testing of Composition without Medium\<close>
-(* ----------------------------------------------------------------------- *)
-
-
-definition senderTSPF2 :: "'a sender \<Rightarrow> ('a MABP tstream\<^sup>\<Omega>) ufun" where
-"senderTSPF2 se \<equiv> Abs_cufun (\<lambda> x. (ubDom\<cdot>x = {c_ar, c_abpIn})
-                \<leadsto> Abs_ubundle [c_dr \<mapsto> tsMap BoolPair\<cdot>(se\<cdot>(tsMap invData\<cdot>(x . c_abpIn))\<cdot>(tsMap invBool\<cdot>(x . c_ar)))])"
-
-lemma sender_mono: assumes "se \<in> tsSender" shows "monofun (\<lambda> x. (ubDom\<cdot>x = {c_ar, c_abpIn})
-                \<leadsto> Abs_ubundle [c_dr \<mapsto> tsMap BoolPair\<cdot>(se\<cdot>(tsMap invData\<cdot>(x . c_abpIn))\<cdot>(tsMap invBool\<cdot>(x . c_ar)))])"
-  sorry
-
-lemma sender_cont: assumes "se \<in> tsSender" shows "cont (\<lambda> x. (ubDom\<cdot>x = {c_ar, c_abpIn})
-                \<leadsto> Abs_ubundle [c_dr \<mapsto> tsMap BoolPair\<cdot>(se\<cdot>(tsMap invData\<cdot>(x . c_abpIn))\<cdot>(tsMap invBool\<cdot>(x . c_ar)))])"
-  sorry
-
-lemma sender_well: assumes "se \<in> tsSender" shows "ufWell (\<Lambda> x. (ubDom\<cdot>x = {c_ar, c_abpIn})
-                \<leadsto> Abs_ubundle [c_dr \<mapsto> tsMap BoolPair\<cdot>(se\<cdot>(tsMap invData\<cdot>(x . c_abpIn))\<cdot>(tsMap invBool\<cdot>(x . c_ar)))])"
-  sorry
-
-lift_definition SND2 :: "(('a MABP tstream\<^sup>\<Omega>) ufun) uspec" is
-"Rev {senderTSPF2 s | s. s \<in> tsSender}"
-  sorry
-
-definition recvTSPF2 :: "('a MABP tstream\<^sup>\<Omega>) ufun" where
-"recvTSPF2 \<equiv> Abs_cufun (\<lambda> x. (ubDom\<cdot>x = {c_dr}) \<leadsto> Abs_ubundle [c_ar    \<mapsto> (tsMap::(bool \<Rightarrow> 'a MABP) \<Rightarrow> bool tstream \<rightarrow> 'a MABP tstream) Bool\<cdot>(fst ( tsRec\<cdot>((tsMap invBoolPair)\<cdot>(x . c_dr)))),
-                                        c_abpOut \<mapsto> (tsMap::('a \<Rightarrow> 'a MABP) \<Rightarrow> 'a tstream \<rightarrow> 'a MABP tstream) Data\<cdot>(snd ( tsRec\<cdot>((tsMap invBoolPair)\<cdot>(x . c_dr))))])"
-
-lemma recv_mono: "monofun (\<lambda> x. (ubDom\<cdot>x = {c_dr}) \<leadsto> Abs_ubundle [c_ar    \<mapsto> (tsMap::(bool \<Rightarrow> 'a MABP) \<Rightarrow> bool tstream \<rightarrow> 'a MABP tstream) Bool\<cdot>(fst ( tsRec\<cdot>((tsMap invBoolPair)\<cdot>(x . c_dr)))),
-                                        c_abpOut \<mapsto> (tsMap::('a \<Rightarrow> 'a MABP) \<Rightarrow> 'a tstream \<rightarrow> 'a MABP tstream) Data\<cdot>(snd ( tsRec\<cdot>((tsMap invBoolPair)\<cdot>(x . c_dr))))])"
-  sorry
-
-lemma recv_cont: "cont (\<lambda> x. (ubDom\<cdot>x = {c_dr}) \<leadsto> Abs_ubundle [c_ar    \<mapsto> (tsMap::(bool \<Rightarrow> 'a MABP) \<Rightarrow> bool tstream \<rightarrow> 'a MABP tstream) Bool\<cdot>(fst ( tsRec\<cdot>((tsMap invBoolPair)\<cdot>(x . c_dr)))),
-                                        c_abpOut \<mapsto> (tsMap::('a \<Rightarrow> 'a MABP) \<Rightarrow> 'a tstream \<rightarrow> 'a MABP tstream) Data\<cdot>(snd ( tsRec\<cdot>((tsMap invBoolPair)\<cdot>(x . c_dr))))])"
-  sorry
-
-lemma recv_well: "ufWell (\<Lambda> x. (ubDom\<cdot>x = {c_dr}) \<leadsto> Abs_ubundle [c_ar    \<mapsto> (tsMap::(bool \<Rightarrow> 'a MABP) \<Rightarrow> bool tstream \<rightarrow> 'a MABP tstream) Bool\<cdot>(fst ( tsRec\<cdot>((tsMap invBoolPair)\<cdot>(x . c_dr)))),
-                                        c_abpOut \<mapsto> (tsMap::('a \<Rightarrow> 'a MABP) \<Rightarrow> 'a tstream \<rightarrow> 'a MABP tstream) Data\<cdot>(snd ( tsRec\<cdot>((tsMap invBoolPair)\<cdot>(x . c_dr))))])"
-  sorry
-
-lift_definition RCV2 :: "(('a MABP tstream\<^sup>\<Omega>) ufun) uspec" is
-"Rev {recvTSPF2}"
-  sorry
-
-abbreviation speccompABP_nmed :: "(('a MABP tstream\<^sup>\<Omega>) ufun) uspec" where
-"speccompABP_nmed \<equiv> uspecFeedbackComp(SND \<circle> RCV)"
-
-
-lemma tsaltbitpro_inp2out_nmed:
-  assumes send_def: "send \<in> tsSender"
-    and ds_def: "ds_stream = send\<cdot>i\<cdot>as_stream"
-    and as_def: "as_stream = tsProjSnd\<cdot>ds_stream"
-    and i_inf: "#\<surd>i = \<infinity>"
-  shows "tsAbs\<cdot>(tsRecSnd\<cdot>ds_stream) = tsAbs\<cdot>i"
-  using as_def ds_def send_def tsaltbitpro_inp2out_nmed by auto
-
-lemma h1: assumes "s \<in> tsSender" shows "UFun.ufDom\<cdot>(ufunclSerComp (senderTSPF2 s) recvTSPF2) = {c_abpIn, c_ar}"
-  apply (simp add: ufdom_insert ubclDom_ubundle_def)
-  sorry                                                              
-
-lemma h2: assumes "s \<in> tsSender" shows "UFun.ufRan\<cdot>(ufunclSerComp (senderTSPF2 s) recvTSPF2) = {c_abpOut, c_ar}"
-  sorry
-
-abbreviation abpFixH :: "('a tstream \<rightarrow> bool tstream \<rightarrow> ('a \<times> bool) tstream) \<Rightarrow>  'a MABP tstream ubundle \<Rightarrow> 'a MABP tstream ubundle \<rightarrow> 'a MABP tstream ubundle" where
-"abpFixH s tb \<equiv> (\<Lambda> x. Abs_ubundle[c_dr \<mapsto> tsMap BoolPair\<cdot>(s\<cdot>(tsMap invData\<cdot>(tb . c_abpIn))\<cdot>(tsMap invBool\<cdot>(x . c_ar))),
-                                    c_ar \<mapsto> (tsMap::(bool \<Rightarrow> 'a MABP) \<Rightarrow> bool tstream \<rightarrow> 'a MABP tstream) Bool\<cdot>(fst ( tsRec\<cdot>((tsMap invBoolPair)\<cdot>(x . c_dr)))),
-                                    c_abpOut \<mapsto> (tsMap::('a \<Rightarrow> 'a MABP) \<Rightarrow> 'a tstream \<rightarrow> 'a MABP tstream) Data\<cdot>(snd ( tsRec\<cdot>((tsMap invBoolPair)\<cdot>(x . c_dr))))
-                                   ])"
-
-lemma abp_speccomp: assumes "f \<in> Rep_rev_uspec speccompABP_nmed"
-                            and "ubDom\<cdot>tb = {c_abpIn}"
-                          shows "tsAbs\<cdot>((f \<rightleftharpoons> tb) . c_abpOut) = tsAbs\<cdot>(tb . c_abpIn)"
-proof - 
-  have f1: "\<exists> s \<in> tsSender. (f = (\<mu>(ufunclSerComp (senderTSPF2 s) recvTSPF2)))"
-    apply (simp add: ufunclSerComp_ufun_def)
-    (* Cannot be proven until Instatiation *)
-    sorry
-  then obtain s where f12: "s \<in> tsSender \<and> (f = (\<mu>(ufunclSerComp (senderTSPF2 s) recvTSPF2)))"
-    by blast
-  then have f13: "f = (\<mu>(ufunclSerComp (senderTSPF2 s) recvTSPF2))"
-    by blast
-  have f14: "s \<in> tsSender"
-    using f12 by blast
-
-
-  have f20: "ubclDom\<cdot>tb = {c_abpIn, c_ar} - {c_ar}"
-    apply(simp add: ubclDom_ubundle_def)
-    using assms by blast                    
-  have f2: "(f \<rightleftharpoons> tb) . c_abpOut =  ubFix (ufFeedH (ufunclSerComp (senderTSPF2 s) recvTSPF2) tb) {c_abpOut, c_ar}  .  c_abpOut"
-    apply(subst f13)
-    apply(simp add: ufFeedbackComp_def)
-    apply(simp add: ufFeedbackComp_cont ufFeedbackComp_well)
-    apply(simp add: f12 h1 h2)
-    by(simp add: f20)
-
-
-  have f3: "cont (\<lambda> x. Abs_ubundle[c_dr \<mapsto> tsMap BoolPair\<cdot>(s\<cdot>(tsMap invData\<cdot>(tb . c_abpIn))\<cdot>(tsMap invBool\<cdot>(x . c_ar))),
-                                    c_ar \<mapsto> (tsMap::(bool \<Rightarrow> 'a MABP) \<Rightarrow> bool tstream \<rightarrow> 'a MABP tstream) Bool\<cdot>(fst ( tsRec\<cdot>((tsMap invBoolPair)\<cdot>(x . c_dr)))),
-                                    c_abpOut \<mapsto> (tsMap::('a \<Rightarrow> 'a MABP) \<Rightarrow> 'a tstream \<rightarrow> 'a MABP tstream) Data\<cdot>(snd ( tsRec\<cdot>((tsMap invBoolPair)\<cdot>(x . c_dr))))
-                                   ])"
-    sorry
-  have f4: "ubFix (ufFeedH (ufunclSerComp (senderTSPF2 s) recvTSPF2) tb) {c_abpOut, c_ar}  .  c_abpOut
-          = ubFix (abpFixH s tb) {c_abpOut, c_ar, c_dr} . c_abpOut"
-    (* Should be possible to prove with equality of lubs *)
-    sorry
-  have f5: "ubfun_io_eq (abpFixH s tb) {c_abpOut, c_ar, c_dr}"
-    sorry
-  then have f6: "ubFix (abpFixH s tb) {c_abpOut, c_ar, c_dr} =  (abpFixH s tb)\<cdot>(ubFix (abpFixH s tb) {c_abpOut, c_ar, c_dr})"
-    using ubfix_eq by blast
-
-
-  (* After proving the fixed points propties we can now show the assumptions of the tsaltbitpro_inp2out_nmed lemma *)
-  (*
-    i = (tsMap invData\<cdot>(tb . c_abpIn))
-    ds_stream = (tsMap invBoolPair\<cdot>((ubFix (abpFixH s tb) {c_abpOut, c_ar, c_dr}) . c_dr))
-    as_stream = (tsMap invBool\<cdot>((ubFix (abpFixH s tb) {c_abpOut, c_ar, c_dr}) . c_ar))
-
-  *)
-  have f7: "(tsMap invBoolPair\<cdot>((ubFix (abpFixH s tb) {c_abpOut, c_ar, c_dr}) . c_dr)) = s\<cdot>(tsMap invData\<cdot>(tb . c_abpIn))\<cdot>(tsMap invBool\<cdot>((ubFix (abpFixH s tb) {c_abpOut, c_ar, c_dr}) . c_ar))"
-    sorry
-
-  have f8: "(tsMap invBool\<cdot>((ubFix (abpFixH s tb) {c_abpOut, c_ar, c_dr}) . c_ar)) = tsProjSnd\<cdot>(tsMap invBoolPair\<cdot>((ubFix (abpFixH s tb) {c_abpOut, c_ar, c_dr}) . c_dr))"
-    sorry
-
-  (* More assms are necessary for this subgoal*)
-  have f9: "#\<surd>(tsMap invData\<cdot>(tb . c_abpIn)) = \<infinity>"
-    sorry
-
-  (* Result of tsaltbitpro_inp2out_nmed lemma *)
-  have f10: "tsAbs\<cdot>(tsRecSnd\<cdot>(tsMap invBoolPair\<cdot>((ubFix (abpFixH s tb) {c_abpOut, c_ar, c_dr}) . c_dr))) = tsAbs\<cdot>(tsMap invData\<cdot>(tb . c_abpIn))"
-    using f7 f8 f9 f14 by(simp add: tsaltbitpro_inp2out_nmed)
-  
-  
-
-  
-  show ?thesis
-      sorry  
-qed
-
-
-
-
-
-
-(* ----------------------------------------------------------------------- *)
-section \<open>More Lemmas\<close>
-(* ----------------------------------------------------------------------- *)
-
-(*
-lemma tsaltbitpro_inp2out_nmed:
-  assumes send_def: "send \<in> tsSender"
-    and ds_def: "c_ds = send\<cdot>i\<cdot>c_as"
-    and as_def: "c_as = tsProjSnd\<cdot>c_ds"
-    and i_inf: "#\<surd>i = \<infinity>"
-  shows "tsAbs\<cdot>(tsRecSnd\<cdot>c_ds) = tsAbs\<cdot>i"
-  sorry    
-
-lemma tsaltbitpro_inp2out:
-  assumes send_def: "send \<in> tsSender"
-    and p1_def: "#({True} \<ominus> p1) = \<infinity>"
-    and p2_def: "#({True} \<ominus> p2) = \<infinity>"
-    and ds_def: "c_ds = send\<cdot>i\<cdot>c_as"
-    and dr_def: "c_dr = tsMed\<cdot>c_ds\<cdot>p1"
-    and ar_def: "c_ar = tsProjSnd\<cdot>c_dr"
-    (* definition 5 *)
-    and as_def: "c_as = tsMed\<cdot>c_ar\<cdot>p2"
-    and i_ninf: "#(tsAbs\<cdot>i) \<noteq> \<infinity>"
-  shows "tsAbs\<cdot>(tsProjFst\<cdot>(tsRemDups\<cdot>c_dr)) = tsAbs\<cdot>i"
-  sorry
-*)
-
-
-lemma abp_gencomp_final: assumes "f \<in> Rep_rev_uspec gencompABP"
-                            and "ubDom\<cdot>tb = {c_abpIn}"
-  shows "tsAbs\<cdot>((f \<rightleftharpoons> tb) . c_abpOut) = tsAbs\<cdot>(tb . c_abpIn)"
-  oops  
-
-lemma abp_speccomp_final: assumes "f \<in> Rep_rev_uspec speccompABP"
-                            and "ubDom\<cdot>tb = {c_abpIn}"
-  shows "tsAbs\<cdot>((f \<rightleftharpoons> tb) . c_abpOut) = tsAbs\<cdot>(tb . c_abpIn)"
-  oops 
-
+definition idTSPF2 :: "('a MABP tstream\<^sup>\<Omega>) ufun" where
+"idTSPF2 \<equiv> Abs_cufun (\<lambda> x. (ubDom\<cdot>x = {c_abpOut}) \<leadsto> Abs_ubundle[c_idOut \<mapsto> x . c_abpOut])"
 
 
 (* ----------------------------------------------------------------------- *)
 section \<open>lemmata\<close>
 (* ----------------------------------------------------------------------- *)
 
+
 subsection \<open>general\<close>
+
 
 lemma tsmap_id[simp]: assumes "inj f" shows "tsMap (inv f)\<cdot>(tsMap f\<cdot>ts) = ts"
 apply(induction ts)
@@ -367,8 +144,10 @@ by(simp_all add: assms tsmap_delayfun  tsmap_mlscons)
 lemma med_ora_length: assumes "#({True} \<ominus> ora) = \<infinity>"
   shows "#ora = \<infinity>"
   using assms sfilterl4 by auto  
-  
+
+
 subsection \<open>datatype\<close>
+
 
   (* inverse BoolPair applied to BoolPair is identity *)
 lemma data_bool_pair_inv [simp]: "(invBoolPair) (BoolPair x) = x"
@@ -383,132 +162,22 @@ lemma data_data_inv [simp]: "(inv Data) (Data x) = x"
   by (meson MABP.inject(3) f_inv_into_f rangeI)
 
 
-subsection \<open>id\<close>
-
-lemma id_result_well: "ubWell [c_idOut \<mapsto> x . c_abpOut]"
-  apply (rule ubwellI)
-  apply (simp add: domIff)
-  sorry
-
-lemma id_in_out_eq: assumes "ubDom\<cdot>(x::'a::uscl\<^sup>\<Omega>) = {c_abpOut}"
-  shows "((\<lambda> (x::'a::uscl\<^sup>\<Omega>). (ubDom\<cdot>x = {c_abpOut}) \<leadsto> Abs_ubundle [c_idOut \<mapsto> x . c_abpOut])\<rightharpoonup>(x::'a::uscl\<^sup>\<Omega>)) . c_idOut= (x::'a::uscl\<^sup>\<Omega>) . c_abpOut"
-  apply simp
-  apply (rule, rule)
-   apply (simp_all add: assms)
-   by (simp add: id_result_well ubgetch_ubrep_eq)
-
- thm Rep_ubundle_inject
-lemma id_tspf_cont: "cont (\<lambda> x. (ubDom\<cdot>x = {c_abpOut}) \<leadsto> Abs_ubundle [c_idOut \<mapsto> x . c_abpOut])"
-  apply (rule contI2)
-   apply (rule monofunI)
-   apply (case_tac "(ubDom\<cdot>x = {c_abpOut})")
-    apply (frule ubcldom_fix)
-    apply (simp, rule, rule)
-  apply (rule some_below)
-     apply (subst below_ubundle_def)
-     apply (simp add: id_result_well part_below ubgetch_below ubclDom_ubundle_def)
-    apply (simp add: ubdom_below) +
-  apply (rule, rule, rule)
-  apply (subst some_lub_chain_eq3)
-   apply (rule chainI)
-   apply (simp add: id_result_well po_class.chainE ubgetch_below ubrep_lessI)
-proof - 
-  fix Y::"nat \<Rightarrow> 'a\<^sup>\<Omega>"
-  assume a1: "ubDom\<cdot>(Lub Y) = {c_abpOut}" and chain_Y: "chain Y" 
-  have f0: "\<And> i. ubDom\<cdot>(Y i) = {c_abpOut}"
-    by (simp add: a1 chain_Y)
-  have f1: "chain (\<lambda> i. [c_idOut \<mapsto> Y i  .  c_abpOut])"
-    by (simp add: chain_Y part_map_chain)
-  have f2: "ubWell (\<Squnion>i::nat. [c_idOut \<mapsto> Y i  .  c_abpOut])"
-    using adm_def f1 id_result_well ubWell_adm by auto
-  have f3: "chain (\<lambda>i::nat. Abs_ubundle [c_idOut \<mapsto> Y i  .  c_abpOut])"
-    apply (rule chainI)
-    by (simp add: chain_Y id_result_well po_class.chainE ubgetch_below ubrep_lessI)
-  have f4: "Rep_ubundle (Abs_ubundle (\<Squnion>i::nat. [c_idOut \<mapsto> Y i  .  c_abpOut])) = Rep_ubundle (\<Squnion>i::nat. Abs_ubundle [c_idOut \<mapsto> Y i  .  c_abpOut])"
-    apply (simp add: f2)
-    by (metis (mono_tags, lifting) f3 id_result_well lub_eq ubrep_lub ubrep_ubabs)
-  have f5: "(Abs_ubundle (\<Squnion>i::nat. [c_idOut \<mapsto> Y i  .  c_abpOut])) = (\<Squnion>i::nat. Abs_ubundle [c_idOut \<mapsto> Y i  .  c_abpOut])"
-    using Rep_ubundle_inject f4 by blast
-  have f6: "chain (\<lambda> i. (Y i) . c_abpOut)"
-    by (simp add: chain_Y)
-  have f7: "dom [c_idOut \<mapsto> \<Squnion>i::nat. Y i  .  c_abpOut] = dom (\<Squnion>i::nat. [c_idOut \<mapsto> Y i  .  c_abpOut])"
-    by (metis (no_types, lifting) dom_fun_upd f1 option.simps(3) part_dom_lub)
-  have f8: "\<And> i. dom (\<Squnion>i::nat. [c_idOut \<mapsto> Y i  .  c_abpOut]) = dom [c_idOut \<mapsto> Y i  .  c_abpOut]"
-    using f7 by auto
-  have f9: "\<And> i. dom [c_idOut \<mapsto> Y i  .  c_abpOut] = {c_idOut}"
-    by (simp add: domIff)
-  have f10: "\<And> x. x \<noteq> c_idOut \<Longrightarrow> (\<Squnion>i::nat. [c_idOut \<mapsto> Y i  .  c_abpOut]) x = None"
-    using dom_def f8 by auto
-  have f11: "\<forall> i . [c_idOut \<mapsto> Y i  .  c_abpOut] c_idOut \<sqsubseteq> (\<Squnion>i::nat. [c_idOut \<mapsto> Y i  .  c_abpOut]) c_idOut"
-    using fun_below_iff 
-    by (metis (mono_tags, lifting) f1 is_ub_thelub)
-  have f12: "\<Squnion> i. ([c_idOut \<mapsto> Y i  .  c_abpOut] c_idOut) \<sqsubseteq> (\<Squnion>i::nat. [c_idOut \<mapsto> Y i  .  c_abpOut]) c_idOut"
-    using f11 by auto
-  have f13: "Some (\<Squnion>i::nat. Y i  .  c_abpOut) =  (\<Squnion>i::nat. Some (Y i  .  c_abpOut))"
-    apply (subst some_lub_chain_eq3)
-     apply (rule chainI)
-     apply (simp add: chain_Y monofun_cfun_arg po_class.chainE)
-    by simp
-  have f14: "(\<Squnion>i::nat. Some (Y i  .  c_abpOut)) = (\<Squnion> i. ([c_idOut \<mapsto> Y i  .  c_abpOut] c_idOut))"
-    by simp
-  have f15: " Some (\<Squnion>i::nat. Y i  .  c_abpOut) \<sqsubseteq> (\<Squnion>i::nat. [c_idOut \<mapsto> Y i  .  c_abpOut]) c_idOut"
-    apply (subst f13)
-    apply (subst f14)
-    using f1 lub_fun by fastforce
-  have f6: "[c_idOut \<mapsto> \<Squnion>i::nat. Y i  .  c_abpOut] \<sqsubseteq> (\<Squnion>i::nat. [c_idOut \<mapsto> Y i  .  c_abpOut])"
-    apply (simp add: fun_below_iff)
-    using f10 f15 by auto
-  show "Some (Abs_ubundle [c_idOut \<mapsto> Lub Y  .  c_abpOut]) \<sqsubseteq> Some (\<Squnion>i::nat. Abs_ubundle [c_idOut \<mapsto> Y i  .  c_abpOut])"
-    apply (subst contlub_cfun_arg, simp add: chain_Y)
-    apply (rule some_below)
-    apply (fold f5)
-  proof -
-    have "(\<Squnion>n. [c_idOut \<mapsto> Y n . c_abpOut] c_idOut) = Some (\<Squnion>n. Y n . c_abpOut)"
-      using f13 f14 by presburger
-    then have "(\<Squnion>n. [c_idOut \<mapsto> Y n . c_abpOut]) = [c_idOut \<mapsto> \<Squnion>n. Y n . c_abpOut]"
-      by (simp add: f1 fun_belowI lub_fun po_eq_conv)
-    then show "Abs_ubundle [c_idOut \<mapsto> \<Squnion>n. Y n . c_abpOut] \<sqsubseteq> Abs_ubundle (\<Squnion>n. [c_idOut \<mapsto> Y n . c_abpOut])"
-      by simp
-  qed
-qed
-
-
-
-lemma id_tspf_well: "ufWell (Abs_cfun (\<lambda> x. (ubDom\<cdot>x = {c_abpOut}) \<leadsto> Abs_ubundle [c_idOut \<mapsto> x . c_abpOut]))"
-  apply (rule ufun_wellI)
-    apply (simp_all add: Abs_cfun_inverse2 id_tspf_cont ubclDom_ubundle_def)
-    apply (simp_all add: domIff2)
-  apply (simp add: ubDom_def)
-  by (simp add: id_result_well)
-
-lemma id_tspf_dom: "ufDom\<cdot>id_TSPF = {c_abpOut}"
-  apply (simp add: id_TSPF_def ufDom_def)
-  apply (simp add: id_tspf_well id_tspf_cont)
-  apply (simp add: domIff)
-  by (metis ubclDom_h ubclDom_ubundle_def)
-
-lemma id_tspf_ran: "ufRan\<cdot>id_TSPF = {c_idOut}"
-  apply (simp add: ufran_least)
-  apply (simp add: ubclDom_ubundle_def ubclLeast_ubundle_def)
-proof -
-  have f1: "ufDom\<cdot> (Abs_cufun (\<lambda>u. (ubDom\<cdot>u = {c_abpOut})\<leadsto>Abs_ubundle [c_idOut \<mapsto> u . c_abpOut::'a MABP tstream])) = {c_abpOut}"
-    by (metis (no_types) id_TSPF_def id_tspf_dom)
-  have "\<And>c. ubWell [c \<mapsto> \<bottom>::'a MABP tstream]"
-    by (metis (no_types) insertI1 option.sel ubWell_single_channel ubgetchE ubleast_ubdom ubleast_ubgetch)
-  then show "ubDom\<cdot> (id_TSPF \<rightleftharpoons> (ubLeast (ufDom\<cdot> (id_TSPF::('a MABP tstream\<^sup>\<Omega>) ufun))::'a MABP tstream\<^sup>\<Omega>)) = {c_idOut}"
-    using f1 by (simp add: id_TSPF_def id_tspf_cont id_tspf_well ubdom_ubrep_eq)
-qed
-
 subsection \<open>receiver\<close>
+
 
 subsubsection \<open>defs\<close>
 
-      (* helper functions to prove cont *)
+
+(* helper functions to prove cont *)
 definition recvCH1 :: "'a MABP tstream\<^sup>\<Omega> \<Rightarrow> 'a MABP tstream"  where
 "recvCH1 \<equiv> (\<lambda> x. tsMap Bool\<cdot>(fst (tsRec\<cdot>((tsMap invBoolPair)\<cdot>(x .c_dr)))))"
 
 definition recvCH2 :: "'a MABP tstream\<^sup>\<Omega> \<Rightarrow> 'a MABP tstream"  where
 "recvCH2 \<equiv> (\<lambda> x. tsMap Data\<cdot>(snd (tsRec\<cdot>((tsMap invBoolPair)\<cdot>(x .c_dr)))))"
+
+
+subsubsection \<open>mono/cont\<close>
+
 
 lemma recvCH1_contlub: assumes "chain Y"
   shows "recvCH1 ((\<Squnion>i. Y i)) = (\<Squnion>i. (recvCH1 ((Y i))))"
@@ -533,30 +202,12 @@ lemma recv_tsb_well [simp]:
                                   c_abpOut \<mapsto> tsMap Data\<cdot>(snd (tsRec\<cdot>((tsMap invBoolPair)\<cdot>(x . c_dr))))]"
   apply (rule ubwellI)
   apply (simp add: tsmap_tsdom_range)
-proof -
-  fix c::channel
-  assume a1: "c = c_abpOut \<or> c = c_ar"
-  show "(c = c_ar \<longrightarrow> usclOkay c_ar (tsMap Bool\<cdot>(fst (tsRec\<cdot>(tsMap invBoolPair\<cdot>(x  .  c_dr)))))) \<and>
-                  (c \<noteq> c_ar \<longrightarrow> (c = c_abpOut \<longrightarrow> usclOkay c_abpOut (tsMap Data\<cdot>(snd (tsRec\<cdot>(tsMap invBoolPair\<cdot>(x  .  c_dr)))))) \<and> (c \<noteq> c_abpOut \<longrightarrow> usclOkay c (the None)))"
-    apply rule
-    using tsmap_tsdom_range usclOkay_tstream_def apply fastforce
-  proof rule
-    assume a2: "c \<noteq> c_ar"
-    have f1: "c = c_abpOut"
-      using a1 a2 by auto
-    show "(c = c_abpOut \<longrightarrow> usclOkay c_abpOut (tsMap Data\<cdot>(snd (tsRec\<cdot>(tsMap invBoolPair\<cdot>(x  .  c_dr)))))) \<and> (c \<noteq> c_abpOut \<longrightarrow> usclOkay c (the None))"
-      apply rule
-      using tsmap_tsdom_range usclOkay_tstream_def apply fastforce
-      by (simp add: f1)
-  qed
-qed
+  by (metis ctype_MABP.simps(2) ctype_MABP.simps(6) tsmap_tsdom_range usclOkay_tstream_def)
 
 lemma recv_tsb_dom: "ubclDom\<cdot>(Abs_ubundle([c_ar \<mapsto> tsMap Bool\<cdot>(fst (tsRec\<cdot>((tsMap invBoolPair)\<cdot>(x . c_dr)))),
                               c_abpOut \<mapsto> tsMap Data\<cdot>(snd (tsRec\<cdot>((tsMap invBoolPair)\<cdot>(x . c_dr))))]))
                      = {c_ar, c_abpOut}"
   by (simp add: insert_commute ubclDom_ubundle_def ubdom_ubrep_eq)
-
-
 
 lemma rec_tsb_mono: "\<And>(x::'a MABP tstream ubundle) y::'a MABP tstream ubundle. ubclDom\<cdot>x = {c_dr} \<Longrightarrow> x \<sqsubseteq> y \<Longrightarrow>
           Abs_ubundle([c_ar \<mapsto> tsMap Bool\<cdot>(fst (tsRec\<cdot>(tsMap invBoolPair\<cdot>(x  .  c_dr)))),
@@ -565,8 +216,7 @@ lemma rec_tsb_mono: "\<And>(x::'a MABP tstream ubundle) y::'a MABP tstream ubund
              c_abpOut \<mapsto> tsMap Data\<cdot>(snd (tsRec\<cdot>(tsMap invBoolPair\<cdot>(y  .  c_dr))))])"
       apply (rule ub_below)
        apply (simp_all add: ubdom_below ubdom_ubrep_eq ubgetch_ubrep_eq)
-       by (simp add: fst_monofun snd_monofun monofun_cfun_arg ubgetch_below)
-                                                                       
+       by (simp add: fst_monofun snd_monofun monofun_cfun_arg ubgetch_below)     
 
 lemma recvTSPF_mono [simp]: "monofun (\<lambda> x. (ubclDom\<cdot>x = {c_dr}) \<leadsto>
                                     Abs_ubundle([c_ar \<mapsto> tsMap Bool\<cdot>(fst (tsRec\<cdot>((tsMap invBoolPair)\<cdot>(x . c_dr)))),
@@ -595,7 +245,6 @@ proof (rule lubgetCh)
                        c_abpOut \<mapsto> tsMap Data\<cdot>(snd (tsRec\<cdot>(tsMap invBoolPair\<cdot>(Y i  .  c_dr))))]))"
      using assms(3) recv_tsb_dom tb_chain ubcldom_lub_eq2I by blast
 qed
-
 
   (* show that recTSPF is cont, proof concept taken from TSPF_Template_CaseStudy *)
 lemma recvTSPF_cont [simp]:
@@ -648,7 +297,9 @@ proof (rule ufun_contI, simp add: rec_tsb_mono)
 qed
 
 
-  subsubsection \<open>tspf_well\<close>
+subsubsection \<open>uf_well/tickCount\<close>
+
+
 declare [[simp_trace_new]]
  (* show that the recvTSPF fulfills the tickcount property *)
 lemma recvTSPF_tick: assumes "ubDom\<cdot>b = {c_dr}" and "(ubLen b) = n"
@@ -672,7 +323,6 @@ proof -
     apply (simp add: ubgetch_ubrep_eq)
     by (metis f2 f3 usclLen_tstream_def)
 qed
-
 
   (* recvTSPF is an actual TSPF *)
 lemma recvTSPF_well [simp]:
@@ -699,18 +349,18 @@ lemma recv_tspfran: "ufRan\<cdot>(recvTSPF) = {c_ar, c_abpOut}"
     apply (simp only: recvTSPF_def)
   by (simp add:  recv_tsb_dom ubcldom_least_cs) 
 
+
 subsection \<open>sender\<close>
-(*
 
-  (* lift a sender function to a TSPF *)
-definition senderTSPF :: "'a sender \<Rightarrow> ('a MABP tstream\<^sup>\<Omega>) ufun" where
-"senderTSPF se \<equiv> Abs_cufun (\<lambda> x. (ubclDom\<cdot>x = {c_as, c_abpIn})
-                \<leadsto> Abs_ubundle([c_ds \<mapsto> tsMap BoolPair\<cdot>(se\<cdot>(tsMap invData\<cdot>(x . c_abpIn))\<cdot>(tsMap invBool\<cdot>(x . c_as)))]))"
 
-*)
+subsubsection \<open>defs\<close>
+
 
 definition senderCH :: "'a sender \<Rightarrow> 'a MABP tstream\<^sup>\<Omega> \<Rightarrow> 'a MABP tstream"  where
 "senderCH se \<equiv> (\<lambda> x. tsMap BoolPair\<cdot>(se\<cdot>(tsMap invData\<cdot>(x . c_abpIn))\<cdot>(tsMap invBool\<cdot>(x . c_as))))"
+
+
+subsubsection \<open>mono/cont\<close>
 
 
 lemma senderCH_contlub: assumes "chain Y"
@@ -769,7 +419,9 @@ proof (rule ufun_contI, simp add: sender_tsb_mono)
     by (simp add: a1 senderCH_contlub)
 qed
 
-subsubsection \<open>tspf_well\<close>
+
+subsubsection \<open>uf_well/tickCount\<close>
+
 
 lemma ublen_min_eq_2_ch: assumes "ubDom\<cdot>b = {ch1, ch2}"
   shows "(ubLen b) = min (usclLen\<cdot>(b . ch1)) (usclLen\<cdot>(b . ch2))"
@@ -894,24 +546,24 @@ lemma sender_tspfran: "ufRan\<cdot>(senderTSPF se) = {c_ds}"
   by (simp add:  sender_tsb_dom1 ubcldom_least_cs) 
 
 
-  subsection \<open>medium_rs\<close>
+subsection \<open>medium\<close>
 
 subsubsection \<open>defs\<close>
 
-definition medRSH :: "bool stream \<Rightarrow> 'a MABP tstream\<^sup>\<Omega> \<Rightarrow> 'a MABP tstream"  where
-"medRSH bst \<equiv> (\<lambda> x. (tsMap::(bool \<Rightarrow> 'a MABP) \<Rightarrow> bool tstream \<rightarrow> 'a MABP tstream) Bool\<cdot>(tsMed\<cdot>(tsMap invBool\<cdot>(x  .  c_ar))\<cdot>bst))"
+definition medH :: "bool stream \<Rightarrow> channel \<Rightarrow> ('b \<Rightarrow> 'a MABP) \<Rightarrow> 'a MABP tstream\<^sup>\<Omega> \<Rightarrow> 'a MABP tstream"  where
+"medH bst In f\<equiv> (\<lambda> x. tsMap f\<cdot>(tsMed\<cdot>(tsMap (inv f)\<cdot>(x  .  In))\<cdot>bst))"
 
-lemma medrsh_cont [simp]: "cont (medRSH bst)"
-  by (simp add: medRSH_def)
+lemma medh_cont [simp]: "cont (medH bst In f)"
+  by (simp add: medH_def)
 
-lemma medrsh_contlub: assumes "chain Y"
-  shows "(medRSH bst) ((\<Squnion>i. Y i)) = (\<Squnion>i. ((medRSH bst) ((Y i))))"
+lemma medh_contlub: assumes "chain Y"
+  shows "(medH bst In f) ((\<Squnion>i. Y i)) = (\<Squnion>i. ((medH bst In f) ((Y i))))"
   apply (rule cont2contlubE)
   by (simp_all add: assms)
 
-lemma to_medrsh: "tsMap Bool\<cdot>(tsMed\<cdot>(tsMap invBool\<cdot>(x  .  c_ar))\<cdot>bst)
-                  = ((medRSH :: bool stream \<Rightarrow> 'a MABP tstream\<^sup>\<Omega> \<Rightarrow> 'a MABP tstream) bst) x"
-  by (simp add: medRSH_def)
+lemma to_medh: "tsMap f\<cdot>(tsMed\<cdot>(tsMap (inv f)\<cdot>(x  .  In))\<cdot>bst)
+                  = ((medH :: bool stream \<Rightarrow> channel \<Rightarrow> ('b \<Rightarrow> 'a MABP) \<Rightarrow> 'a MABP tstream\<^sup>\<Omega> \<Rightarrow> 'a MABP tstream) bst In f) x"
+  by (simp add: medH_def)
 
 subsubsection \<open>pre\<close>
 
@@ -920,328 +572,675 @@ lemma tsmed_input_cont [simp]: "cont (\<lambda> x. tsMed\<cdot>x\<cdot>bst)"
 
 lemma tsmed_input_mono [simp]: "monofun (\<lambda> x. tsMed\<cdot>x\<cdot>bst)"
   using cont2mono tsmed_input_cont by blast
+(*
+lemma medrs_tsb_well [simp]: "ubWell [as \<mapsto> tsMap Bool\<cdot>(tsMed\<cdot>(tsMap invBool\<cdot>(x . ar))\<cdot>bst)]"
+  apply (rule ubwellI)
+  apply (simp add: usOkay_tstream_def)
+  by (simp add: tsmap_tsdom_range) (*"tsDom\<cdot>(tsMap f\<cdot>ts) \<subseteq> range f"*)
+  (*by (simp add: tsmap_tsdom_range usOkay_tstream_def)*)*)
 
-
-lemma medrs_tsb_well [simp]: "ubWell  [c_as \<mapsto> tsMap Bool\<cdot>(tsMed\<cdot>(tsMap invBool\<cdot>(x . c_ar))\<cdot>bst)]"
+lemma med_tsb_well [simp]: assumes "(ctype::channel \<Rightarrow> 'a MABP set) Out = range f"        (*bool \<rightarrow> f*)
+  shows "ubWell [Out \<mapsto> (tsMap f\<cdot>(tsMed\<cdot>(tsMap (inv f)\<cdot>((x . In):: 'a MABP tstream))\<cdot>bst):: 'a MABP tstream)]"
   apply (rule ubwellI)
   apply (simp add: usclOkay_tstream_def)
-  by (simp add: tsmap_tsdom_range)
+  by (simp add: assms tsmap_tsdom_range)
 
-lemma medrs_tsb_dom: "ubclDom\<cdot>(Abs_ubundle([c_as \<mapsto> tsMap Bool\<cdot>(tsMed\<cdot>(tsMap invBool\<cdot>(x . c_ar))\<cdot>bst)])) = {c_as}"
-  apply (simp add: ubclDom_ubundle_def)
-  by (simp add: ubdom_ubrep_eq)
+
+lemma med_tsb_dom: assumes "(ctype::channel \<Rightarrow> 'a MABP set) Out = range f"
+  shows "ubDom\<cdot>(Abs_ubundle([Out \<mapsto> (tsMap f\<cdot>(tsMed\<cdot>(tsMap (inv f)\<cdot>((x . In):: 'a MABP tstream))\<cdot>bst):: 'a MABP tstream)])) = {Out}"
+  by  (simp add: assms ubdom_ubrep_eq)
 
 
 subsubsection \<open>cont\<close>
 
   (* prerequirement for the mono proofs of the tspf *)
-lemma medrs_tsb_mono: "\<And>(x::'a MABP tstream\<^sup>\<Omega>) y::'a MABP tstream\<^sup>\<Omega>.
-       ubclDom\<cdot>x = {c_ar} \<Longrightarrow> x \<sqsubseteq> y \<Longrightarrow> Abs_ubundle([c_as \<mapsto> (tsMap::(bool \<Rightarrow> 'a MABP) \<Rightarrow> bool tstream \<rightarrow> 'a MABP tstream) Bool\<cdot>(tsMed\<cdot>(tsMap invBool\<cdot>(x  .  c_ar))\<cdot>bst)]) \<sqsubseteq> Abs_ubundle([c_as \<mapsto> tsMap Bool\<cdot>(tsMed\<cdot>(tsMap invBool\<cdot>(y  .  c_ar))\<cdot>bst)])"
-  apply (simp_all add: ubclDom_ubundle_def)
-  apply (rule ub_below)
+lemma med_tsb_mono: assumes "(ctype::channel \<Rightarrow> 'a MABP set) Out = range f"
+  shows "\<And>(x::'a MABP tstream\<^sup>\<Omega>) y::'a MABP tstream\<^sup>\<Omega>.
+       ubDom\<cdot>x = {In} \<Longrightarrow> x \<sqsubseteq> y \<Longrightarrow> Abs_ubundle([Out \<mapsto> (tsMap f\<cdot>(tsMed\<cdot>(tsMap (inv f)\<cdot>((x . In):: 'a MABP tstream))\<cdot>bst):: 'a MABP tstream)]) \<sqsubseteq> Abs_ubundle([Out \<mapsto> (tsMap f\<cdot>(tsMed\<cdot>(tsMap (inv f)\<cdot>((y . In):: 'a MABP tstream))\<cdot>bst):: 'a MABP tstream)])"
   apply (simp_all add: ubdom_below ubdom_ubrep_eq ubgetch_ubrep_eq)
-  apply (simp add: to_medrsh)
-  using cont2mono medrsh_cont monofun_def by blast
+  apply (rule ub_below)
+  apply (simp_all add: assms ubdom_below ubdom_ubrep_eq ubgetch_ubrep_eq)
+  by (simp add: monofun_cfun_arg monofun_cfun_fun)
 
+lemma med_mono [simp]: assumes "(ctype::channel \<Rightarrow> 'a MABP set) Out = range f"
+  shows "monofun (\<lambda> x::'a MABP tstream\<^sup>\<Omega>. (ubDom\<cdot>x = {In})
+                           \<leadsto> Abs_ubundle([Out \<mapsto> tsMap
+                                f\<cdot>(tsMed\<cdot>(tsMap (inv f)\<cdot>((x . In):: 'a MABP tstream))\<cdot>bst)]))"
+  by (simp add: assms med_tsb_mono monofun_def some_below ubdom_below)
 
-lemma medrs_mono [simp]: "monofun (\<lambda> x::'a MABP tstream\<^sup>\<Omega>. (ubclDom\<cdot>x = {c_ar})
-                           \<leadsto> Abs_ubundle([c_as \<mapsto> (tsMap::(bool \<Rightarrow> 'a MABP) \<Rightarrow> bool tstream \<rightarrow> 'a MABP tstream)
-                                Bool\<cdot>(tsMed\<cdot>(tsMap invBool\<cdot>(x . c_ar))\<cdot>bst)]))"
-  apply (rule ufun_monoI2)
-  by (simp add: medrs_tsb_mono)
-
-lemma medrs_tsb_getc: assumes "chain (Y::nat \<Rightarrow> 'a MABP tstream\<^sup>\<Omega>)" and "ubclDom\<cdot>(\<Squnion>i::nat. Y i) = {c_ar}"
-                      and "c = c_as"
-  shows "(\<Squnion>i::nat. Abs_ubundle([c_as \<mapsto> (tsMap::(bool \<Rightarrow> 'a MABP) \<Rightarrow> bool tstream \<rightarrow> 'a MABP tstream) Bool\<cdot>(tsMed\<cdot>(tsMap invBool\<cdot>(Y i  .  c_ar))\<cdot>bst)]))  .  c_as
-          =  (\<Squnion>i::nat. (Abs_ubundle([c_as \<mapsto> (tsMap::(bool \<Rightarrow> 'a MABP) \<Rightarrow> bool tstream \<rightarrow> 'a MABP tstream) Bool\<cdot>(tsMed\<cdot>(tsMap invBool\<cdot>(Y i  .  c_ar))\<cdot>bst)])) . c_as)"
-proof (rule lubgetCh)
-  have f2: "\<And> i. ubclDom\<cdot>(Y i) =  ubclDom\<cdot>(\<Squnion>i. Y i)"
-    by (simp add: assms(1) ubclDom_ubundle_def)
-  show tb_chain: "chain (\<lambda>i::nat. Abs_ubundle([c_as \<mapsto> (tsMap::(bool \<Rightarrow> 'a MABP) \<Rightarrow> bool tstream \<rightarrow> 'a MABP tstream) Bool\<cdot>(tsMed\<cdot>(tsMap invBool\<cdot>(Y i  .  c_ar))\<cdot>bst)]))"
-    by (simp add: assms(1) assms(2) f2 medrs_tsb_mono po_class.chainE po_class.chainI)
-  show "c_as \<in> ubclDom\<cdot>(\<Squnion>i::nat. Abs_ubundle([c_as \<mapsto> (tsMap::(bool \<Rightarrow> 'a MABP) \<Rightarrow> bool tstream \<rightarrow> 'a MABP tstream) Bool\<cdot>(tsMed\<cdot>(tsMap invBool\<cdot>(Y i  .  c_ar))\<cdot>bst)]))"
-    by (metis (mono_tags, lifting) insert_iff medrs_tsb_dom tb_chain ubclDom_ubundle_def ubdom_chain_eq2)
+lemma med_tsb_getc: assumes "chain (Y::nat \<Rightarrow> 'a MABP tstream\<^sup>\<Omega>)" and "ubDom\<cdot>(\<Squnion>i::nat. Y i) = {In}"
+                      and "c = Out" and "(ctype::channel \<Rightarrow> 'a MABP set) Out = range f"
+  shows "(\<Squnion>i::nat. Abs_ubundle([Out \<mapsto> tsMap f\<cdot>(tsMed\<cdot>(tsMap (inv f)\<cdot>(Y i  .  In))\<cdot>bst)]))  .  Out
+          =  (\<Squnion>i::nat. (Abs_ubundle([Out \<mapsto> tsMap f\<cdot>(tsMed\<cdot>(tsMap (inv f)\<cdot>(Y i  .  In))\<cdot>bst)])) . Out)"
+proof -
+  have f1: "\<forall>c f u ca ua s. ((ctype c::'a MABP set) \<noteq> range f \<or> ubDom\<cdot>u \<noteq> {ca} \<or> u \<notsqsubseteq> ua) \<or> Abs_ubundle [c \<mapsto> tsMap f\<cdot> (tsMed\<cdot>(tsMap (inv f)\<cdot>(u . ca)::'b tstream)\<cdot> s)] \<sqsubseteq> Abs_ubundle [c \<mapsto> tsMap f\<cdot>(tsMed\<cdot>(tsMap (inv f)\<cdot>(ua . ca))\<cdot>s)]"
+    using med_tsb_mono by blast
+  obtain nn :: "(nat \<Rightarrow> 'a MABP tstream\<^sup>\<Omega>) \<Rightarrow> nat" where
+    f2: "\<forall>f. (\<not> chain f \<or> (\<forall>n. f n \<sqsubseteq> f (Suc n))) \<and> (chain f \<or> f (nn f) \<notsqsubseteq> f (Suc (nn f)))"
+    using po_class.chain_def by moura
+  then have f3: "\<forall>n. Y n \<sqsubseteq> Y (Suc n)"
+    by (metis (no_types) assms(1))
+  have "ubDom\<cdot> (Y (nn (\<lambda>n. Abs_ubundle [Out \<mapsto> tsMap f\<cdot> (tsMed\<cdot>(tsMap (inv f)\<cdot>(Y n . In))\<cdot> bst)]))) = {In}"
+    by (simp add: assms(1) assms(2))
+  then have "chain (\<lambda>n. Abs_ubundle [Out \<mapsto> tsMap f\<cdot> (tsMed\<cdot>(tsMap (inv f)\<cdot>(Y n . In))\<cdot>bst)])"
+    using f3 f2 f1 by (meson assms(4))
+  then show ?thesis
+    using contlub_cfun_arg by blast
 qed
+(*proof (rule lubgetCh)
+  have f2: "\<And> i. ubDom\<cdot>(Y i) =  ubDom\<cdot>(\<Squnion>i. Y i)"
+    by (simp add: assms(1))
+  show tb_chain: "chain (\<lambda>i::nat. Abs_ubundle([Out \<mapsto> tsMap f\<cdot>(tsMed\<cdot>(tsMap (inv f)\<cdot>(Y i  .  In))\<cdot>bst)]))"
+    by (simp add: assms po_class.chainE po_class.chainI med_tsb_mono)
+  show "Out \<in> ubDom\<cdot>(\<Squnion>i::nat. Abs_ubundle([Out \<mapsto> tsMap f\<cdot>(tsMed\<cdot>(tsMap (inv f)\<cdot>(Y i  .  In))\<cdot>bst)]))"
+    by (metis (mono_tags, lifting) assms(4) insertCI med_tsb_dom tb_chain ubdom_chain_eq2)
+qed*)
 
-
-
-lemma medrs_cont [simp]: "cont (\<lambda> x::'a MABP tstream\<^sup>\<Omega>. (ubclDom\<cdot>x = {c_ar})
-                           \<leadsto> Abs_ubundle([c_as \<mapsto> (tsMap::(bool \<Rightarrow> 'a MABP) \<Rightarrow> bool tstream \<rightarrow> 'a MABP tstream)
-                                Bool\<cdot>(tsMed\<cdot>(tsMap invBool\<cdot>(x . c_ar))\<cdot>bst)]))"
-proof (rule ufun_contI)
-  show medrs_mo : "\<And>(x::'a MABP tstream\<^sup>\<Omega>) y::'a MABP tstream\<^sup>\<Omega>.
-       ubclDom\<cdot>x = {c_ar} \<Longrightarrow> x \<sqsubseteq> y \<Longrightarrow> Abs_ubundle [c_as \<mapsto> tsMap Bool\<cdot>(tsMed\<cdot>(tsMap invBool\<cdot>(x  .  c_ar))\<cdot>bst)] 
-          \<sqsubseteq> Abs_ubundle [c_as \<mapsto> tsMap Bool\<cdot>(tsMed\<cdot>(tsMap invBool\<cdot>(y  .  c_ar))\<cdot>bst)]"
-    by (simp add: medrs_tsb_well monofun_cfun_arg monofun_cfun_fun option.distinct(1) option.sel ub_below ubdom_ubrep_eq ubgetch_ubrep_eq)
-
-  have f1: " \<And>Y::nat \<Rightarrow> 'a MABP tstream\<^sup>\<Omega>. chain Y \<Longrightarrow> ubclDom\<cdot>(\<Squnion>i::nat. Y i) = {c_ar} \<Longrightarrow>
-       ubclDom\<cdot>(\<Squnion>i::nat. Abs_ubundle([c_as \<mapsto> (tsMap::(bool \<Rightarrow> 'a MABP) \<Rightarrow> bool tstream \<rightarrow> 'a MABP tstream) Bool\<cdot>(tsMed\<cdot>(tsMap invBool\<cdot>(Y i  .  c_ar))\<cdot>bst)])) = {c_as}"
-    by (metis (mono_tags, lifting) medrs_tsb_dom medrs_tsb_mono po_class.chain_def ubcldom_lub_eq2I)
-  show "\<And>Y::nat \<Rightarrow> 'a MABP tstream\<^sup>\<Omega>. chain Y \<Longrightarrow> ubclDom\<cdot>(\<Squnion>i::nat. Y i) = {c_ar} \<Longrightarrow>
-       Abs_ubundle([c_as \<mapsto> (tsMap::(bool \<Rightarrow> 'a MABP) \<Rightarrow> bool tstream \<rightarrow> 'a MABP tstream) Bool\<cdot>(tsMed\<cdot>(tsMap invBool\<cdot>((\<Squnion>i::nat. Y i)  .  c_ar))\<cdot>bst)]) \<sqsubseteq> (\<Squnion>i::nat. Abs_ubundle([c_as \<mapsto> tsMap Bool\<cdot>(tsMed\<cdot>(tsMap invBool\<cdot>(Y i  .  c_ar))\<cdot>bst)]))"
+lemma med_cont [simp]: assumes "(ctype::channel \<Rightarrow> 'a MABP set) Out = range f"
+  shows "cont (\<lambda> x::'a MABP tstream\<^sup>\<Omega>. (ubDom\<cdot>x = {In})
+                           \<leadsto> Abs_ubundle([Out \<mapsto> (tsMap
+                                f\<cdot>(tsMed\<cdot>(tsMap (inv f)\<cdot>((x . In):: 'a MABP tstream))\<cdot>bst):: 'a MABP tstream)]))"
+proof -
+  have g1: " \<And>Y::nat \<Rightarrow> 'a MABP tstream\<^sup>\<Omega>. chain Y \<Longrightarrow> ubDom\<cdot>(\<Squnion>i::nat. Y i) = {In} \<Longrightarrow>
+       ubDom\<cdot>(\<Squnion>i::nat. Abs_ubundle([Out \<mapsto> tsMap f\<cdot>(tsMed\<cdot>(tsMap (inv f)\<cdot>(Y i  .  In))\<cdot>bst)])) = {Out}"
   proof -
-    fix Y::"nat \<Rightarrow> 'a MABP tstream\<^sup>\<Omega>"
-    assume chain_Y: "chain Y" and chain_Y_dom: "ubclDom\<cdot>(\<Squnion>i::nat. Y i) = {c_ar}"
-    have f10: "(\<Squnion>i::nat. Abs_ubundle [c_as \<mapsto> tsMap Bool\<cdot>(tsMed\<cdot>(tsMap invBool\<cdot>(Y i  .  c_ar))\<cdot>bst)])  .  c_as =
-                    (\<Squnion>i::nat. Abs_ubundle [c_as \<mapsto> tsMap Bool\<cdot>(tsMed\<cdot>(tsMap invBool\<cdot>(Y i  .  c_ar))\<cdot>bst)]  .  c_as)"
-      apply (rule cont2contlubE, simp)
-      apply (rule chainI)
-      by (simp add: chain_Y monofun_cfun_arg monofun_cfun_fun po_class.chainE ub_below ubdom_ubrep_eq ubgetch_ubrep_eq)
-    show "Abs_ubundle([c_as \<mapsto> (tsMap::(bool \<Rightarrow> 'a MABP) \<Rightarrow> bool tstream \<rightarrow> 'a MABP tstream) Bool\<cdot>(tsMed\<cdot>(tsMap invBool\<cdot>((\<Squnion>i::nat. Y i)  .  c_ar))\<cdot>bst)]) \<sqsubseteq> (\<Squnion>i::nat. Abs_ubundle([c_as \<mapsto> tsMap Bool\<cdot>(tsMed\<cdot>(tsMap invBool\<cdot>(Y i  .  c_ar))\<cdot>bst)]))"
-      apply (rule ub_below)
-       apply (simp_all add: ubdom_below ubdom_ubrep_eq ubgetch_ubrep_eq f1) 
-       apply (metis (mono_tags, lifting) chain_Y chain_Y_dom f1 ubclDom_ubundle_def)
-      apply (subst f10)
-      by (metis (mono_tags, lifting) chain_Y fun_upd_same lub_eq medrs_tsb_well medrsh_contlub not_below2not_eq option.sel to_medrsh ubgetch_ubrep_eq)
+    fix Y :: "nat \<Rightarrow> 'a MABP tstream\<^sup>\<Omega>"
+    assume a1: "chain Y"
+    assume a2: "UBundle.ubDom\<cdot>(\<Squnion>i. Y i) = {In}"
+    obtain nn :: "(nat \<Rightarrow> 'a MABP tstream\<^sup>\<Omega>) \<Rightarrow> nat" where
+      f3: "\<forall>f. (\<not> chain f \<or> (\<forall>n. f n \<sqsubseteq> f (Suc n))) \<and> (chain f \<or> f (nn f) \<notsqsubseteq> f (Suc (nn f)))"
+      using po_class.chain_def by moura
+    have f4: "\<forall>c f u ca ua s. ((ctype c::'a MABP set) \<noteq> range f \<or> UBundle.ubDom\<cdot>u \<noteq> {ca} \<or> u \<notsqsubseteq> ua) \<or> Abs_ubundle [c \<mapsto> tsMap f\<cdot> (tsMed\<cdot>(tsMap (inv f)\<cdot>(u . ca)::'b tstream)\<cdot> s)] \<sqsubseteq> Abs_ubundle [c \<mapsto> tsMap f\<cdot>(tsMed\<cdot>(tsMap (inv f)\<cdot>(ua . ca))\<cdot>s)]"
+      using med_tsb_mono by blast
+    have "UBundle.ubDom\<cdot> (Y (nn (\<lambda>n. Abs_ubundle [Out \<mapsto> tsMap f\<cdot> (tsMed\<cdot>(tsMap (inv f)\<cdot>(Y n . In))\<cdot> bst)]))) = {In}"
+      using a2 a1 by simp
+    then have "chain (\<lambda>n. Abs_ubundle [Out \<mapsto> tsMap f\<cdot> (tsMed\<cdot>(tsMap (inv f)\<cdot>(Y n . In))\<cdot>bst)])"
+      using f4 f3 a1 by (meson assms)
+    then show "UBundle.ubDom\<cdot> (\<Squnion>n. Abs_ubundle [Out \<mapsto> tsMap f\<cdot> (tsMed\<cdot>(tsMap (inv f)\<cdot>(Y n . In))\<cdot>bst)]) = {Out}"
+      using assms med_tsb_dom ubdom_chain_eq2 by blast
   qed
+  (*  by (metis (mono_tags, lifting) assms med_tsb_dom med_tsb_mono po_class.chain_def ubdom_chain_eq2)*) (*geht auch, aber langsam*)
+
+  have g2: "\<And>Y::nat \<Rightarrow> 'a MABP tstream\<^sup>\<Omega>. chain Y \<Longrightarrow> ubDom\<cdot>(\<Squnion>i::nat. Y i) = {In} \<Longrightarrow>
+       Abs_ubundle([Out \<mapsto> tsMap f\<cdot>(tsMed\<cdot>(tsMap (inv f)\<cdot>((\<Squnion>i::nat. Y i)  .  In))\<cdot>bst)]) \<sqsubseteq> (\<Squnion>i::nat. Abs_ubundle([Out \<mapsto> tsMap f\<cdot>(tsMed\<cdot>(tsMap (inv f)\<cdot>(Y i  .  In))\<cdot>bst)]))"
+    apply (rule ub_below)
+    apply (simp_all add: ubdom_below ubdom_ubrep_eq ubgetch_ubrep_eq g1)
+    apply (simp add: assms med_tsb_getc ubdom_ubrep_eq ubgetch_ubrep_eq)
+    apply (simp add: medh_contlub to_medh)
+    proof -
+      fix Y :: "nat \<Rightarrow> 'a MABP tstream\<^sup>\<Omega>" and c :: channel
+      assume a1: "chain Y"
+      assume a2: "UBundle.ubDom\<cdot>(\<Squnion>i. Y i) = {In}"
+      assume a3: "c \<in> UBundle.ubDom\<cdot> (Abs_ubundle [Out \<mapsto> \<Squnion>i. medH bst In f (Y i)])"
+      have f4: "\<forall>f. \<not> ubWell f \<or> Rep_ubundle (Abs_ubundle f::'a MABP tstream\<^sup>\<Omega>) = f"
+        by auto
+      obtain nn :: "(nat \<Rightarrow> 'a MABP tstream) \<Rightarrow> (nat \<Rightarrow> 'a MABP tstream) \<Rightarrow> nat" where
+        f5: "\<forall>f fa. f (nn fa f) \<noteq> fa (nn fa f) \<or> Lub f = Lub fa"
+        by (meson lub_eq)
+      have f6: "\<forall>c f ca u s. (ctype c::'a MABP set) \<noteq> range f \<or> ubWell [c \<mapsto> tsMap f\<cdot> (tsMed\<cdot>(tsMap (inv f)\<cdot>(u . ca)::'b tstream)\<cdot>s)]"
+        by auto
+      then have f7: "ubWell [Out \<mapsto> medH bst In f (Y (nn (\<lambda>n. medH bst In f (Y n)) (\<lambda>n. Abs_ubundle [Out \<mapsto> medH bst In f (Y n)] . Out)))]"
+        by (simp add: assms to_medh)
+      have f8: "\<forall>f n. \<not> chain f \<or> UBundle.ubDom\<cdot>(f n::'a MABP tstream\<^sup>\<Omega>) = UBundle.ubDom\<cdot>(Lub f)"
+        using ubdom_chain_eq2 by blast
+      have f9: "\<forall>c f u ca ua s. ((ctype c::'a MABP set) \<noteq> range f \<or> UBundle.ubDom\<cdot>u \<noteq> {ca} \<or> u \<notsqsubseteq> ua) \<or> Abs_ubundle [c \<mapsto> tsMap f\<cdot> (tsMed\<cdot>(tsMap (inv f)\<cdot>(u . ca)::'b tstream)\<cdot> s)] \<sqsubseteq> Abs_ubundle [c \<mapsto> tsMap f\<cdot>(tsMed\<cdot>(tsMap (inv f)\<cdot>(ua . ca))\<cdot>s)]"
+        using med_tsb_mono by blast
+      obtain nna :: "(nat \<Rightarrow> 'a MABP tstream\<^sup>\<Omega>) \<Rightarrow> nat" where
+        f10: "\<forall>f. (\<not> chain f \<or> (\<forall>n. f n \<sqsubseteq> f (Suc n))) \<and> (chain f \<or> f (nna f) \<notsqsubseteq> f (Suc (nna f)))"
+        using po_class.chain_def by moura
+      then have "Abs_ubundle [Out \<mapsto> medH bst In f (Y (nna (\<lambda>n. Abs_ubundle [Out \<mapsto> medH bst In f (Y n)])))] \<sqsubseteq> Abs_ubundle [Out \<mapsto> medH bst In f (Y (Suc (nna (\<lambda>n. Abs_ubundle [Out \<mapsto> medH bst In f (Y n)]))))]"
+        using f9 a2 a1 by (simp add: assms to_medh)
+      then have f11: "chain (\<lambda>n. Abs_ubundle [Out \<mapsto> medH bst In f (Y n)])"
+        using f10 by auto
+      then have "UBundle.ubDom\<cdot> (Abs_ubundle [Out \<mapsto> medH bst In f (Y (nn (\<lambda>n. medH bst In f (Y n)) (\<lambda>n. Abs_ubundle [Out \<mapsto> medH bst In f (Y n)] . Out)))]) = UBundle.ubDom\<cdot> (\<Squnion>n. Abs_ubundle [Out \<mapsto> medH bst In f (Y n)])"
+        using f8 by meson
+      then have "[Out \<mapsto> medH bst In f (Y (nn (\<lambda>n. medH bst In f (Y n)) (\<lambda>n. Abs_ubundle [Out \<mapsto> medH bst In f (Y n)] . Out)))] Out = Some (Abs_ubundle [Out \<mapsto> medH bst In f (Y (nn (\<lambda>n. medH bst In f (Y n)) (\<lambda>n. Abs_ubundle [Out \<mapsto> medH bst In f (Y n)] . Out)))] . Out)"
+        using f8 f7 ubdom_insert ubgetchE by fastforce
+      then have "Abs_ubundle [Out \<mapsto> medH bst In f (Y (nn (\<lambda>n. medH bst In f (Y n)) (\<lambda>n. Abs_ubundle [Out \<mapsto> medH bst In f (Y n)] . Out)))] . Out = medH bst In f (Y (nn (\<lambda>n. medH bst In f (Y n)) (\<lambda>n. Abs_ubundle [Out \<mapsto> medH bst In f (Y n)] . Out)))"
+        by force
+      then have "(\<Squnion>n. Abs_ubundle [Out \<mapsto> medH bst In f (Y n)] . Out) = (\<Squnion>n. medH bst In f (Y n))"
+        using f5 by meson
+      then have "ubWell [Out \<mapsto> (Rep_ubundle (\<Squnion>n. Abs_ubundle [Out \<mapsto> medH bst In f (Y n)]))\<rightharpoonup>Out] \<longrightarrow> [Out \<mapsto> (Rep_ubundle (\<Squnion>n. Abs_ubundle [Out \<mapsto> medH bst In f (Y n)]))\<rightharpoonup>Out] c = Some (Abs_ubundle [Out \<mapsto> \<Squnion>n. medH bst In f (Y n)] . c)"
+        using f11 f4 a3 by (metis (no_types) contlub_cfun_arg ubgetchE ubgetch_insert)
+      then have f12: "ubWell [Out \<mapsto> (Rep_ubundle (\<Squnion>n. Abs_ubundle [Out \<mapsto> medH bst In f (Y n)]))\<rightharpoonup>Out] \<longrightarrow> c = Out \<and> (((Rep_ubundle (\<Squnion>n. Abs_ubundle [Out \<mapsto> medH bst In f (Y n)]))\<rightharpoonup>Out) = ((Rep_ubundle (Abs_ubundle [Out \<mapsto> \<Squnion>n. medH bst In f (Y n)]))\<rightharpoonup>c)) \<or> c \<noteq> Out \<and> (None = Some ((Rep_ubundle (Abs_ubundle [Out \<mapsto> \<Squnion>n. medH bst In f (Y n)]))\<rightharpoonup>c))"
+        using map_upd_Some_unfold ubgetch_insert by fastforce
+      then have f13: "ubWell [Out \<mapsto> (Rep_ubundle (\<Squnion>n. Abs_ubundle [Out \<mapsto> medH bst In f (Y n)]))\<rightharpoonup>Out] \<longrightarrow> Abs_ubundle [Out \<mapsto> \<Squnion>n. medH bst In f (Y n)] . c = (\<Squnion>n. Abs_ubundle [Out \<mapsto> medH bst In f (Y n)]) . Out"
+        by (metis (no_types) option.simps(3) ubgetch_insert)
+      have f14: "Rep_ubundle (Abs_ubundle [Out \<mapsto> medH bst In f (Y (v2_4 (\<lambda>n. UBundle.ubDom\<cdot> (Abs_ubundle [Out \<mapsto> medH bst In f (Y n)])) (\<lambda>n. UBundle.ubDom\<cdot>(Y n))))]) = [Out \<mapsto> medH bst In f (Y (v2_4 (\<lambda>n. UBundle.ubDom\<cdot> (Abs_ubundle [Out \<mapsto> medH bst In f (Y n)])) (\<lambda>n. UBundle.ubDom\<cdot>(Y n))))]"
+        using f6 by (simp add: assms to_medh)
+      have "dom [Out \<mapsto> medH bst In f (Y (v2_4 (\<lambda>n. UBundle.ubDom\<cdot> (Abs_ubundle [Out \<mapsto> medH bst In f (Y n)])) (\<lambda>n. UBundle.ubDom\<cdot>(Y n))))] = insert Out (dom (Map.empty::channel \<Rightarrow> 'a MABP tstream option))"
+        by force
+      then have "Out \<in> UBundle.ubDom\<cdot> (\<Squnion>n. Abs_ubundle [Out \<mapsto> medH bst In f (Y n)])"
+        using f14 f11 f8 by (metis (no_types) dom_empty singletonI ubdom_insert)
+      then show "Abs_ubundle [Out \<mapsto> \<Squnion>n. medH bst In f (Y n)] . c \<sqsubseteq> (\<Squnion>n. Abs_ubundle [Out \<mapsto> medH bst In f (Y n)]) . c"
+        using f13 f12 by (simp add: ubWell_single_channel)
+    qed
+
+  show ?thesis
+    apply (rule contI2)
+    apply (simp add: assms ub_below)
+    apply (simp add: med_tsb_getc ubdom_ubrep_eq ubgetch_ubrep_eq)
+    apply (simp add: medh_contlub to_medh)
+    proof -
+      have f1: "\<forall>u ua. (u::'a MABP tstream\<^sup>\<Omega>) \<notsqsubseteq> ua \<or> Some u \<sqsubseteq> Some ua"
+        using some_below by blast
+      have f2: "\<forall>fa. (\<not> chain fa \<or> UBundle.ubDom\<cdot>(Lub fa) \<noteq> {In}) \<or> Abs_ubundle [Out \<mapsto> tsMap f\<cdot> (tsMed\<cdot>(tsMap (inv f)\<cdot>(Lub fa . In))\<cdot> bst)] \<sqsubseteq> (\<Squnion>n. Abs_ubundle [Out \<mapsto> tsMap f\<cdot> (tsMed\<cdot>(tsMap (inv f)\<cdot>(fa n . In))\<cdot>bst)])"
+        using g2 by blast
+      obtain nn :: "(nat \<Rightarrow> ('a MABP tstream\<^sup>\<Omega>) option) \<Rightarrow> (nat \<Rightarrow> ('a MABP tstream\<^sup>\<Omega>) option) \<Rightarrow> nat" where
+        f3: "\<forall>f fa. f (nn fa f) \<noteq> fa (nn fa f) \<or> Lub f = Lub fa"
+        by (meson lub_eq)
+      have "Some (Abs_ubundle [Out \<mapsto> medH bst In f (v0_0 (nn (\<lambda>n. Some (Abs_ubundle [Out \<mapsto> tsMap f\<cdot> (tsMed\<cdot>(tsMap (inv f)\<cdot>(v0_0 n . In))\<cdot> bst)])) (\<lambda>n. Some (Abs_ubundle [Out \<mapsto> medH bst In f (v0_0 n)]))))]) = Some (Abs_ubundle [Out \<mapsto> tsMap f\<cdot> (tsMed\<cdot> (tsMap (inv f)\<cdot> (v0_0 (nn (\<lambda>n. Some (Abs_ubundle [Out \<mapsto> tsMap f\<cdot> (tsMed\<cdot> (tsMap (inv f)\<cdot>(v0_0 n . In))\<cdot> bst)])) (\<lambda>n. Some (Abs_ubundle [Out \<mapsto> medH bst In f (v0_0 n)]))) . In))\<cdot> bst)])"
+        by (simp add: to_medh)
+      then have f4: "(\<Squnion>n. Some (Abs_ubundle [Out \<mapsto> medH bst In f (v0_0 n)])) = (\<Squnion>n. Some (Abs_ubundle [Out \<mapsto> tsMap f\<cdot> (tsMed\<cdot>(tsMap (inv f)\<cdot>(v0_0 n . In))\<cdot>bst)]))"
+        using f3 by meson
+      have f5: "\<forall>f. \<not> chain f \<or> (\<Squnion>n. Some (f n::'a MABP tstream\<^sup>\<Omega>)) = Some (Lub f)"
+        using some_lub_chain_eq3 by blast
+      have f6: "\<forall>c f u ca ua s. ((ctype c::'a MABP set) \<noteq> range f \<or> UBundle.ubDom\<cdot>u \<noteq> {ca} \<or> u \<notsqsubseteq> ua) \<or> Abs_ubundle [c \<mapsto> tsMap f\<cdot> (tsMed\<cdot>(tsMap (inv f)\<cdot>(u . ca)::'b tstream)\<cdot> s)] \<sqsubseteq> Abs_ubundle [c \<mapsto> tsMap f\<cdot>(tsMed\<cdot>(tsMap (inv f)\<cdot>(ua . ca))\<cdot>s)]"
+        by (metis (no_types) med_tsb_mono)
+      obtain nna :: "(nat \<Rightarrow> 'a MABP tstream\<^sup>\<Omega>) \<Rightarrow> nat" where
+        f7: "\<forall>f. (\<not> chain f \<or> (\<forall>n. f n \<sqsubseteq> f (Suc n))) \<and> (chain f \<or> f (nna f) \<notsqsubseteq> f (Suc (nna f)))"
+        using po_class.chain_def by moura
+      then have f8: "(\<not> chain (\<lambda>n. Abs_ubundle [Out \<mapsto> tsMap f\<cdot> (tsMed\<cdot>(tsMap (inv f)\<cdot>(v0_0 n . In))\<cdot> bst)]) \<or> (\<forall>n. Abs_ubundle [Out \<mapsto> tsMap f\<cdot> (tsMed\<cdot>(tsMap (inv f)\<cdot>(v0_0 n . In))\<cdot> bst)] \<sqsubseteq> Abs_ubundle [Out \<mapsto> tsMap f\<cdot> (tsMed\<cdot>(tsMap (inv f)\<cdot>(v0_0 (Suc n) . In))\<cdot> bst)])) \<and> (chain (\<lambda>n. Abs_ubundle [Out \<mapsto> tsMap f\<cdot> (tsMed\<cdot>(tsMap (inv f)\<cdot>(v0_0 n . In))\<cdot> bst)]) \<or> Abs_ubundle [Out \<mapsto> tsMap f\<cdot> (tsMed\<cdot> (tsMap (inv f)\<cdot> (v0_0 (nna (\<lambda>n. Abs_ubundle [Out \<mapsto> tsMap f\<cdot> (tsMed\<cdot>(tsMap (inv f)\<cdot>(v0_0 n . In))\<cdot> bst)])) . In))\<cdot> bst)] \<notsqsubseteq> Abs_ubundle [Out \<mapsto> tsMap f\<cdot> (tsMed\<cdot> (tsMap (inv f)\<cdot> (v0_0 (Suc (nna (\<lambda>n. Abs_ubundle [Out \<mapsto> tsMap f\<cdot> (tsMed\<cdot> (tsMap (inv f)\<cdot>(v0_0 n . In))\<cdot> bst)]))) . In))\<cdot> bst)])"
+        by auto
+      { assume "Some (Abs_ubundle [Out \<mapsto> \<Squnion>n. medH bst In f (v0_0 n)]) \<notsqsubseteq> (\<Squnion>n. Some (Abs_ubundle [Out \<mapsto> medH bst In f (v0_0 n)]))"
+        { assume "(Some (Abs_ubundle [Out \<mapsto> \<Squnion>n. medH bst In f (v0_0 n)]) \<sqsubseteq> (\<Squnion>n. Some (Abs_ubundle [Out \<mapsto> medH bst In f (v0_0 n)]))) \<noteq> (Some (Abs_ubundle [Out \<mapsto> tsMap f\<cdot> (tsMed\<cdot>(tsMap (inv f)\<cdot>(Lub v0_0 . In))\<cdot> bst)]) \<sqsubseteq> Some (\<Squnion>n. Abs_ubundle [Out \<mapsto> tsMap f\<cdot> (tsMed\<cdot>(tsMap (inv f)\<cdot>(v0_0 n . In))\<cdot>bst)]))"
+        then have "(\<Squnion>n. Some (Abs_ubundle [Out \<mapsto> medH bst In f (v0_0 n)])) \<noteq> Some (\<Squnion>n. Abs_ubundle [Out \<mapsto> tsMap f\<cdot> (tsMed\<cdot>(tsMap (inv f)\<cdot>(v0_0 n . In))\<cdot>bst)]) \<or> (\<Squnion>n. medH bst In f (v0_0 n)) \<noteq> tsMap f\<cdot> (tsMed\<cdot>(tsMap (inv f)\<cdot>(Lub v0_0 . In))\<cdot>bst)"
+          by auto
+        moreover
+          { assume "(\<Squnion>n. medH bst In f (v0_0 n)) \<noteq> tsMap f\<cdot> (tsMed\<cdot>(tsMap (inv f)\<cdot>(Lub v0_0 . In))\<cdot>bst)"
+          then have "(UBundle.ubDom\<cdot>(Lub v0_0) \<noteq> {In} \<or> \<not> chain v0_0) \<or> Some (Abs_ubundle [Out \<mapsto> \<Squnion>n. medH bst In f (v0_0 n)]) \<sqsubseteq> (\<Squnion>n. Some (Abs_ubundle [Out \<mapsto> medH bst In f (v0_0 n)]))"
+            by (metis (no_types) cont2contlubE medh_cont to_medh)
+          }
+        ultimately have "(UBundle.ubDom\<cdot>(Lub v0_0) \<noteq> {In} \<or> \<not> chain v0_0) \<or> Some (Abs_ubundle [Out \<mapsto> \<Squnion>n. medH bst In f (v0_0 n)]) \<sqsubseteq> (\<Squnion>n. Some (Abs_ubundle [Out \<mapsto> medH bst In f (v0_0 n)]))"
+          using f8 f7 f6 f5 f4 assms by force
+        }
+        then have "(UBundle.ubDom\<cdot>(Lub v0_0) \<noteq> {In} \<or> \<not> chain v0_0) \<or> Some (Abs_ubundle [Out \<mapsto> \<Squnion>n. medH bst In f (v0_0 n)]) \<sqsubseteq> (\<Squnion>n. Some (Abs_ubundle [Out \<mapsto> medH bst In f (v0_0 n)]))"
+          using f2 f1 by meson
+      }
+      then have f9: "(UBundle.ubDom\<cdot>(Lub v0_0) \<noteq> {In} \<or> \<not> chain v0_0) \<or> Some (Abs_ubundle [Out \<mapsto> \<Squnion>n. medH bst In f (v0_0 n)]) \<sqsubseteq> (\<Squnion>n. Some (Abs_ubundle [Out \<mapsto> medH bst In f (v0_0 n)]))"
+        by meson
+      obtain uu :: "nat \<Rightarrow> 'a MABP tstream\<^sup>\<Omega>" where
+        "(\<exists>v0. (UBundle.ubDom\<cdot>(Lub v0) = {In} \<and> chain v0) \<and> Some (Abs_ubundle [Out \<mapsto> \<Squnion>uua. medH bst In f (v0 uua)]) \<notsqsubseteq> (\<Squnion>uua. Some (Abs_ubundle [Out \<mapsto> medH bst In f (v0 uua)]))) = ((UBundle.ubDom\<cdot>(Lub uu) = {In} \<and> chain uu) \<and> Some (Abs_ubundle [Out \<mapsto> \<Squnion>uua. medH bst In f (uu uua)]) \<notsqsubseteq> (\<Squnion>uua. Some (Abs_ubundle [Out \<mapsto> medH bst In f (uu uua)])))"
+        by (metis (no_types))
+      then show "\<forall>fa. UBundle.ubDom\<cdot>(Lub fa) = {In} \<longrightarrow> chain fa \<longrightarrow> Some (Abs_ubundle [Out \<mapsto> \<Squnion>n. medH bst In f (fa n)]) \<sqsubseteq> (\<Squnion>n. Some (Abs_ubundle [Out \<mapsto> medH bst In f (fa n)]))"
+        proof -
+          obtain nnb :: "(nat \<Rightarrow> ('a MABP tstream\<^sup>\<Omega>) option) \<Rightarrow> (nat \<Rightarrow> ('a MABP tstream\<^sup>\<Omega>) option) \<Rightarrow> nat" where
+            f1: "\<forall>f fa. f (nnb fa f) \<noteq> fa (nnb fa f) \<or> Lub f = Lub fa"
+            by (meson lub_eq)
+          have "Some (Abs_ubundle [Out \<mapsto> medH bst In f (v0_0a (nnb (\<lambda>n. Some (Abs_ubundle [Out \<mapsto> tsMap f\<cdot> (tsMed\<cdot> (tsMap (inv f)\<cdot>(v0_0a n . In))\<cdot> bst)])) (\<lambda>n. Some (Abs_ubundle [Out \<mapsto> medH bst In f (v0_0a n)]))))]) = Some (Abs_ubundle [Out \<mapsto> tsMap f\<cdot> (tsMed\<cdot> (tsMap (inv f)\<cdot> (v0_0a (nnb (\<lambda>n. Some (Abs_ubundle [Out \<mapsto> tsMap f\<cdot> (tsMed\<cdot> (tsMap (inv f)\<cdot>(v0_0a n . In))\<cdot> bst)])) (\<lambda>n. Some (Abs_ubundle [Out \<mapsto> medH bst In f (v0_0a n)]))) . In))\<cdot> bst)])"
+            by (simp add: to_medh)
+          then have f2: "(\<Squnion>n. Some (Abs_ubundle [Out \<mapsto> medH bst In f (v0_0a n)])) = (\<Squnion>n. Some (Abs_ubundle [Out \<mapsto> tsMap f\<cdot> (tsMed\<cdot>(tsMap (inv f)\<cdot>(v0_0a n . In))\<cdot>bst)]))"
+            using f1 by meson
+          have f3: "\<forall>c f u ca ua s. (ctype c::'a MABP set) \<noteq> range f \<or> UBundle.ubDom\<cdot>u \<noteq> {ca} \<or> u \<notsqsubseteq> ua \<or> Abs_ubundle [c \<mapsto> tsMap f\<cdot> (tsMed\<cdot>(tsMap (inv f)\<cdot>(u . ca)::'b tstream)\<cdot> s)] \<sqsubseteq> Abs_ubundle [c \<mapsto> tsMap f\<cdot>(tsMed\<cdot>(tsMap (inv f)\<cdot>(ua . ca))\<cdot>s)]"
+            using med_tsb_mono by blast
+          obtain nnc :: "(nat \<Rightarrow> 'a MABP tstream\<^sup>\<Omega>) \<Rightarrow> nat" where
+            f4: "\<forall>f. (\<not> chain f \<or> (\<forall>n. f n \<sqsubseteq> f (Suc n))) \<and> (chain f \<or> f (nnc f) \<notsqsubseteq> f (Suc (nnc f)))"
+            using po_class.chain_def by moura
+          then have f5: "(\<not> chain (\<lambda>n. Abs_ubundle [Out \<mapsto> tsMap f\<cdot> (tsMed\<cdot>(tsMap (inv f)\<cdot>(v0_0a n . In))\<cdot> bst)]) \<or> (\<forall>n. Abs_ubundle [Out \<mapsto> tsMap f\<cdot> (tsMed\<cdot>(tsMap (inv f)\<cdot>(v0_0a n . In))\<cdot> bst)] \<sqsubseteq> Abs_ubundle [Out \<mapsto> tsMap f\<cdot> (tsMed\<cdot>(tsMap (inv f)\<cdot>(v0_0a (Suc n) . In))\<cdot> bst)])) \<and> (chain (\<lambda>n. Abs_ubundle [Out \<mapsto> tsMap f\<cdot> (tsMed\<cdot>(tsMap (inv f)\<cdot>(v0_0a n . In))\<cdot> bst)]) \<or> Abs_ubundle [Out \<mapsto> tsMap f\<cdot> (tsMed\<cdot> (tsMap (inv f)\<cdot> (v0_0a (nnc (\<lambda>n. Abs_ubundle [Out \<mapsto> tsMap f\<cdot> (tsMed\<cdot>(tsMap (inv f)\<cdot>(v0_0a n . In))\<cdot> bst)])) . In))\<cdot> bst)] \<notsqsubseteq> Abs_ubundle [Out \<mapsto> tsMap f\<cdot> (tsMed\<cdot> (tsMap (inv f)\<cdot> (v0_0a (Suc (nnc (\<lambda>n. Abs_ubundle [Out \<mapsto> tsMap f\<cdot> (tsMed\<cdot> (tsMap (inv f)\<cdot>(v0_0a n . In))\<cdot> bst)]))) . In))\<cdot> bst)])"
+            by auto
+          obtain uua :: "nat \<Rightarrow> 'a MABP tstream\<^sup>\<Omega>" where
+            "(\<exists>v0. (UBundle.ubDom\<cdot>(Lub v0) = {In} \<and> chain v0) \<and> Some (Abs_ubundle [Out \<mapsto> \<Squnion>uua. medH bst In f (v0 uua)]) \<notsqsubseteq> (\<Squnion>uua. Some (Abs_ubundle [Out \<mapsto> medH bst In f (v0 uua)]))) = ((UBundle.ubDom\<cdot>(Lub uua) = {In} \<and> chain uua) \<and> Some (Abs_ubundle [Out \<mapsto> \<Squnion>uuaa. medH bst In f (uua uuaa)]) \<notsqsubseteq> (\<Squnion>uuaa. Some (Abs_ubundle [Out \<mapsto> medH bst In f (uua uuaa)])))"
+            by moura
+          moreover
+          { assume "Some (Abs_ubundle [Out \<mapsto> \<Squnion>n. medH bst In f (uua n)]) \<notsqsubseteq> (\<Squnion>n. Some (Abs_ubundle [Out \<mapsto> medH bst In f (uua n)]))"
+            { assume "(Some (Abs_ubundle [Out \<mapsto> \<Squnion>n. medH bst In f (uua n)]) \<sqsubseteq> (\<Squnion>n. Some (Abs_ubundle [Out \<mapsto> medH bst In f (uua n)]))) \<noteq> (Some (Abs_ubundle [Out \<mapsto> tsMap f\<cdot> (tsMed\<cdot>(tsMap (inv f)\<cdot>(Lub uua . In))\<cdot> bst)]) \<sqsubseteq> Some (\<Squnion>n. Abs_ubundle [Out \<mapsto> tsMap f\<cdot> (tsMed\<cdot>(tsMap (inv f)\<cdot>(uua n . In))\<cdot>bst)]))"
+            moreover
+              { assume "(\<Squnion>n. medH bst In f (uua n)) \<noteq> tsMap f\<cdot>(tsMed\<cdot>(tsMap (inv f)\<cdot>(Lub uua . In))\<cdot>bst)"
+              then have "(UBundle.ubDom\<cdot>(Lub uua) \<noteq> {In} \<or> \<not> chain uua) \<or> Some (Abs_ubundle [Out \<mapsto> \<Squnion>n. medH bst In f (uua n)]) \<sqsubseteq> (\<Squnion>n. Some (Abs_ubundle [Out \<mapsto> medH bst In f (uua n)]))"
+                by (metis (no_types) medh_contlub to_medh)
+              }
+              ultimately have "(UBundle.ubDom\<cdot>(Lub uua) \<noteq> {In} \<or> \<not> chain uua) \<or> Some (Abs_ubundle [Out \<mapsto> \<Squnion>n. medH bst In f (uua n)]) \<sqsubseteq> (\<Squnion>n. Some (Abs_ubundle [Out \<mapsto> medH bst In f (uua n)]))"
+                using f5 f4 f3 f2 assms f5 
+                proof -
+                  have f1: "\<forall>f. \<not> chain f \<or> Some (Lub f::'a MABP tstream\<^sup>\<Omega>) = (\<Squnion>n. Some (f n))"
+                    using some_lub_chain_eq by auto
+                  have f2: "\<forall>c f u ca ua s. ((ctype c::'a MABP set) \<noteq> range f \<or> UBundle.ubDom\<cdot>u \<noteq> {ca} \<or> u \<notsqsubseteq> ua) \<or> Abs_ubundle [c \<mapsto> tsMap f\<cdot> (tsMed\<cdot>(tsMap (inv f)\<cdot>(u . ca)::'b tstream)\<cdot> s)] \<sqsubseteq> Abs_ubundle [c \<mapsto> tsMap f\<cdot>(tsMed\<cdot>(tsMap (inv f)\<cdot>(ua . ca))\<cdot>s)]"
+                    by (metis (no_types) med_tsb_mono)
+                  obtain nnd :: "(nat \<Rightarrow> 'a MABP tstream\<^sup>\<Omega>) \<Rightarrow> nat" where
+                    f3: "\<forall>f. (\<not> chain f \<or> (\<forall>n. f n \<sqsubseteq> f (Suc n))) \<and> (chain f \<or> f (nnd f) \<notsqsubseteq> f (Suc (nnd f)))"
+                    using po_class.chain_def by moura
+                  then have f4: "(\<not> chain (\<lambda>n. Abs_ubundle [Out \<mapsto> tsMap f\<cdot> (tsMed\<cdot>(tsMap (inv f)\<cdot>(uua n . In))\<cdot> bst)]) \<or> (\<forall>n. Abs_ubundle [Out \<mapsto> tsMap f\<cdot> (tsMed\<cdot>(tsMap (inv f)\<cdot>(uua n . In))\<cdot> bst)] \<sqsubseteq> Abs_ubundle [Out \<mapsto> tsMap f\<cdot> (tsMed\<cdot>(tsMap (inv f)\<cdot>(uua (Suc n) . In))\<cdot> bst)])) \<and> (chain (\<lambda>n. Abs_ubundle [Out \<mapsto> tsMap f\<cdot> (tsMed\<cdot>(tsMap (inv f)\<cdot>(uua n . In))\<cdot>bst)]) \<or> Abs_ubundle [Out \<mapsto> tsMap f\<cdot> (tsMed\<cdot> (tsMap (inv f)\<cdot> (uua (nnd (\<lambda>n. Abs_ubundle [Out \<mapsto> tsMap f\<cdot> (tsMed\<cdot> (tsMap (inv f)\<cdot>(uua n . In))\<cdot> bst)])) . In))\<cdot> bst)] \<notsqsubseteq> Abs_ubundle [Out \<mapsto> tsMap f\<cdot> (tsMed\<cdot> (tsMap (inv f)\<cdot> (uua (Suc (nnd (\<lambda>n. Abs_ubundle [Out \<mapsto> tsMap f\<cdot> (tsMed\<cdot> (tsMap (inv f)\<cdot>(uua n . In))\<cdot> bst)]))) . In))\<cdot> bst)])"
+                    by meson
+                  obtain nne :: "(nat \<Rightarrow> ('a MABP tstream\<^sup>\<Omega>) option) \<Rightarrow> (nat \<Rightarrow> ('a MABP tstream\<^sup>\<Omega>) option) \<Rightarrow> nat" where
+                    f5: "\<forall>f fa. f (nne fa f) \<noteq> fa (nne fa f) \<or> Lub f = Lub fa"
+                    by (meson lub_eq)
+                  have "Some (Abs_ubundle [Out \<mapsto> medH bst In f (uua (nne (\<lambda>n. Some (Abs_ubundle [Out \<mapsto> tsMap f\<cdot> (tsMed\<cdot> (tsMap (inv f)\<cdot>(uua n . In))\<cdot> bst)])) (\<lambda>n. Some (Abs_ubundle [Out \<mapsto> medH bst In f (uua n)]))))]) = Some (Abs_ubundle [Out \<mapsto> tsMap f\<cdot> (tsMed\<cdot> (tsMap (inv f)\<cdot> (uua (nne (\<lambda>n. Some (Abs_ubundle [Out \<mapsto> tsMap f\<cdot> (tsMed\<cdot> (tsMap (inv f)\<cdot>(uua n . In))\<cdot> bst)])) (\<lambda>n. Some (Abs_ubundle [Out \<mapsto> medH bst In f (uua n)]))) . In))\<cdot> bst)])"
+                    by (simp add: to_medh)
+                  then have f6: "(\<Squnion>n. Some (Abs_ubundle [Out \<mapsto> medH bst In f (uua n)])) = (\<Squnion>n. Some (Abs_ubundle [Out \<mapsto> tsMap f\<cdot> (tsMed\<cdot>(tsMap (inv f)\<cdot>(uua n . In))\<cdot>bst)]))"
+                    using f5 by meson
+                  { assume "Some (Abs_ubundle [Out \<mapsto> tsMap f\<cdot> (tsMed\<cdot>(tsMap (inv f)\<cdot>(Lub uua . In))\<cdot> bst)]) \<sqsubseteq> Some (\<Squnion>n. Abs_ubundle [Out \<mapsto> tsMap f\<cdot> (tsMed\<cdot>(tsMap (inv f)\<cdot>(uua n . In))\<cdot>bst)])"
+                  then have "UBundle.ubDom\<cdot>(Lub uua) \<noteq> {In} \<or> \<not> chain uua \<or> Some (Abs_ubundle [Out \<mapsto> \<Squnion>n. medH bst In f (uua n)]) \<sqsubseteq> (\<Squnion>n. Some (Abs_ubundle [Out \<mapsto> medH bst In f (uua n)]))"
+                    using f6 f4 f3 f2 f1 \<open>(\<Squnion>n::nat. medH (bst::bool stream) (In::channel) (f::'b::countable \<Rightarrow> 'a::countable MABP) ((uua::nat \<Rightarrow> 'a::countable MABP tstream\<^sup>\<Omega>) n)) \<noteq> tsMap f\<cdot> (tsMed\<cdot>(tsMap (inv f)\<cdot>(Lub uua . In))\<cdot> bst) \<Longrightarrow> (UBundle.ubDom\<cdot>(Lub uua) \<noteq> {In} \<or> \<not> chain uua) \<or> Some (Abs_ubundle [Out::channel \<mapsto> \<Squnion>n::nat. medH bst In f (uua n)]) \<sqsubseteq> (\<Squnion>n::nat. Some (Abs_ubundle [Out \<mapsto> medH bst In f (uua n)]))\<close> assms by force
+                  }
+                  then show ?thesis
+                    using \<open>(Some (Abs_ubundle [Out::channel \<mapsto> \<Squnion>n::nat. medH (bst::bool stream) (In::channel) (f::'b::countable \<Rightarrow> 'a::countable MABP) ((uua::nat \<Rightarrow> 'a::countable MABP tstream\<^sup>\<Omega>) n)]) \<sqsubseteq> (\<Squnion>n::nat. Some (Abs_ubundle [Out \<mapsto> medH bst In f (uua n)]))) \<noteq> (Some (Abs_ubundle [Out \<mapsto> tsMap f\<cdot> (tsMed\<cdot>(tsMap (inv f)\<cdot>(Lub uua . In))\<cdot> bst)]) \<sqsubseteq> Some (\<Squnion>n::nat. Abs_ubundle [Out \<mapsto> tsMap f\<cdot> (tsMed\<cdot>(tsMap (inv f)\<cdot>(uua n . In))\<cdot>bst)]))\<close> by linarith
+                qed
+            }
+            then have "(UBundle.ubDom\<cdot>(Lub uua) \<noteq> {In} \<or> \<not> chain uua) \<or> Some (Abs_ubundle [Out \<mapsto> \<Squnion>n. medH bst In f (uua n)]) \<sqsubseteq> (\<Squnion>n. Some (Abs_ubundle [Out \<mapsto> medH bst In f (uua n)]))"
+              using g2 some_below by blast
+          }
+          ultimately show ?thesis
+            by blast
+        qed
+    qed
 qed
 
 
   subsubsection \<open>tspf_well\<close>
-  
  (* show that the mediumRSTSPF template  fulfills the tickcount property *)
-lemma medrs_tick: assumes "ubclDom\<cdot>b = {c_ar}" and "(ubLen b) = n" and "#bst=\<infinity>"
-  shows "n \<le> (ubclLen (Abs_ubundle([c_as \<mapsto> (tsMap::(bool \<Rightarrow> 'a MABP) \<Rightarrow> bool tstream \<rightarrow> 'a MABP tstream) Bool\<cdot>(tsMed\<cdot>(tsMap invBool\<cdot>(b  .  c_ar))\<cdot>bst)])))"
+lemma med_tick: assumes "ubDom\<cdot>b = {In}" and "(ubLen b) = n" and "#bst=\<infinity>" and "(ctype::channel \<Rightarrow> 'a MABP set) Out = range f"
+  shows "n \<le> (ubclLen (Abs_ubundle([Out \<mapsto> (tsMap f\<cdot>(tsMed\<cdot>(tsMap (inv f)\<cdot>((b . In):: 'a MABP tstream))\<cdot>bst):: 'a MABP tstream)])))"
 proof -
-  have "(ubLen b) = usclLen\<cdot>(b . c_ar)"
+  have "(ubLen b) = usclLen\<cdot>(b . In)"
     apply (rule uslen_ubLen_ch3)
     by (metis assms(1) ubclDom_ubundle_def)
-  hence f1: "n = usclLen\<cdot>(b . c_ar)"
+  hence f1: "n = usclLen\<cdot>(b . In)"
     using assms(2) by blast
-  hence f2: "n \<le> usclLen\<cdot>((tsMap::(bool \<Rightarrow> 'a MABP) \<Rightarrow> bool tstream \<rightarrow> 'a MABP tstream) Bool\<cdot>(tsMed\<cdot>(tsMap invBool\<cdot>(b  .  c_ar))\<cdot>bst))"
+  hence f2: "n \<le> usclLen\<cdot>(tsMap f\<cdot>(tsMed\<cdot>(tsMap (inv f)\<cdot>(b  .  In))\<cdot>bst))"
     by (simp add: assms(3) usclLen_tstream_def)
   show ?thesis
     apply (simp add: ubclLen_ubundle_def)
     apply (rule ubLen_geI)
-    apply (simp add: medrs_tsb_dom ubgetch_ubrep_eq)
-    by (simp add: f2 ubdom_ubrep_eq)
+    apply (simp add: assms med_tsb_dom ubgetch_ubrep_eq)
+    by (simp add: assms f2 ubdom_ubrep_eq)
 qed
-  
-      
-    
+
+
+
   (* a medium is a tspf if the oracle bool stream bst is infinitly long*)
-lemma medrs_well [simp]: assumes "#bst=\<infinity>"
-  shows "ufWell (\<Lambda> (x::'a MABP tstream\<^sup>\<Omega>). (ubclDom\<cdot>x = {c_ar})
-                           \<leadsto> Abs_ubundle([c_as \<mapsto> (tsMap::(bool \<Rightarrow> 'a MABP) \<Rightarrow> bool tstream \<rightarrow> 'a MABP tstream)
-                                Bool\<cdot>(tsMed\<cdot>(tsMap invBool\<cdot>(x . c_ar))\<cdot>bst)]))"
+lemma med_well [simp]: assumes "#bst=\<infinity>" and "(ctype::channel \<Rightarrow> 'a MABP set) Out = range f"
+  shows "ufWell (\<Lambda> (x::'a MABP tstream\<^sup>\<Omega>). (ubDom\<cdot>x = {In})
+                           \<leadsto> Abs_ubundle([Out \<mapsto> (tsMap
+                                f\<cdot>(tsMed\<cdot>(tsMap (inv f)\<cdot>((x . In):: 'a MABP tstream))\<cdot>bst):: 'a MABP tstream)]))"
   apply (rule ufun_wellI)
-    apply (simp_all add: domIff2)
-  by (simp add:  ubclDom_ubundle_def ubDom_def)
+  apply (simp_all add: domIff2 assms)
+  by  (simp_all add: med_tsb_dom assms ubclDom_ubundle_def)
 
-      
-lemma medrs_revsubst: "Abs_cufun (tsMedRSAbb bst) = (medRS_TSPF bst)"
-  by (simp add: medRS_TSPF_def)
-    
-lemma medrs_tspfdom: assumes "#bst =\<infinity>"
-  shows "ufDom\<cdot>(medRS_TSPF bst) = {c_ar}"
-    apply (simp add: medRS_TSPF_def)
-    apply (simp add: ufdom_insert assms)
-    apply (simp add: domIff2)
-  by (simp add: ubclDom_h)
-   
-lemma medrs_tspfran: assumes "#bst =\<infinity>"
-  shows "ufRan\<cdot>(medRS_TSPF bst) = {c_as}"   
-    apply (simp add: medRS_TSPF_def)
-    apply (simp add: ufran_least medrs_tspfdom assms)
-    apply (simp add: medrs_revsubst medrs_tspfdom assms)
-  by (simp add: medrs_tsb_dom ubcldom_least_cs)
 
+lemma med_revsubst: "Abs_cufun (tsMedAbb bst In Out f) = (med_TSPF bst In Out f)"
+  by (simp add: med_TSPF_def)
+
+
+lemma med_tspfdom: assumes "#bst =\<infinity>" and "(ctype::channel \<Rightarrow> 'a MABP set) Out = range f"
+  shows "ufDom\<cdot>((med_TSPF :: bool stream \<Rightarrow> channel \<Rightarrow> channel \<Rightarrow> ('b \<Rightarrow> 'a MABP) \<Rightarrow> ('a MABP tstream\<^sup>\<Omega>)ufun) bst In Out f) = {In}"
+  apply (simp add: med_TSPF_def)
+  apply (simp add: ufdom_insert)
+  apply (simp_all add: assms)
+  apply (simp add: domIff)
+  by (metis ubclDom_h ubclDom_ubundle_def)
+
+
+lemma med_tspfran: assumes "#bst =\<infinity>" and "(ctype::channel \<Rightarrow> 'a MABP set) Out = range f"
+  shows "ufRan\<cdot>((med_TSPF :: bool stream \<Rightarrow> channel \<Rightarrow> channel \<Rightarrow> ('b \<Rightarrow> 'a MABP) \<Rightarrow> ('a MABP tstream\<^sup>\<Omega>)ufun) bst In Out f) = {Out}"
+  apply (simp add: med_TSPF_def)
+  apply (simp add: ufran_least med_tspfdom assms)
+  apply (simp add: med_revsubst med_tspfdom assms)
+  by (metis assms(2) med_tsb_dom ubclDom_ubundle_def ubcldom_least_cs)
 
   (* now special lemmata for TSPS instantiation *)
 
-lemma medrs_well2 [simp]: assumes "#({True} \<ominus> bst) = \<infinity>"
-  shows "ufWell (\<Lambda> (x::'a MABP tstream\<^sup>\<Omega>). (ubclDom\<cdot>x = {c_ar})
-                           \<leadsto> Abs_ubundle([c_as \<mapsto> (tsMap::(bool \<Rightarrow> 'a MABP) \<Rightarrow> bool tstream \<rightarrow> 'a MABP tstream)
-                                Bool\<cdot>(tsMed\<cdot>(tsMap invBool\<cdot>(x . c_ar))\<cdot>bst)]))"
-proof -
-   have "#bst = \<infinity>"
-     by (simp add: med_ora_length assms(1))
-   thus ?thesis  
-     by (simp add: medrs_tspfdom)
-qed
-  
-
-lemma medrs_tspfdom2: assumes "#({True} \<ominus> bst) = \<infinity>"
-  shows "ufclDom\<cdot>(medRS_TSPF bst) = {c_ar}"
-proof -
-  have "#bst = \<infinity>"
-    by (simp add: med_ora_length assms(1))
-  thus ?thesis
-    by (simp add: medrs_tspfdom ufclDom_ufun_def)
-qed
-  
-lemma medrs_tspfran2: assumes "#({True} \<ominus> bst) = \<infinity>"
-  shows "ufRan\<cdot>(medRS_TSPF bst) = {c_as}"
-proof -
-  have "#bst = \<infinity>"
-    by (simp add: med_ora_length assms(1))
-  thus ?thesis
-    by (simp add: medrs_tspfran)
-qed
-
-  (* necessary for TSPS instantiation *)
-lemma medrs_tsps_dom1 [simp]: "f = medRS_TSPF ora \<and> #({True} \<ominus> ora) = \<infinity> \<Longrightarrow> ufDom\<cdot>f = {c_ar}"
-  by (metis medrs_tspfdom2 ufclDom_ufun_def)
-
-lemma medrs_tsps_dom2 [simp]: "\<exists>ora::bool stream. f = medRS_TSPF ora \<and> #({True} \<ominus> ora) = \<infinity> 
-                               \<Longrightarrow> ufDom\<cdot>f = {c_ar}"
-  using medrs_tsps_dom1  by auto
- 
-lemma medrs_tsps_ran1 [simp]: "f = medRS_TSPF ora \<and> #({True} \<ominus> ora) = \<infinity> \<Longrightarrow> ufRan\<cdot>f = {c_as}"
-  by (simp add: medrs_tspfran2)
-
-lemma medrs_tsps_ran2 [simp]: "\<exists>ora::bool stream. f = medRS_TSPF ora \<and> #({True} \<ominus> ora) = \<infinity> 
-                               \<Longrightarrow> ufRan\<cdot>f = {c_as}"
-  using medrs_tsps_ran1 by auto
-
-
-      
-  subsection \<open>medium_sr\<close>     
-
-subsubsection \<open>defs\<close>
-
-definition medSRH :: "bool stream \<Rightarrow> 'a MABP tstream\<^sup>\<Omega> \<Rightarrow> 'a MABP tstream"  where
-"medSRH bst \<equiv> (\<lambda> x. (tsMap:: ('a \<times> bool \<Rightarrow> 'a MABP) \<Rightarrow> ('a \<times> bool) tstream \<rightarrow> 'a MABP tstream) 
-            BoolPair\<cdot>(tsMed\<cdot>(tsMap invBoolPair\<cdot>(x . c_ds))\<cdot>bst))"
-
-lemma medsrh_cont [simp]: "cont (medSRH bst)"
-  by (simp add: medSRH_def)
-
-lemma medsrh_contlub: assumes "chain Y"
-  shows "(medSRH bst) ((\<Squnion>i. Y i)) = (\<Squnion>i. ((medSRH bst) ((Y i))))"
-  apply (rule cont2contlubE)
-  by (simp_all add: assms)
-
-lemma to_medsrh: "tsMap BoolPair\<cdot>(tsMed\<cdot>(tsMap invBoolPair\<cdot>(x  .  c_ds))\<cdot>bst)
-                  = ((medSRH :: bool stream \<Rightarrow> 'a MABP tstream\<^sup>\<Omega> \<Rightarrow> 'a MABP tstream) bst) x"
-  by (simp add: medSRH_def)
-
-subsubsection \<open>pre\<close>
-(*
-lemma tsmed_input_cont [simp]: "cont (\<lambda> x. tsMed\<cdot>x\<cdot>bst)"
-  by simp
-
-lemma tsmed_input_mono [simp]: "monofun (\<lambda> x. tsMed\<cdot>x\<cdot>bst)"
-  using cont2mono tsmed_input_cont by blast
-*)
-
-lemma medsr_tsb_well[simp]: "ubWell [c_dr \<mapsto> tsMap BoolPair\<cdot>(tsMed\<cdot>(tsMap invBoolPair\<cdot>(x . c_ds))\<cdot>bst)]"
-  apply (rule ubwellI)
-  apply (simp add: usclOkay_tstream_def)
-  by (simp add: tsmap_tsdom_range)
-
-lemma medsr_tsb_dom: "ubDom\<cdot>(Abs_ubundle [c_dr \<mapsto> tsMap BoolPair\<cdot>(tsMed\<cdot>(tsMap invBoolPair\<cdot>(x . c_ds))\<cdot>bst)]) = {c_dr}"
-  by (simp add: ubdom_ubrep_eq)
-    
-  subsubsection \<open>cont\<close>
-    
-(* definition tsMedSRTSPF :: "bool stream \<Rightarrow> 'a MABP TSPF" where
-"tsMedSRTSPF bst\<equiv> Abs_CTSPF (\<lambda> x. (tsbDom\<cdot>x = {c_ds})
-  \<leadsto> [c_dr \<mapsto> (tsMap:: ('a \<times> bool \<Rightarrow> 'a MABP) \<Rightarrow> ('a \<times> bool) tstream \<rightarrow> 'a MABP tstream) 
-            BoolPair\<cdot>(tsMed\<cdot>(tsMap invBoolPair\<cdot>(x . c_ds))\<cdot>bst)]\<Omega>)" *)
-
-(* this can be shown analogue to before *)
-lemma medsr_cont [simp]: "cont (\<lambda> x::'a MABP tstream\<^sup>\<Omega>. (tsbDom\<cdot>x = {c_ds})
-  \<leadsto> Abs_ubundle [c_dr \<mapsto> (tsMap:: ('a \<times> bool \<Rightarrow> 'a MABP) \<Rightarrow> ('a \<times> bool) tstream \<rightarrow> 'a MABP tstream) 
-            BoolPair\<cdot>(tsMed\<cdot>(tsMap invBoolPair\<cdot>(x . c_ds))\<cdot>bst)])"
-  sorry
-    
- 
-  subsubsection \<open>tspf_well\<close>
-
-lemma medsr_tick: assumes "ubDom\<cdot>b = {c_ds}" and "(ubLen b) = n" and "#bst=\<infinity>"
-  shows "n \<le> (ubLen (Abs_ubundle [c_dr \<mapsto> (tsMap:: ('a \<times> bool \<Rightarrow> 'a MABP) \<Rightarrow> ('a \<times> bool) tstream \<rightarrow> 'a MABP tstream) 
-            BoolPair\<cdot>(tsMed\<cdot>(tsMap invBoolPair\<cdot>(b . c_ds))\<cdot>bst)]))"
-proof -
-  have "(ubLen b) = #\<surd>(b . c_ds)"
-    apply (simp add: ubLen_def assms(1))
-    apply (rule Least_equality)
-    by (simp_all add: usclLen_tstream_def)
-  hence f1: "n = #\<surd>(b . c_ds)"
-    using assms(2) by blast
-  hence f2: "n \<le> #\<surd>((tsMap:: ('a \<times> bool \<Rightarrow> 'a MABP) \<Rightarrow> ('a \<times> bool) tstream \<rightarrow> 'a MABP tstream) 
-            BoolPair\<cdot>(tsMed\<cdot>(tsMap invBoolPair\<cdot>(b . c_ds))\<cdot>bst))"
-    by (simp add: assms(3))
-  show ?thesis
-    apply (rule ubLen_geI)
-    apply (simp add: medsr_tsb_dom ubgetch_ubrep_eq)
-    by (metis f2 medsr_tsb_dom singletonD ubclDom_ubundle_def usclLen_tstream_def)
-qed    
-    
-  (* a medium is a tspf if the oracle bool stream bst is infinitly long*)
-lemma medsr_well [simp]: assumes "#bst=\<infinity>"
-  shows "ufWell (\<Lambda> x.(ubDom\<cdot>x = {c_ds})
-  \<leadsto> Abs_ubundle [c_dr \<mapsto> (tsMap:: ('a \<times> bool \<Rightarrow> 'a MABP) \<Rightarrow> ('a \<times> bool) tstream \<rightarrow> 'a MABP tstream) 
-            BoolPair\<cdot>(tsMed\<cdot>(tsMap invBoolPair\<cdot>(x . c_ds))\<cdot>bst)])"
-  apply (rule ufun_wellI)
-  by (simp_all add: domIff2 medsr_tsb_dom ubclDom_ubundle_def)
- 
-lemma medsr_revsubst: "Abs_cufun (medSR_TSPFAbb bst) = (medSR_TSPF bst)"
-  by (simp add: medSR_TSPF_def)
-    
-lemma medsr_tspfdom: assumes "#bst =\<infinity>"
-  shows "ufDom\<cdot>(medSR_TSPF bst) = {c_ds}"
-    apply (simp add: medSR_TSPF_def)
-    apply (simp add: ufdom_insert assms ubclDom_ubundle_def)
-  apply (simp add: domIff2)
-  by (meson tfl_some ubleast_ubdom)
-
-   
-lemma medsr_tspfran: assumes "#bst =\<infinity>"
-  shows "ufRan\<cdot>(medSR_TSPF bst) = {c_dr}"   
-    apply (simp add: medSR_TSPF_def)
-    apply (simp add: ufran_least medsr_tspfdom assms)
-  apply (simp add: medsr_revsubst medsr_tspfdom assms)
-  apply (simp add: ubclDom_ubundle_def)
-  sorry
-
-  (* now special lemmata for TSPS instantiation *)
-
-lemma medsr_well2 [simp]: assumes "#({True} \<ominus> bst) = \<infinity>"
-  shows "ufWell (\<Lambda> x.(ubDom\<cdot>x = {c_ds})
-  \<leadsto> Abs_ubundle [c_dr \<mapsto> (tsMap:: ('a \<times> bool \<Rightarrow> 'a MABP) \<Rightarrow> ('a \<times> bool) tstream \<rightarrow> 'a MABP tstream) 
-            BoolPair\<cdot>(tsMed\<cdot>(tsMap invBoolPair\<cdot>(x . c_ds))\<cdot>bst)])"
+lemma med_well2 [simp]: assumes "#({True} \<ominus> bst) = \<infinity>" and "(ctype::channel \<Rightarrow> 'a MABP set) Out = range f"
+  shows "ufWell (\<Lambda> (x::'a MABP tstream\<^sup>\<Omega>). (ubDom\<cdot>x = {In})
+                           \<leadsto> Abs_ubundle([Out \<mapsto> (tsMap
+                                f\<cdot>(tsMed\<cdot>(tsMap (inv f)\<cdot>((x . In):: 'a MABP tstream))\<cdot>bst):: 'a MABP tstream)]))"
 proof -
    have "#bst = \<infinity>"
      by (simp add: med_ora_length assms(1))
    thus ?thesis
-     by (simp add: medsr_tspfdom)
-qed
-  
+     by (simp add: assms(2))
+ qed
 
-lemma medsr_tspfdom2: assumes "#({True} \<ominus> bst) = \<infinity>"
-  shows "ufDom\<cdot>(medSR_TSPF bst) = {c_ds}"
+
+lemma med_tspfdom2: assumes "#({True} \<ominus> bst) = \<infinity>" and "(ctype::channel \<Rightarrow> 'a MABP set) Out = range f"
+  shows "ufDom\<cdot>((med_TSPF :: bool stream \<Rightarrow> channel \<Rightarrow> channel \<Rightarrow> ('b \<Rightarrow> 'a MABP) \<Rightarrow> ('a MABP tstream\<^sup>\<Omega>)ufun) bst In Out f) = {In}"
 proof -
   have "#bst = \<infinity>"
     by (simp add: med_ora_length assms(1))
   thus ?thesis
-    by (simp add: medsr_tspfdom)
+    by (simp add: assms med_tspfdom)
 qed
-  
-lemma medsr_tspfran2: assumes "#({True} \<ominus> bst) = \<infinity>"
-  shows "ufRan\<cdot>(medSR_TSPF bst) = {c_dr}"
+
+
+lemma med_tspfran2: assumes "#({True} \<ominus> bst) = \<infinity>" and "(ctype::channel \<Rightarrow> 'a MABP set) Out = range f"
+  shows "ufRan\<cdot>((med_TSPF :: bool stream \<Rightarrow> channel \<Rightarrow> channel \<Rightarrow> ('b \<Rightarrow> 'a MABP) \<Rightarrow> ('a MABP tstream\<^sup>\<Omega>)ufun) bst In Out f) = {Out}"
 proof -
   have "#bst = \<infinity>"
     by (simp add: med_ora_length assms(1))
   thus ?thesis
-    by (simp add: medsr_tspfran)
+    by (simp add: assms(2) med_tspfran)
 qed
+
 
   (* necessary for TSPS instantiation *)
-lemma medsr_tsps_dom1 [simp]: "f = medSR_TSPF ora \<and> #({True} \<ominus> ora) = \<infinity> \<Longrightarrow> ufDom\<cdot>f = {c_ds}"
-  by (simp add: medsr_tspfdom2)
+lemma med_tsps_dom1 [simp]: assumes "(ctype::channel \<Rightarrow> 'a MABP set) Out = range f" shows
+  "g = (med_TSPF :: bool stream \<Rightarrow> channel \<Rightarrow> channel \<Rightarrow> ('b \<Rightarrow> 'a MABP) \<Rightarrow> ('a MABP tstream\<^sup>\<Omega>)ufun) ora In Out f \<and> #({True} \<ominus> ora) = \<infinity> \<Longrightarrow> ufDom\<cdot>g = {In}"
+  by (simp add: assms med_tspfdom2)
 
-lemma medsr_tsps_dom2 [simp]: "\<exists>ora::bool stream. f = medSR_TSPF ora \<and> #({True} \<ominus> ora) = \<infinity> 
-                               \<Longrightarrow> ufDom\<cdot>f = {c_ds}"
-  using medsr_tsps_dom1  by auto
- 
-lemma medsr_tsps_ran1 [simp]: "f = medSR_TSPF ora \<and> #({True} \<ominus> ora) = \<infinity> \<Longrightarrow> ufRan\<cdot>f = {c_dr}"
-  by (simp add: medsr_tspfran2)
 
-lemma medsr_tsps_ran2 [simp]: "\<exists>ora::bool stream. f = medSR_TSPF ora \<and> #({True} \<ominus> ora) = \<infinity> 
-                               \<Longrightarrow> ufRan\<cdot>f = {c_dr}"
-  using medsr_tsps_ran1 by auto
-      
+lemma med_tsps_dom2 [simp]: assumes "(ctype::channel \<Rightarrow> 'a MABP set) Out = range f" shows
+  "\<exists>ora::bool stream. g = (med_TSPF :: bool stream \<Rightarrow> channel \<Rightarrow> channel \<Rightarrow> ('b \<Rightarrow> 'a MABP) \<Rightarrow> ('a MABP tstream\<^sup>\<Omega>)ufun) ora In Out f \<and> #({True} \<ominus> ora) = \<infinity> 
+                               \<Longrightarrow> ufDom\<cdot>g = {In}"
+  using assms med_tsps_dom1 by auto
+
+
+lemma med_tsps_ran1 [simp]: assumes "(ctype::channel \<Rightarrow> 'a MABP set) Out = range f" shows
+  "g = (med_TSPF :: bool stream \<Rightarrow> channel \<Rightarrow> channel \<Rightarrow> ('b \<Rightarrow> 'a MABP) \<Rightarrow> ('a MABP tstream\<^sup>\<Omega>)ufun) ora In Out f \<and> #({True} \<ominus> ora) = \<infinity> \<Longrightarrow> ufRan\<cdot>g = {Out}"
+  by (simp add: assms med_tspfran2)
+
+
+lemma med_tsps_ran2 [simp]: assumes "(ctype::channel \<Rightarrow> 'a MABP set) Out = range f" shows
+  "\<exists>ora::bool stream. g = (med_TSPF :: bool stream \<Rightarrow> channel \<Rightarrow> channel \<Rightarrow> ('b \<Rightarrow> 'a MABP) \<Rightarrow> ('a MABP tstream\<^sup>\<Omega>)ufun) ora In Out f \<and> #({True} \<ominus> ora) = \<infinity> 
+                               \<Longrightarrow> ufRan\<cdot>g = {Out}"
+  using assms med_tsps_ran1 by auto
+
+
+lemma med_ufIsWeak: assumes "#bst =\<infinity>" and "(ctype::channel \<Rightarrow> 'a MABP set) Out = range f" shows
+  "ufIsWeak (Abs_ufun(\<Lambda> (x::'a MABP tstream\<^sup>\<Omega>). (ubDom\<cdot>x = {In})
+                           \<leadsto> Abs_ubundle([Out \<mapsto> tsMap
+                                f\<cdot>(tsMed\<cdot>(tsMap (inv f)\<cdot>(x . In))\<cdot>bst)])))"
+  apply (simp add: ufIsWeak_def)
+  apply (simp add: assms domIff)
+  apply (rule, rule)
+  apply (subst med_tick)
+  by (simp_all add: assms ubclLen_ubundle_def)
+
+
+subsection\<open>id\<close>
+
+
+subsubsection\<open>mono/cont\<close>
+
+
+lemma idTSPF_mono: "monofun (\<lambda> x. (ubDom\<cdot>x = {c_abpOut}) \<leadsto> x)"
+  by (simp add: monofunI some_below ubdom_below)
+
+lemma idTSPF_cont: "cont (\<lambda> x. (ubDom\<cdot>x = {c_abpOut}) \<leadsto> x)"
+  apply(rule contI2)
+   apply(simp add: idTSPF_mono)
+  using some_lub_chain_eq by fastforce
+
+
+subsubsection\<open>ufWell/tickCount\<close>
+
+
+lemma idTSPF_well: "ufWell (\<Lambda> x. (ubDom\<cdot>x = {c_abpOut}) \<leadsto> x)"
+  apply(rule ufun_wellI)
+    by (simp_all add: idTSPF_cont domIff2 ubclDom_ubundle_def)
+
+lemma idTSPF_tickCount: "ufIsWeak (Abs_cufun (\<lambda> x. (ubDom\<cdot>x = {c_abpOut}) \<leadsto> x))"
+  apply(simp add: ufIsWeak_def)
+  by (simp add: idTSPF_cont idTSPF_well domIff rep_abs_cufun) 
+
+lemma idTSPF_dom: "ufDom\<cdot>idTSPF = {c_abpOut}"
+  apply(simp add: idTSPF_def)
+  apply (fold ubclDom_ubundle_def)
+  apply (subst ufun_ufdom_abs)
+  by (simp_all add: ubclDom_ubundle_def idTSPF_cont idTSPF_well)
+
+lemma idTSPF_ran: "ufRan\<cdot>idTSPF = {c_abpOut}"
+  apply(simp add: idTSPF_def)
+proof -
+have f1: "\<forall>f. \<not> cont f \<or> \<not> ufWell (Abs_cfun f) \<or> Rep_cufun (Abs_cufun f::('a MABP tstream\<^sup>\<Omega>) ufun) = f"
+  by (metis rep_abs_cufun)
+  then have f2: "Rep_cufun (Abs_cufun (\<lambda>u. (ubDom\<cdot>(u::'a MABP tstream\<^sup>\<Omega>) = {c_abpOut})\<leadsto>u)) = (\<lambda>u. (ubDom\<cdot>u = {c_abpOut})\<leadsto>u)"
+    using idTSPF_cont idTSPF_well by blast
+  have "ubclLeast (ufDom\<cdot> (Abs_cufun (\<lambda>u. (ubDom\<cdot>(u::'a MABP tstream\<^sup>\<Omega>) = {c_abpOut})\<leadsto>u))) \<in> dom (\<lambda>u. (ubDom\<cdot>(u::'a MABP tstream\<^sup>\<Omega>) = {c_abpOut})\<leadsto>u)"
+    using f1 by (metis (no_types) idTSPF_cont idTSPF_well ufunLeastIDom)
+  then have f3: "(ubDom\<cdot> (ubclLeast (ufDom\<cdot> (Abs_cufun (\<lambda>u. (ubDom\<cdot>(u::'a MABP tstream\<^sup>\<Omega>) = {c_abpOut})\<leadsto>u)))::'a MABP tstream\<^sup>\<Omega>) = {c_abpOut})\<leadsto>ubclLeast (ufDom\<cdot> (Abs_cufun (\<lambda>u. (ubDom\<cdot> (u::'a MABP tstream\<^sup>\<Omega>) = {c_abpOut})\<leadsto>u)))::'a MABP tstream\<^sup>\<Omega> \<noteq> None"
+    by blast
+  then have "Rep_cufun (Abs_cufun (\<lambda>u. (ubDom\<cdot>(u::'a MABP tstream\<^sup>\<Omega>) = {c_abpOut})\<leadsto>u)) (ubclLeast (ufDom\<cdot> (Abs_cufun (\<lambda>u. (ubDom\<cdot>(u::'a MABP tstream\<^sup>\<Omega>) = {c_abpOut})\<leadsto>u)))) = Some (ubclLeast (ufDom\<cdot> (Abs_cufun (\<lambda>u. (ubDom\<cdot>(u::'a MABP tstream\<^sup>\<Omega>) = {c_abpOut})\<leadsto>u))))"
+    using f2 by presburger
+  then have "Abs_cufun (\<lambda>u. (ubDom\<cdot>(u::'a MABP tstream\<^sup>\<Omega>) = {c_abpOut})\<leadsto>u) \<rightleftharpoons> ubclLeast (ufDom\<cdot> (Abs_cufun (\<lambda>u. (ubDom\<cdot>(u::'a MABP tstream\<^sup>\<Omega>) = {c_abpOut})\<leadsto>u))) = ubclLeast (ufDom\<cdot> (Abs_cufun (\<lambda>u. (ubDom\<cdot>(u::'a MABP tstream\<^sup>\<Omega>) = {c_abpOut})\<leadsto>u)))"
+    by (metis option.sel)
+  then have f4: "ufRan\<cdot> (Abs_cufun (\<lambda>u. (ubDom\<cdot>(u::'a MABP tstream\<^sup>\<Omega>) = {c_abpOut})\<leadsto>u)) = ubclDom\<cdot> (ubclLeast (ufDom\<cdot> (Abs_cufun (\<lambda>u. (ubDom\<cdot>(u::'a MABP tstream\<^sup>\<Omega>) = {c_abpOut})\<leadsto>u)))::'a MABP tstream\<^sup>\<Omega>)"
+    by (simp add: UFun_Comp.ufran_least)
+  have "Rep_cufun (Abs_cufun (\<lambda>u. (ubDom\<cdot>(u::'a MABP tstream\<^sup>\<Omega>) = {c_abpOut})\<leadsto>u)) (ubclLeast (ufDom\<cdot> (Abs_cufun (\<lambda>u. (ubDom\<cdot>(u::'a MABP tstream\<^sup>\<Omega>) = {c_abpOut})\<leadsto>u)))) = Some (ubclLeast (ufDom\<cdot> (Abs_cufun (\<lambda>u. (ubDom\<cdot>(u::'a MABP tstream\<^sup>\<Omega>) = {c_abpOut})\<leadsto>u))))"
+    using f3 f2 by presburger
+  then have "ufRan\<cdot> (Abs_cufun (\<lambda>u. (ubDom\<cdot>(u::'a MABP tstream\<^sup>\<Omega>) = {c_abpOut})\<leadsto>u)) = ufDom\<cdot> (Abs_cufun (\<lambda>u. (ubDom\<cdot>(u::'a MABP tstream\<^sup>\<Omega>) = {c_abpOut})\<leadsto>u))"
+    using f4 ufdom_2ufundom by blast
+  then show "ufRan\<cdot> (Abs_cufun (\<lambda>u. (ubDom\<cdot>(u::'a MABP tstream\<^sup>\<Omega>) = {c_abpOut})\<leadsto>u)) = {c_abpOut}"
+    by (metis (no_types) idTSPF_dom idTSPF_def)
+qed
+
+subsection\<open>id2\<close>
+
+lemma c_abpOut_idOut_ctype_eq: "\<And> x::('a MABP tstream). usclOkay c_idOut x = usclOkay c_abpOut x"
+  by (simp add: usclOkay_tstream_def)
+
+lemma idTSPF2_result_ubwell:  assumes "ubDom\<cdot>(x::'a MABP tstream\<^sup>\<Omega>) = {c_abpOut}" 
+  shows "ubWell [c_idOut \<mapsto> (x::('a MABP tstream\<^sup>\<Omega>)) . c_abpOut]"
+  apply (rule ubwellI)
+  apply (simp add: domIff)
+  by (simp add: assms c_abpOut_idOut_ctype_eq ubgetch_insert)
+
+lemma idTSPF2_result_dom:  assumes "ubDom\<cdot>(x::'a MABP tstream\<^sup>\<Omega>) = {c_abpOut}" 
+  shows "ubDom\<cdot>(Abs_ubundle [c_idOut \<mapsto> (x::('a MABP tstream\<^sup>\<Omega>)) . c_abpOut]) = {c_idOut}"
+  by (simp add: assms idTSPF2_result_ubwell ubdom_ubrep_eq)
+
+lemma idTSPF2_io_eq: assumes "ubDom\<cdot>(x::'a MABP tstream\<^sup>\<Omega>) = {c_abpOut}"
+  shows "((\<lambda> (x::'a MABP tstream\<^sup>\<Omega>). (ubDom\<cdot>x = {c_abpOut}) \<leadsto> Abs_ubundle [c_idOut \<mapsto> x . c_abpOut])\<rightharpoonup>x) . c_idOut
+    = (x::'a MABP tstream\<^sup>\<Omega>) . c_abpOut"
+  apply simp apply rule
+  apply (simp add: idTSPF2_result_ubwell ubgetch_ubrep_eq)
+  by (simp add: assms)
+
+lemma idTSPF2_result_below: assumes "(x::('a MABP tstream\<^sup>\<Omega>)) \<sqsubseteq> y" 
+  and "ubDom\<cdot>(x::'a MABP tstream\<^sup>\<Omega>) = {c_abpOut}"
+  shows "Abs_ubundle [c_idOut \<mapsto> x . c_abpOut] \<sqsubseteq>  Abs_ubundle [c_idOut \<mapsto> y . c_abpOut]"
+  apply (rule ub_below)
+   apply (subst ubdom_ubrep_eq)
+    apply (simp add: assms(2) idTSPF2_result_ubwell)
+   apply (subst ubdom_ubrep_eq)
+  using assms(1) assms(2) idTSPF2_result_ubwell ubdom_below apply blast
+   apply (simp add: domIff)
+  apply (simp add: assms idTSPF2_result_dom)
+  apply (subst ubgetch_ubrep_eq) 
+    apply (simp add: assms(2) idTSPF2_result_ubwell)
+  apply (subst ubgetch_ubrep_eq) 
+  using assms(1) assms(2) idTSPF2_result_ubwell ubdom_below apply blast
+  by (simp add: assms(1) monofun_cfun_arg)
+
+subsubsection\<open>mono/cont\<close>
+
+lemma idTSPF2_mono: "monofun (\<lambda> (x::('a MABP tstream\<^sup>\<Omega>)). (ubDom\<cdot>x = {c_abpOut}) \<leadsto> Abs_ubundle[c_idOut \<mapsto> x . c_abpOut])"
+  apply (rule monofunI)
+  apply (case_tac "(ubDom\<cdot>x \<noteq> {c_abpOut})")
+   apply (simp add: ubdom_below)
+  apply (simp) apply (rule, rule)
+   apply (rule some_below)
+   apply (rule ub_below)
+    apply (simp add: ubdom_ubrep_eq idTSPF2_result_ubwell)
+   apply (simp add: cont2monofunE idTSPF2_result_ubwell ubgetch_ubrep_eq)
+  by (simp add: ubdom_below)
+
+
+lemma idTSPF2_cont: "cont (\<lambda> (x::('a MABP tstream\<^sup>\<Omega>)). (ubDom\<cdot>x = {c_abpOut}) \<leadsto> Abs_ubundle[c_idOut \<mapsto> x . c_abpOut])"
+  apply(rule contI2)
+   apply (simp add: idTSPF2_mono)
+proof (rule, rule)
+  fix Y::"nat \<Rightarrow> 'a MABP tstream\<^sup>\<Omega>"
+  assume a1: "chain Y"
+  have f1: "\<And> i. ubDom\<cdot>(\<Squnion>i::nat. Y i) = ubDom\<cdot>(Y i)"
+    by (simp add: a1)
+  have f2: "ubDom\<cdot>(Lub Y) = {c_abpOut} \<Longrightarrow> Some (\<Squnion>i::nat. (Abs_ubundle [c_idOut \<mapsto> Y i  .  c_abpOut])) = 
+    (\<Squnion>i::nat. Some (Abs_ubundle [c_idOut \<mapsto> Y i  .  c_abpOut]))"
+    apply (rule some_lub_chain_eq2)
+    apply (rule chainI)
+    apply (rule idTSPF2_result_below)
+     apply (simp add: a1 po_class.chainE)
+    by (simp add: a1)
+  have f30: "\<And>c.  ubDom\<cdot>(Lub Y) = {c_abpOut} \<Longrightarrow>  c \<in> ubDom\<cdot>(Abs_ubundle [c_idOut \<mapsto> Lub Y  .  c_abpOut])  
+        \<Longrightarrow> (\<Squnion>i::nat. Abs_ubundle [c_idOut \<mapsto> Y i  .  c_abpOut])  .  c = 
+              (\<Squnion>i::nat. Abs_ubundle [c_idOut \<mapsto> Y i  .  c_abpOut] .  c)"
+    apply (rule ubgetch_lub)
+    apply (rule chainI)
+     apply (rule idTSPF2_result_below)
+      apply (simp add: a1 po_class.chainE)
+     apply (simp add: a1)
+    by (metis (mono_tags, lifting) a1 idTSPF2_result_below idTSPF2_result_dom po_class.chainE po_class.chainI ubdom_chain_eq2)
+  have f31: "ubDom\<cdot>(Lub Y) = {c_abpOut} \<Longrightarrow> ubDom\<cdot>(Abs_ubundle [c_idOut \<mapsto> Lub Y  .  c_abpOut]) = {c_idOut}"
+    by (simp add: idTSPF2_result_dom)
+  have f3: " ubDom\<cdot>(Lub Y) = {c_abpOut} \<Longrightarrow> Some (Abs_ubundle [c_idOut \<mapsto> Lub Y  .  c_abpOut]) \<sqsubseteq> 
+         Some (\<Squnion>i::nat. (Abs_ubundle [c_idOut \<mapsto> Y i  .  c_abpOut]))"
+    apply (rule some_below)
+    apply (rule ub_below)
+     apply (metis (mono_tags, lifting) a1 idTSPF2_result_below idTSPF2_result_dom po_class.chainE po_class.chainI ubdom_chain_eq2)
+    apply (subst ubgetch_ubrep_eq)
+     apply (simp add: idTSPF2_result_ubwell)  
+    apply (simp only: f30)    
+    apply (subst ubgetch_ubrep_eq)
+     apply (simp add: a1 idTSPF2_result_ubwell)
+    apply (simp add: f31)
+    by (metis a1 below_refl contlub_cfun_arg)
+  show "(ubDom\<cdot>(\<Squnion>i::nat. Y i) = {c_abpOut})\<leadsto>Abs_ubundle [c_idOut \<mapsto> (\<Squnion>i::nat. Y i)  .  c_abpOut] 
+    \<sqsubseteq> (\<Squnion>i::nat. (ubDom\<cdot>(Y i) = {c_abpOut})\<leadsto>Abs_ubundle [c_idOut \<mapsto> Y i  .  c_abpOut])"
+    apply (case_tac "ubDom\<cdot>(\<Squnion>i::nat. Y i) \<noteq> {c_abpOut}")
+     apply (simp_all add: a1)
+    using f2 f3 by auto
+qed
+
+subsubsection\<open>ufWell/tickCount\<close>
+
+
+lemma idTSPF2_well: "ufWell (\<Lambda> (x::('a MABP tstream\<^sup>\<Omega>)). (ubDom\<cdot>x = {c_abpOut}) \<leadsto> Abs_ubundle[c_idOut \<mapsto> x . c_abpOut])"
+  apply(rule ufun_wellI)
+    apply(simp_all add: idTSPF2_cont ubclDom_ubundle_def domIff2)
+  apply (subst ubdom_ubrep_eq)
+  by (simp_all add: idTSPF2_result_ubwell domIff)
+
+lemma idTSPF2_tickCount: "ufIsWeak (Abs_cufun (\<lambda> (x::('a MABP tstream\<^sup>\<Omega>)). (ubDom\<cdot>x = {c_abpOut}) \<leadsto> Abs_ubundle[c_idOut \<mapsto> x . c_abpOut]))"
+  apply(simp add: ufIsWeak_def)
+  apply (rule, rule)
+  apply (simp add: idTSPF2_well idTSPF2_cont domIff2)
+  apply (simp add: ubclLen_ubundle_def)
+  by (simp add: idTSPF2_result_ubwell uslen_ubLen_ch1 uslen_ubLen_ch3)
+
+lemma idTSPF2_dom: "ufDom\<cdot>idTSPF2 = {c_abpOut}"
+  apply(simp add: idTSPF2_def)
+  apply (fold ubclDom_ubundle_def)
+  apply (subst ufun_ufdom_abs)
+  by (simp_all add: ubclDom_ubundle_def idTSPF2_cont idTSPF2_well)
+
+lemma idTSPF2_ran: "ufRan\<cdot>idTSPF2 = {c_idOut}"
+  apply (simp add: ufran_least)
+  apply(simp add: idTSPF2_dom)
+  apply(simp add: ubclDom_ubundle_def idTSPF2_def)
+  apply (simp add: rep_abs_cufun idTSPF2_cont idTSPF2_well)
+  apply (rule, rule)
+   apply (simp add: idTSPF2_result_dom)
+  by (simp add: ubclLeast_ubundle_def)
+
+
+(* ----------------------------------------------------------------------- *)
+section \<open>Components\<close>
+(* ----------------------------------------------------------------------- *)
+
+
+lemma h1: "inv Rev (Rev S) = S"
+  by (meson injI inv_f_eq rev.inject)
+
+lift_definition SND :: "(('a MABP tstream\<^sup>\<Omega>) ufun) uspec" is
+"Rev {senderTSPF s | s. s \<in> tsSender}"
+  apply(subst h1)
+  apply(simp add: uspecWell_def)
+  apply(simp add: ufclDom_ufun_def ufclRan_ufun_def)
+  using sender_tspfdom sender_tspfran
+  by metis
+
+lift_definition RCV :: "(('a MABP tstream\<^sup>\<Omega>) ufun) uspec" is
+"Rev {recvTSPF}"
+  apply(subst h1)
+  by(simp add: uspecWell_def)
+
+lift_definition MEDSR :: "('a MABP tstream\<^sup>\<Omega>) ufun uspec" is "Rev {medSR_TSPF ora | ora. #({True} \<ominus> ora)=\<infinity>}"
+  apply (simp add: inv_def)
+  apply (simp add: uspecWell_def)
+  apply (subst ufclDom_ufun_def)
+  apply (subst  ufclRan_ufun_def)
+  using med_tsps_dom2 med_tsps_ran2 by (metis ctype_MABP.simps(4))
+
+lift_definition MEDRS :: "('a MABP tstream\<^sup>\<Omega>) ufun uspec" is "Rev {medRS_TSPF ora | ora. #({True} \<ominus> ora)=\<infinity>}"
+  apply (simp add: inv_def)
+  apply (simp add: uspecWell_def)
+  apply (subst ufclDom_ufun_def)
+  apply (subst  ufclRan_ufun_def)
+  using med_tsps_dom2 med_tsps_ran2 by (metis ctype_MABP.simps(5))
+
+lift_definition ID :: "(('a MABP tstream\<^sup>\<Omega>) ufun) uspec" is
+"Rev {idTSPF2}"
+  apply(subst h1)
+  by(simp add: uspecWell_def)
+
+
+abbreviation gencompABP :: "(('a MABP tstream\<^sup>\<Omega>) ufun) uspec" where
+"gencompABP \<equiv> ((SND \<Otimes> MEDSR) \<Otimes> RCV) \<Otimes> MEDRS"
+
+abbreviation speccompABP :: "(('a MABP tstream\<^sup>\<Omega>) ufun) uspec" where
+"speccompABP \<equiv> uspecFeedbackComp(((SND \<circle> MEDSR) \<circle> RCV) \<circle> (MEDRS \<parallel> ID))"
+
+
+(* ----------------------------------------------------------------------- *)
+section \<open>Composition with special operators\<close>
+(* ----------------------------------------------------------------------- *)
+
+
+abbreviation innerABP where
+"innerABP s ora1 ora2 \<equiv> (ufSerComp (ufSerComp (ufSerComp (senderTSPF s) (medRS_TSPF ora1)) recvTSPF) (ufParComp (medRS_TSPF ora2) idTSPF))"
+
+abbreviation fixABPHelper where
+"fixABPHelper se ora1 ora2 tb \<equiv> (\<lambda> x. Abs_ubundle[
+    c_ds     \<mapsto> tsMap BoolPair\<cdot>(se\<cdot>(tsMap invData\<cdot>(tb . c_abpIn))\<cdot>(tsMap invBool\<cdot>(x . c_as))),
+    c_dr     \<mapsto> tsMap BoolPair\<cdot>(tsMed\<cdot>(tsMap invBoolPair\<cdot>(x . c_ds))\<cdot>ora1),
+    c_ar     \<mapsto> tsMap Bool\<cdot>(fst ( tsRec\<cdot>((tsMap invBoolPair)\<cdot>(x . c_dr)))),
+    c_abpOut \<mapsto> tsMap Data\<cdot>(snd ( tsRec\<cdot>((tsMap invBoolPair)\<cdot>(x . c_dr)))),
+    c_as     \<mapsto> tsMap Bool\<cdot>(tsMed\<cdot>(tsMap invBool\<cdot>(x . c_ar))\<cdot>ora2)
+    ])"
+
+abbreviation fixABPHelperCont where
+"fixABPHelperCont se ora1 ora2 tb \<equiv> (\<Lambda> x. Abs_ubundle[
+    c_ds     \<mapsto> tsMap BoolPair\<cdot>(se\<cdot>(tsMap invData\<cdot>(tb . c_abpIn))\<cdot>(tsMap invBool\<cdot>(x . c_as))),
+    c_dr     \<mapsto> tsMap BoolPair\<cdot>(tsMed\<cdot>(tsMap invBoolPair\<cdot>(x . c_ds))\<cdot>ora1),
+    c_ar     \<mapsto> tsMap Bool\<cdot>(fst ( tsRec\<cdot>((tsMap invBoolPair)\<cdot>(x . c_dr)))),
+    c_abpOut \<mapsto> tsMap Data\<cdot>(snd ( tsRec\<cdot>((tsMap invBoolPair)\<cdot>(x . c_dr)))),
+    c_as     \<mapsto> tsMap Bool\<cdot>(tsMed\<cdot>(tsMap invBool\<cdot>(x . c_ar))\<cdot>ora2)
+    ])"
+
+abbreviation abpFix where
+"abpFix s ora1 ora2 tb \<equiv> ubFix (fixABPHelperCont s ora1 ora2 tb) {c_abpOut, c_ar, c_as, c_dr, c_ds}"
+
+lemma abpHelper_ubWell: "\<And>x. ubWell [
+      c_ds     \<mapsto> tsMap BoolPair\<cdot>(s\<cdot>(tsMap invData\<cdot>(tb . c_abpIn))\<cdot>(tsMap invBool\<cdot>(x . c_as))),
+      c_dr     \<mapsto> tsMap BoolPair\<cdot>(tsMed\<cdot>(tsMap invBoolPair\<cdot>(x . c_ds))\<cdot>ora1),
+      c_ar     \<mapsto> tsMap Bool\<cdot>(fst ( tsRec\<cdot>((tsMap invBoolPair)\<cdot>(x . c_dr)))),
+      c_abpOut \<mapsto> tsMap Data\<cdot>(snd ( tsRec\<cdot>((tsMap invBoolPair)\<cdot>(x . c_dr)))),
+      c_as     \<mapsto> tsMap Bool\<cdot>(tsMed\<cdot>(tsMap invBool\<cdot>(x . c_ar))\<cdot>ora2)
+      ]"
+  apply(simp add: ubWell_def)
+  apply(simp add: usclOkay_tstream_def)
+  by (simp_all add: tsmap_tsdom_range)
+
+lemma abpHelper_cont: assumes "#({True} \<ominus> ora1) = \<infinity>"
+  and "#({True} \<ominus> ora2) = \<infinity>"
+  and "se \<in> tsSender"
+  and "ubDom\<cdot>tb = {c_abpIn}"
+shows "cont (fixABPHelper se ora1 ora2 tb)"
+  sorry
+
+
+(* Lemma from Dennis group  *)
+lemma tsaltbitpro_inp2out:
+  assumes send_def: "send \<in> tsSender"
+    and p1_def: "#({True} \<ominus> p1) = \<infinity>"
+    and p2_def: "#({True} \<ominus> p2) = \<infinity>"
+    and ds_def: "ds = send\<cdot>i\<cdot>as"
+    and dr_def: "dr = tsMed\<cdot>ds\<cdot>p1"
+    and ar_def: "ar = tsProjSnd\<cdot>dr"
+    and as_def: "as = tsMed\<cdot>ar\<cdot>p2"
+  shows "tsAbs\<cdot>(tsProjFst\<cdot>(tsRemDups\<cdot>dr)) = tsAbs\<cdot>i"
+  sorry
+
+
+(*=================DDD=========================================*)
 (* ----------------------------------------------------------------------- *)
 section \<open>Component Definitions\<close>
 (* ----------------------------------------------------------------------- *)
@@ -1724,5 +1723,688 @@ proof -
     apply (fold f206)
     by (simp add: f1_def f2_f3_def f4_f5_def f6_f7_def f8_f9_def ufunclFeedbackComp_ufun_def ufunclParComp_ufun_def ufunclSerComp_ufun_def)
 qed
+
+(*=========================================================================================================================================================*)
+
+
+lemma abp_speccomp_final: assumes "f \<in> Rep_rev_uspec speccompABP"
+                            and "ubDom\<cdot>tb = {c_abpIn}"
+  shows "tsAbs\<cdot>((f \<rightleftharpoons> tb) . c_abpOut) = tsAbs\<cdot>(tb . c_abpIn)"
+proof - 
+  have f1: "\<exists> s \<in> tsSender. \<exists>ora1 ora2. (#({True} \<ominus> ora1) = \<infinity>) \<and> (#({True} \<ominus> ora2) = \<infinity>) \<and>
+     (f =  (\<mu>(ufSerComp (ufSerComp (ufSerComp (senderTSPF s) (medRS_TSPF ora1)) recvTSPF) (ufParComp (medRS_TSPF ora2) idTSPF))))"
+    sorry
+  then obtain s where f12: "(s \<in> tsSender) \<and> (\<exists> ora1 ora2. (#({True} \<ominus> ora1) = \<infinity>) \<and> (#({True} \<ominus> ora2) = \<infinity>) \<and>
+     (f =  (\<mu>(ufSerComp (ufSerComp (ufSerComp (senderTSPF s) (medRS_TSPF ora1)) recvTSPF) (ufParComp (medRS_TSPF ora2) idTSPF)))))"
+    using f1 by blast
+  then obtain ora1  where f13: "(#({True} \<ominus> ora1) = \<infinity>) \<and> (\<exists> ora2. (#({True} \<ominus> ora2) = \<infinity>) \<and>
+     (f =  (\<mu>(ufSerComp (ufSerComp (ufSerComp (senderTSPF s) (medRS_TSPF ora1)) recvTSPF) (ufParComp (medRS_TSPF ora2) idTSPF)))))"
+    using f1 by blast
+  then obtain ora2  where f14: "(#({True} \<ominus> ora2) = \<infinity>) \<and>
+     (f =  (\<mu>(ufSerComp (ufSerComp (ufSerComp (senderTSPF s) (medRS_TSPF ora1)) recvTSPF) (ufParComp (medRS_TSPF ora2) idTSPF))))"
+    using f1 by blast
+  then have f15: "(f =  (\<mu>(ufSerComp (ufSerComp (ufSerComp (senderTSPF s) (medRS_TSPF ora1)) recvTSPF) (ufParComp (medRS_TSPF ora2) idTSPF))))"
+    using f1 by blast
+
+
+  have f20: "ufDom\<cdot>(innerABP s ora1 ora2) = {c_abpIn, c_ar}"
+    sorry
+  have f21: "ufRan\<cdot>(innerABP s ora1 ora2) = {c_abpOut, c_ar}"
+    sorry
+
+  have f2: "(f \<rightleftharpoons> tb) . c_abpOut =  (ubFix (ufFeedH (innerABP s ora1 ora2) tb) {c_abpOut, c_ar})  .  c_abpOut"
+    apply(subst f15)
+    apply(simp add: ufFeedbackComp_def)
+    apply(simp add: ufFeedbackComp_cont ufFeedbackComp_well)
+    apply(simp add: f20 f21 assms ubclDom_ubundle_def)
+    by auto
+ 
+  have f3: "(ubFix (ufFeedH (innerABP s ora1 ora2) tb) {c_abpOut, c_ar})  .  c_abpOut = 
+            (ubFix (fixABPHelperCont s ora1 ora2 tb) {c_abpOut, c_ar, c_as, c_dr, c_ds})  .  c_abpOut"
+    sorry
+
+  have f40: "ubfun_io_eq (fixABPHelperCont s ora1 ora2 tb) {c_abpOut, c_ar, c_as, c_dr, c_ds}"
+    sorry
+  then have f41: "ubFix (fixABPHelperCont s ora1 ora2 tb) {c_abpOut, c_ar, c_as, c_dr, c_ds} =  (fixABPHelperCont s ora1 ora2 tb)\<cdot>(ubFix (fixABPHelperCont s ora1 ora2 tb) {c_abpOut, c_ar, c_as, c_dr, c_ds})"
+    using ubfix_eq by blast
+
+  have f42: "\<And>x. ubWell [
+      c_ds     \<mapsto> tsMap BoolPair\<cdot>(s\<cdot>(tsMap invData\<cdot>(tb . c_abpIn))\<cdot>(tsMap invBool\<cdot>(x . c_as))),
+      c_dr     \<mapsto> tsMap BoolPair\<cdot>(tsMed\<cdot>(tsMap invBoolPair\<cdot>(x . c_ds))\<cdot>ora1),
+      c_ar     \<mapsto> tsMap Bool\<cdot>(fst ( tsRec\<cdot>((tsMap invBoolPair)\<cdot>(x . c_dr)))),
+      c_abpOut \<mapsto> tsMap Data\<cdot>(snd ( tsRec\<cdot>((tsMap invBoolPair)\<cdot>(x . c_dr)))),
+      c_as     \<mapsto> tsMap Bool\<cdot>(tsMed\<cdot>(tsMap invBool\<cdot>(x . c_ar))\<cdot>ora2)
+      ]"
+    using abpHelper_ubWell by blast
+  (* After proving the fixed points propties we can now show the assumptions of the tsaltbitpro_inp2out lemma
+  
+    i = (tsMap invData\<cdot>(tb . c_abpIn))
+    ds_stream = (tsMap invBoolPair\<cdot>((ubFix (abpFixH s tb) {c_abpOut, c_ar, c_dr}) . c_dr))
+    as_stream = (tsMap invBool\<cdot>((ubFix (abpFixH s tb) {c_abpOut, c_ar, c_dr}) . c_ar))
+
+  *)
+
+  (* Result *)
+  have f8: "tsAbs\<cdot>(tsProjFst\<cdot>(tsRemDups\<cdot>(tsMap invBoolPair\<cdot>((abpFix s ora1 ora2 tb) . c_dr)))) = tsAbs\<cdot>(tsMap invData\<cdot>(tb . c_abpIn))"
+    
+    sorry
+  have f9: "tsAbs\<cdot>(tsMap Data\<cdot>(tsProjFst\<cdot>(tsRemDups\<cdot>(tsMap invBoolPair\<cdot>((abpFix s ora1 ora2 tb) . c_dr))))) = tsAbs\<cdot>(tb . c_abpIn)"
+  proof - 
+    have f90: "\<And>s. invData (Data s) = s"
+      by simp
+    have f91: "tsDom\<cdot>(tb . c_abpIn) \<subseteq> range Data"
+      by (metis assms(2) ctype_MABP.simps(1) insert_iff ubdom_channel_usokay ubgetch_insert usclOkay_tstream_def)
+    then have f92: "\<exists>s. tb . c_abpIn = tsMap Data\<cdot>s"
+      sorry
+    show ?thesis
+      using f8 
+      sorry
+  qed
+  show ?thesis
+  proof - 
+    have f90: "cont ( fixABPHelper s ora1 ora2 tb)"
+      apply(subst abpHelper_cont, simp_all add: assms)
+      by(simp_all add: f12 f13 f14)
+    have f91: "(abpFix s ora1 ora2 tb) . c_abpOut =
+                tsMap Data\<cdot>(snd ( tsRec\<cdot>((tsMap invBoolPair)\<cdot>(abpFix s ora1 ora2 tb . c_dr))))"
+      apply(subst f41)
+      apply(simp add: f90)
+      apply(simp add: ubGetCh_def)
+      apply(subst ubrep_ubabs)
+      apply (metis (no_types, lifting) f42 ubgetch_insert)   
+       by simp   
+    have f92: "\<And>x. (snd (tsRec\<cdot>(tsMap invBoolPair\<cdot>x))) = (tsProjFst\<cdot>(tsRemDups\<cdot>(tsMap invBoolPair\<cdot>x)))"
+      by(simp add: tsRec_def tsRecSnd_def)
+    show ?thesis
+      apply(subst f2)
+      apply(subst f3)
+      apply(subst f91)
+      apply(subst f92)
+      apply(subst f9)
+      by simp
+  qed
+qed
+
+
+
+(*
+(* ----------------------------------------------------------------------- *)
+section \<open>Testing of Composition without Medium\<close>
+(* ----------------------------------------------------------------------- *)
+
+definition senderTSPF2 :: "'a sender \<Rightarrow> ('a MABP tstream\<^sup>\<Omega>) ufun" where
+"senderTSPF2 se \<equiv> Abs_cufun (\<lambda> x. (ubDom\<cdot>x = {c_ar, c_abpIn})
+                \<leadsto> Abs_ubundle [c_dr \<mapsto> tsMap BoolPair\<cdot>(se\<cdot>(tsMap invData\<cdot>(x . c_abpIn))\<cdot>(tsMap invBool\<cdot>(x . c_ar)))])"
+
+lemma sender_mono: assumes "se \<in> tsSender" shows "monofun (\<lambda> x. (ubDom\<cdot>x = {c_ar, c_abpIn})
+                \<leadsto> Abs_ubundle [c_dr \<mapsto> tsMap BoolPair\<cdot>(se\<cdot>(tsMap invData\<cdot>(x . c_abpIn))\<cdot>(tsMap invBool\<cdot>(x . c_ar)))])"
+  sorry
+
+lemma sender_cont: assumes "se \<in> tsSender" shows "cont (\<lambda> x. (ubDom\<cdot>x = {c_ar, c_abpIn})
+                \<leadsto> Abs_ubundle [c_dr \<mapsto> tsMap BoolPair\<cdot>(se\<cdot>(tsMap invData\<cdot>(x . c_abpIn))\<cdot>(tsMap invBool\<cdot>(x . c_ar)))])"
+  sorry
+
+lemma sender_well: assumes "se \<in> tsSender" shows "ufWell (\<Lambda> x. (ubDom\<cdot>x = {c_ar, c_abpIn})
+                \<leadsto> Abs_ubundle [c_dr \<mapsto> tsMap BoolPair\<cdot>(se\<cdot>(tsMap invData\<cdot>(x . c_abpIn))\<cdot>(tsMap invBool\<cdot>(x . c_ar)))])"
+  sorry
+
+lift_definition SND2 :: "(('a MABP tstream\<^sup>\<Omega>) ufun) uspec" is
+"Rev {senderTSPF2 s | s. s \<in> tsSender}"
+  sorry
+
+definition recvTSPF2 :: "('a MABP tstream\<^sup>\<Omega>) ufun" where
+"recvTSPF2 \<equiv> Abs_cufun (\<lambda> x. (ubDom\<cdot>x = {c_dr}) \<leadsto> Abs_ubundle [c_ar    \<mapsto> (tsMap::(bool \<Rightarrow> 'a MABP) \<Rightarrow> bool tstream \<rightarrow> 'a MABP tstream) Bool\<cdot>(fst ( tsRec\<cdot>((tsMap invBoolPair)\<cdot>(x . c_dr)))),
+                                        c_abpOut \<mapsto> (tsMap::('a \<Rightarrow> 'a MABP) \<Rightarrow> 'a tstream \<rightarrow> 'a MABP tstream) Data\<cdot>(snd ( tsRec\<cdot>((tsMap invBoolPair)\<cdot>(x . c_dr))))])"
+
+lemma recv_mono: "monofun (\<lambda> x. (ubDom\<cdot>x = {c_dr}) \<leadsto> Abs_ubundle [c_ar    \<mapsto> (tsMap::(bool \<Rightarrow> 'a MABP) \<Rightarrow> bool tstream \<rightarrow> 'a MABP tstream) Bool\<cdot>(fst ( tsRec\<cdot>((tsMap invBoolPair)\<cdot>(x . c_dr)))),
+                                        c_abpOut \<mapsto> (tsMap::('a \<Rightarrow> 'a MABP) \<Rightarrow> 'a tstream \<rightarrow> 'a MABP tstream) Data\<cdot>(snd ( tsRec\<cdot>((tsMap invBoolPair)\<cdot>(x . c_dr))))])"
+  sorry
+
+lemma recv_cont: "cont (\<lambda> x. (ubDom\<cdot>x = {c_dr}) \<leadsto> Abs_ubundle [c_ar    \<mapsto> (tsMap::(bool \<Rightarrow> 'a MABP) \<Rightarrow> bool tstream \<rightarrow> 'a MABP tstream) Bool\<cdot>(fst ( tsRec\<cdot>((tsMap invBoolPair)\<cdot>(x . c_dr)))),
+                                        c_abpOut \<mapsto> (tsMap::('a \<Rightarrow> 'a MABP) \<Rightarrow> 'a tstream \<rightarrow> 'a MABP tstream) Data\<cdot>(snd ( tsRec\<cdot>((tsMap invBoolPair)\<cdot>(x . c_dr))))])"
+  sorry
+
+lemma recv_well: "ufWell (\<Lambda> x. (ubDom\<cdot>x = {c_dr}) \<leadsto> Abs_ubundle [c_ar    \<mapsto> (tsMap::(bool \<Rightarrow> 'a MABP) \<Rightarrow> bool tstream \<rightarrow> 'a MABP tstream) Bool\<cdot>(fst ( tsRec\<cdot>((tsMap invBoolPair)\<cdot>(x . c_dr)))),
+                                        c_abpOut \<mapsto> (tsMap::('a \<Rightarrow> 'a MABP) \<Rightarrow> 'a tstream \<rightarrow> 'a MABP tstream) Data\<cdot>(snd ( tsRec\<cdot>((tsMap invBoolPair)\<cdot>(x . c_dr))))])"
+  sorry
+
+lift_definition RCV2 :: "(('a MABP tstream\<^sup>\<Omega>) ufun) uspec" is
+"Rev {recvTSPF2}"
+  sorry
+
+abbreviation speccompABP_nmed :: "(('a MABP tstream\<^sup>\<Omega>) ufun) uspec" where
+"speccompABP_nmed \<equiv> uspecFeedbackComp(SND \<circle> RCV)"
+
+
+lemma tsaltbitpro_inp2out_nmed:
+  assumes send_def: "send \<in> tsSender"
+    and ds_def: "ds_stream = send\<cdot>i\<cdot>as_stream"
+    and as_def: "as_stream = tsProjSnd\<cdot>ds_stream"
+    and i_inf: "#\<surd>i = \<infinity>"
+  shows "tsAbs\<cdot>(tsRecSnd\<cdot>ds_stream) = tsAbs\<cdot>i"
+  using as_def ds_def send_def tsaltbitpro_inp2out_nmed by auto
+
+lemma h1: assumes "s \<in> tsSender" shows "UFun.ufDom\<cdot>(ufunclSerComp (senderTSPF2 s) recvTSPF2) = {c_abpIn, c_ar}"
+  apply (simp add: ufdom_insert ubclDom_ubundle_def)
+  sorry                                                              
+
+lemma h2: assumes "s \<in> tsSender" shows "UFun.ufRan\<cdot>(ufunclSerComp (senderTSPF2 s) recvTSPF2) = {c_abpOut, c_ar}"
+  sorry
+
+abbreviation abpFixH :: "('a tstream \<rightarrow> bool tstream \<rightarrow> ('a \<times> bool) tstream) \<Rightarrow>  'a MABP tstream ubundle \<Rightarrow> 'a MABP tstream ubundle \<rightarrow> 'a MABP tstream ubundle" where
+"abpFixH s tb \<equiv> (\<Lambda> x. Abs_ubundle[c_dr \<mapsto> tsMap BoolPair\<cdot>(s\<cdot>(tsMap invData\<cdot>(tb . c_abpIn))\<cdot>(tsMap invBool\<cdot>(x . c_ar))),
+                                    c_ar \<mapsto> (tsMap::(bool \<Rightarrow> 'a MABP) \<Rightarrow> bool tstream \<rightarrow> 'a MABP tstream) Bool\<cdot>(fst ( tsRec\<cdot>((tsMap invBoolPair)\<cdot>(x . c_dr)))),
+                                    c_abpOut \<mapsto> (tsMap::('a \<Rightarrow> 'a MABP) \<Rightarrow> 'a tstream \<rightarrow> 'a MABP tstream) Data\<cdot>(snd ( tsRec\<cdot>((tsMap invBoolPair)\<cdot>(x . c_dr))))
+                                   ])"
+
+lemma abp_speccomp: assumes "f \<in> Rep_rev_uspec speccompABP_nmed"
+                            and "ubDom\<cdot>tb = {c_abpIn}"
+                          shows "tsAbs\<cdot>((f \<rightleftharpoons> tb) . c_abpOut) = tsAbs\<cdot>(tb . c_abpIn)"
+proof - 
+  have f1: "\<exists> s \<in> tsSender. (f = (\<mu>(ufunclSerComp (senderTSPF2 s) recvTSPF2)))"
+    apply (simp add: ufunclSerComp_ufun_def)
+    (* Cannot be proven until Instatiation *)
+    sorry
+  then obtain s where f12: "s \<in> tsSender \<and> (f = (\<mu>(ufunclSerComp (senderTSPF2 s) recvTSPF2)))"
+    by blast
+  then have f13: "f = (\<mu>(ufunclSerComp (senderTSPF2 s) recvTSPF2))"
+    by blast
+  have f14: "s \<in> tsSender"
+    using f12 by blast
+
+
+  have f20: "ubclDom\<cdot>tb = {c_abpIn, c_ar} - {c_ar}"
+    apply(simp add: ubclDom_ubundle_def)
+    using assms by blast                    
+  have f2: "(f \<rightleftharpoons> tb) . c_abpOut =  ubFix (ufFeedH (ufunclSerComp (senderTSPF2 s) recvTSPF2) tb) {c_abpOut, c_ar}  .  c_abpOut"
+    apply(subst f13)
+    apply(simp add: ufFeedbackComp_def)
+    apply(simp add: ufFeedbackComp_cont ufFeedbackComp_well)
+    apply(simp add: f12 h1 h2)
+    by(simp add: f20)
+
+
+  have f3: "cont (\<lambda> x. Abs_ubundle[c_dr \<mapsto> tsMap BoolPair\<cdot>(s\<cdot>(tsMap invData\<cdot>(tb . c_abpIn))\<cdot>(tsMap invBool\<cdot>(x . c_ar))),
+                                    c_ar \<mapsto> (tsMap::(bool \<Rightarrow> 'a MABP) \<Rightarrow> bool tstream \<rightarrow> 'a MABP tstream) Bool\<cdot>(fst ( tsRec\<cdot>((tsMap invBoolPair)\<cdot>(x . c_dr)))),
+                                    c_abpOut \<mapsto> (tsMap::('a \<Rightarrow> 'a MABP) \<Rightarrow> 'a tstream \<rightarrow> 'a MABP tstream) Data\<cdot>(snd ( tsRec\<cdot>((tsMap invBoolPair)\<cdot>(x . c_dr))))
+                                   ])"
+    sorry
+  have f4: "ubFix (ufFeedH (ufunclSerComp (senderTSPF2 s) recvTSPF2) tb) {c_abpOut, c_ar}  .  c_abpOut
+          = ubFix (abpFixH s tb) {c_abpOut, c_ar, c_dr} . c_abpOut"
+    (* Should be possible to prove with equality of lubs *)
+    sorry
+  have f5: "ubfun_io_eq (abpFixH s tb) {c_abpOut, c_ar, c_dr}"
+    sorry
+  then have f6: "ubFix (abpFixH s tb) {c_abpOut, c_ar, c_dr} =  (abpFixH s tb)\<cdot>(ubFix (abpFixH s tb) {c_abpOut, c_ar, c_dr})"
+    using ubfix_eq by blast
+
+
+  (* After proving the fixed points propties we can now show the assumptions of the tsaltbitpro_inp2out_nmed lemma *)
+  (*
+    i = (tsMap invData\<cdot>(tb . c_abpIn))
+    ds_stream = (tsMap invBoolPair\<cdot>((ubFix (abpFixH s tb) {c_abpOut, c_ar, c_dr}) . c_dr))
+    as_stream = (tsMap invBool\<cdot>((ubFix (abpFixH s tb) {c_abpOut, c_ar, c_dr}) . c_ar))
+
+  *)
+  have f7: "(tsMap invBoolPair\<cdot>((ubFix (abpFixH s tb) {c_abpOut, c_ar, c_dr}) . c_dr)) = s\<cdot>(tsMap invData\<cdot>(tb . c_abpIn))\<cdot>(tsMap invBool\<cdot>((ubFix (abpFixH s tb) {c_abpOut, c_ar, c_dr}) . c_ar))"
+    sorry
+
+  have f8: "(tsMap invBool\<cdot>((ubFix (abpFixH s tb) {c_abpOut, c_ar, c_dr}) . c_ar)) = tsProjSnd\<cdot>(tsMap invBoolPair\<cdot>((ubFix (abpFixH s tb) {c_abpOut, c_ar, c_dr}) . c_dr))"
+    sorry
+
+  (* More assms are necessary for this subgoal*)
+  have f9: "#\<surd>(tsMap invData\<cdot>(tb . c_abpIn)) = \<infinity>"
+    sorry
+
+  (* Result of tsaltbitpro_inp2out_nmed lemma *)
+  have f10: "tsAbs\<cdot>(tsRecSnd\<cdot>(tsMap invBoolPair\<cdot>((ubFix (abpFixH s tb) {c_abpOut, c_ar, c_dr}) . c_dr))) = tsAbs\<cdot>(tsMap invData\<cdot>(tb . c_abpIn))"
+    using f7 f8 f9 f14 by(simp add: tsaltbitpro_inp2out_nmed)
+  
+  
+
+  
+  show ?thesis
+      sorry  
+qed
+
+
+
+
+*)
+(*
+(* ----------------------------------------------------------------------- *)
+section \<open>More Lemmas\<close>
+(* ----------------------------------------------------------------------- *)
+*)
+(*
+lemma tsaltbitpro_inp2out_nmed:
+  assumes send_def: "send \<in> tsSender"
+    and ds_def: "c_ds = send\<cdot>i\<cdot>c_as"
+    and as_def: "c_as = tsProjSnd\<cdot>c_ds"
+    and i_inf: "#\<surd>i = \<infinity>"
+  shows "tsAbs\<cdot>(tsRecSnd\<cdot>c_ds) = tsAbs\<cdot>i"
+  sorry    
+
+lemma tsaltbitpro_inp2out:
+  assumes send_def: "send \<in> tsSender"
+    and p1_def: "#({True} \<ominus> p1) = \<infinity>"
+    and p2_def: "#({True} \<ominus> p2) = \<infinity>"
+    and ds_def: "c_ds = send\<cdot>i\<cdot>c_as"
+    and dr_def: "c_dr = tsMed\<cdot>c_ds\<cdot>p1"
+    and ar_def: "c_ar = tsProjSnd\<cdot>c_dr"
+    (* definition 5 *)
+    and as_def: "c_as = tsMed\<cdot>c_ar\<cdot>p2"
+    and i_ninf: "#(tsAbs\<cdot>i) \<noteq> \<infinity>"
+  shows "tsAbs\<cdot>(tsProjFst\<cdot>(tsRemDups\<cdot>c_dr)) = tsAbs\<cdot>i"
+  sorry
+
+
+
+lemma abp_gencomp_final: assumes "f \<in> Rep_rev_uspec gencompABP"
+                            and "ubDom\<cdot>tb = {c_abpIn}"
+  shows "tsAbs\<cdot>((f \<rightleftharpoons> tb) . c_abpOut) = tsAbs\<cdot>(tb . c_abpIn)"
+  oops  
+
+*)
+
+(*
+  subsection \<open>medium_rs\<close>
+
+(*
+
+definition tsMedRSTSPF :: "bool stream \<Rightarrow> 'a MABP TSPF" where
+"tsMedRSTSPF bst\<equiv> Abs_CTSPF (\<lambda> x. (tsbDom\<cdot>x = {c_ar})
+                           \<leadsto> [c_as \<mapsto> (tsMap::(bool \<Rightarrow> 'a MABP) \<Rightarrow> bool tstream \<rightarrow> 'a MABP tstream) Bool\<cdot>(tsMed\<cdot>(tsMap invBool\<cdot>(x . c_ar))\<cdot>bst)]\<Omega>)"
+
+abbreviation tsMedRSAbb  :: "bool stream \<Rightarrow> 'a MABP TSB \<Rightarrow> 'a MABP TSB option" where
+"tsMedRSAbb bst x \<equiv> ((tsbDom\<cdot>x = {c_ar})
+                           \<leadsto> [c_as \<mapsto> (tsMap::(bool \<Rightarrow> 'a MABP) \<Rightarrow> bool tstream \<rightarrow> 'a MABP tstream) Bool\<cdot>(tsMed\<cdot>(tsMap invBool\<cdot>(x . c_ar))\<cdot>bst)]\<Omega>)"
+
+*)
+subsubsection \<open>defs\<close>
+
+definition medRSH :: "bool stream \<Rightarrow> 'a MABP tstream\<^sup>\<Omega> \<Rightarrow> 'a MABP tstream"  where
+"medRSH bst \<equiv> (\<lambda> x. (tsMap::(bool \<Rightarrow> 'a MABP) \<Rightarrow> bool tstream \<rightarrow> 'a MABP tstream) Bool\<cdot>(tsMed\<cdot>(tsMap invBool\<cdot>(x  .  c_ar))\<cdot>bst))"
+
+lemma medrsh_cont [simp]: "cont (medRSH bst)"
+  by (simp add: medRSH_def)
+
+lemma medrsh_contlub: assumes "chain Y"
+  shows "(medRSH bst) ((\<Squnion>i. Y i)) = (\<Squnion>i. ((medRSH bst) ((Y i))))"
+  apply (rule cont2contlubE)
+  by (simp_all add: assms)
+
+lemma to_medrsh: "tsMap Bool\<cdot>(tsMed\<cdot>(tsMap invBool\<cdot>(x  .  c_ar))\<cdot>bst)
+                  = ((medRSH :: bool stream \<Rightarrow> 'a MABP tstream\<^sup>\<Omega> \<Rightarrow> 'a MABP tstream) bst) x"
+  by (simp add: medRSH_def)
+
+subsubsection \<open>pre\<close>
+
+lemma tsmed_input_cont [simp]: "cont (\<lambda> x. tsMed\<cdot>x\<cdot>bst)"
+  by simp
+
+lemma tsmed_input_mono [simp]: "monofun (\<lambda> x. tsMed\<cdot>x\<cdot>bst)"
+  using cont2mono tsmed_input_cont by blast
+
+
+lemma medrs_tsb_well [simp]: "ubWell  [c_as \<mapsto> tsMap Bool\<cdot>(tsMed\<cdot>(tsMap invBool\<cdot>(x . c_ar))\<cdot>bst)]"
+  apply (rule ubwellI)
+  apply (simp add: usclOkay_tstream_def)
+  by (simp add: tsmap_tsdom_range)
+
+lemma medrs_tsb_dom: "ubclDom\<cdot>(Abs_ubundle([c_as \<mapsto> tsMap Bool\<cdot>(tsMed\<cdot>(tsMap invBool\<cdot>(x . c_ar))\<cdot>bst)])) = {c_as}"
+  apply (simp add: ubclDom_ubundle_def)
+  by (simp add: ubdom_ubrep_eq)
+
+
+subsubsection \<open>cont\<close>
+
+  (* prerequirement for the mono proofs of the tspf *)
+lemma medrs_tsb_mono: "\<And>(x::'a MABP tstream\<^sup>\<Omega>) y::'a MABP tstream\<^sup>\<Omega>.
+       ubclDom\<cdot>x = {c_ar} \<Longrightarrow> x \<sqsubseteq> y \<Longrightarrow> Abs_ubundle([c_as \<mapsto> (tsMap::(bool \<Rightarrow> 'a MABP) \<Rightarrow> bool tstream \<rightarrow> 'a MABP tstream) Bool\<cdot>(tsMed\<cdot>(tsMap invBool\<cdot>(x  .  c_ar))\<cdot>bst)]) \<sqsubseteq> Abs_ubundle([c_as \<mapsto> tsMap Bool\<cdot>(tsMed\<cdot>(tsMap invBool\<cdot>(y  .  c_ar))\<cdot>bst)])"
+  apply (simp_all add: ubclDom_ubundle_def)
+  apply (rule ub_below)
+  apply (simp_all add: ubdom_below ubdom_ubrep_eq ubgetch_ubrep_eq)
+  apply (simp add: to_medrsh)
+  using cont2mono medrsh_cont monofun_def by blast
+
+
+lemma medrs_mono [simp]: "monofun (\<lambda> x::'a MABP tstream\<^sup>\<Omega>. (ubclDom\<cdot>x = {c_ar})
+                           \<leadsto> Abs_ubundle([c_as \<mapsto> (tsMap::(bool \<Rightarrow> 'a MABP) \<Rightarrow> bool tstream \<rightarrow> 'a MABP tstream)
+                                Bool\<cdot>(tsMed\<cdot>(tsMap invBool\<cdot>(x . c_ar))\<cdot>bst)]))"
+  apply (rule ufun_monoI2)
+  by (simp add: medrs_tsb_mono)
+
+lemma medrs_tsb_getc: assumes "chain (Y::nat \<Rightarrow> 'a MABP tstream\<^sup>\<Omega>)" and "ubclDom\<cdot>(\<Squnion>i::nat. Y i) = {c_ar}"
+                      and "c = c_as"
+  shows "(\<Squnion>i::nat. Abs_ubundle([c_as \<mapsto> (tsMap::(bool \<Rightarrow> 'a MABP) \<Rightarrow> bool tstream \<rightarrow> 'a MABP tstream) Bool\<cdot>(tsMed\<cdot>(tsMap invBool\<cdot>(Y i  .  c_ar))\<cdot>bst)]))  .  c_as
+          =  (\<Squnion>i::nat. (Abs_ubundle([c_as \<mapsto> (tsMap::(bool \<Rightarrow> 'a MABP) \<Rightarrow> bool tstream \<rightarrow> 'a MABP tstream) Bool\<cdot>(tsMed\<cdot>(tsMap invBool\<cdot>(Y i  .  c_ar))\<cdot>bst)])) . c_as)"
+proof (rule lubgetCh)
+  have f2: "\<And> i. ubclDom\<cdot>(Y i) =  ubclDom\<cdot>(\<Squnion>i. Y i)"
+    by (simp add: assms(1) ubclDom_ubundle_def)
+  show tb_chain: "chain (\<lambda>i::nat. Abs_ubundle([c_as \<mapsto> (tsMap::(bool \<Rightarrow> 'a MABP) \<Rightarrow> bool tstream \<rightarrow> 'a MABP tstream) Bool\<cdot>(tsMed\<cdot>(tsMap invBool\<cdot>(Y i  .  c_ar))\<cdot>bst)]))"
+    by (simp add: assms(1) assms(2) f2 medrs_tsb_mono po_class.chainE po_class.chainI)
+  show "c_as \<in> ubclDom\<cdot>(\<Squnion>i::nat. Abs_ubundle([c_as \<mapsto> (tsMap::(bool \<Rightarrow> 'a MABP) \<Rightarrow> bool tstream \<rightarrow> 'a MABP tstream) Bool\<cdot>(tsMed\<cdot>(tsMap invBool\<cdot>(Y i  .  c_ar))\<cdot>bst)]))"
+    by (metis (mono_tags, lifting) insert_iff medrs_tsb_dom tb_chain ubclDom_ubundle_def ubdom_chain_eq2)
+qed
+
+
+
+lemma medrs_cont [simp]: "cont (\<lambda> x::'a MABP tstream\<^sup>\<Omega>. (ubclDom\<cdot>x = {c_ar})
+                           \<leadsto> Abs_ubundle([c_as \<mapsto> (tsMap::(bool \<Rightarrow> 'a MABP) \<Rightarrow> bool tstream \<rightarrow> 'a MABP tstream)
+                                Bool\<cdot>(tsMed\<cdot>(tsMap invBool\<cdot>(x . c_ar))\<cdot>bst)]))"
+proof (rule ufun_contI)
+  show medrs_mo : "\<And>(x::'a MABP tstream\<^sup>\<Omega>) y::'a MABP tstream\<^sup>\<Omega>.
+       ubclDom\<cdot>x = {c_ar} \<Longrightarrow> x \<sqsubseteq> y \<Longrightarrow> Abs_ubundle [c_as \<mapsto> tsMap Bool\<cdot>(tsMed\<cdot>(tsMap invBool\<cdot>(x  .  c_ar))\<cdot>bst)] 
+          \<sqsubseteq> Abs_ubundle [c_as \<mapsto> tsMap Bool\<cdot>(tsMed\<cdot>(tsMap invBool\<cdot>(y  .  c_ar))\<cdot>bst)]"
+    by (simp add: medrs_tsb_well monofun_cfun_arg monofun_cfun_fun option.distinct(1) option.sel ub_below ubdom_ubrep_eq ubgetch_ubrep_eq)
+
+  have f1: " \<And>Y::nat \<Rightarrow> 'a MABP tstream\<^sup>\<Omega>. chain Y \<Longrightarrow> ubclDom\<cdot>(\<Squnion>i::nat. Y i) = {c_ar} \<Longrightarrow>
+       ubclDom\<cdot>(\<Squnion>i::nat. Abs_ubundle([c_as \<mapsto> (tsMap::(bool \<Rightarrow> 'a MABP) \<Rightarrow> bool tstream \<rightarrow> 'a MABP tstream) Bool\<cdot>(tsMed\<cdot>(tsMap invBool\<cdot>(Y i  .  c_ar))\<cdot>bst)])) = {c_as}"
+    by (metis (mono_tags, lifting) medrs_tsb_dom medrs_tsb_mono po_class.chain_def ubcldom_lub_eq2I)
+  show "\<And>Y::nat \<Rightarrow> 'a MABP tstream\<^sup>\<Omega>. chain Y \<Longrightarrow> ubclDom\<cdot>(\<Squnion>i::nat. Y i) = {c_ar} \<Longrightarrow>
+       Abs_ubundle([c_as \<mapsto> (tsMap::(bool \<Rightarrow> 'a MABP) \<Rightarrow> bool tstream \<rightarrow> 'a MABP tstream) Bool\<cdot>(tsMed\<cdot>(tsMap invBool\<cdot>((\<Squnion>i::nat. Y i)  .  c_ar))\<cdot>bst)]) \<sqsubseteq> (\<Squnion>i::nat. Abs_ubundle([c_as \<mapsto> tsMap Bool\<cdot>(tsMed\<cdot>(tsMap invBool\<cdot>(Y i  .  c_ar))\<cdot>bst)]))"
+  proof -
+    fix Y::"nat \<Rightarrow> 'a MABP tstream\<^sup>\<Omega>"
+    assume chain_Y: "chain Y" and chain_Y_dom: "ubclDom\<cdot>(\<Squnion>i::nat. Y i) = {c_ar}"
+    have f10: "(\<Squnion>i::nat. Abs_ubundle [c_as \<mapsto> tsMap Bool\<cdot>(tsMed\<cdot>(tsMap invBool\<cdot>(Y i  .  c_ar))\<cdot>bst)])  .  c_as =
+                    (\<Squnion>i::nat. Abs_ubundle [c_as \<mapsto> tsMap Bool\<cdot>(tsMed\<cdot>(tsMap invBool\<cdot>(Y i  .  c_ar))\<cdot>bst)]  .  c_as)"
+      apply (rule cont2contlubE, simp)
+      apply (rule chainI)
+      by (simp add: chain_Y monofun_cfun_arg monofun_cfun_fun po_class.chainE ub_below ubdom_ubrep_eq ubgetch_ubrep_eq)
+    show "Abs_ubundle([c_as \<mapsto> (tsMap::(bool \<Rightarrow> 'a MABP) \<Rightarrow> bool tstream \<rightarrow> 'a MABP tstream) Bool\<cdot>(tsMed\<cdot>(tsMap invBool\<cdot>((\<Squnion>i::nat. Y i)  .  c_ar))\<cdot>bst)]) \<sqsubseteq> (\<Squnion>i::nat. Abs_ubundle([c_as \<mapsto> tsMap Bool\<cdot>(tsMed\<cdot>(tsMap invBool\<cdot>(Y i  .  c_ar))\<cdot>bst)]))"
+      apply (rule ub_below)
+       apply (simp_all add: ubdom_below ubdom_ubrep_eq ubgetch_ubrep_eq f1) 
+       apply (metis (mono_tags, lifting) chain_Y chain_Y_dom f1 ubclDom_ubundle_def)
+      apply (subst f10)
+      by (metis (mono_tags, lifting) chain_Y fun_upd_same lub_eq medrs_tsb_well medrsh_contlub not_below2not_eq option.sel to_medrsh ubgetch_ubrep_eq)
+  qed
+qed
+
+
+  subsubsection \<open>tspf_well\<close>
+  
+ (* show that the mediumRSTSPF template  fulfills the tickcount property *)
+lemma medrs_tick: assumes "ubclDom\<cdot>b = {c_ar}" and "(ubLen b) = n" and "#bst=\<infinity>"
+  shows "n \<le> (ubclLen (Abs_ubundle([c_as \<mapsto> (tsMap::(bool \<Rightarrow> 'a MABP) \<Rightarrow> bool tstream \<rightarrow> 'a MABP tstream) Bool\<cdot>(tsMed\<cdot>(tsMap invBool\<cdot>(b  .  c_ar))\<cdot>bst)])))"
+proof -
+  have "(ubLen b) = usclLen\<cdot>(b . c_ar)"
+    apply (rule uslen_ubLen_ch3)
+    by (metis assms(1) ubclDom_ubundle_def)
+  hence f1: "n = usclLen\<cdot>(b . c_ar)"
+    using assms(2) by blast
+  hence f2: "n \<le> usclLen\<cdot>((tsMap::(bool \<Rightarrow> 'a MABP) \<Rightarrow> bool tstream \<rightarrow> 'a MABP tstream) Bool\<cdot>(tsMed\<cdot>(tsMap invBool\<cdot>(b  .  c_ar))\<cdot>bst))"
+    by (simp add: assms(3) usclLen_tstream_def)
+  show ?thesis
+    apply (simp add: ubclLen_ubundle_def)
+    apply (rule ubLen_geI)
+    apply (simp add: medrs_tsb_dom ubgetch_ubrep_eq)
+    by (simp add: f2 ubdom_ubrep_eq)
+qed
+  
       
-end
+    
+  (* a medium is a tspf if the oracle bool stream bst is infinitly long*)
+lemma medrs_well [simp]: assumes "#bst=\<infinity>"
+  shows "ufWell (\<Lambda> (x::'a MABP tstream\<^sup>\<Omega>). (ubclDom\<cdot>x = {c_ar})
+                           \<leadsto> Abs_ubundle([c_as \<mapsto> (tsMap::(bool \<Rightarrow> 'a MABP) \<Rightarrow> bool tstream \<rightarrow> 'a MABP tstream)
+                                Bool\<cdot>(tsMed\<cdot>(tsMap invBool\<cdot>(x . c_ar))\<cdot>bst)]))"
+  apply (rule ufun_wellI)
+    apply (simp_all add: domIff2)
+  by (simp add:  ubclDom_ubundle_def ubDom_def)
+
+      
+lemma medrs_revsubst: "Abs_cufun (tsMedRSAbb bst) = (medRS_TSPF bst)"
+  by (simp add: medRS_TSPF_def)
+    
+lemma medrs_tspfdom: assumes "#bst =\<infinity>"
+  shows "ufDom\<cdot>(medRS_TSPF bst) = {c_ar}"
+    apply (simp add: medRS_TSPF_def)
+    apply (simp add: ufdom_insert assms)
+    apply (simp add: domIff2)
+  by (simp add: ubclDom_h)
+   
+lemma medrs_tspfran: assumes "#bst =\<infinity>"
+  shows "ufRan\<cdot>(medRS_TSPF bst) = {c_as}"   
+    apply (simp add: medRS_TSPF_def)
+    apply (simp add: ufran_least medrs_tspfdom assms)
+    apply (simp add: medrs_revsubst medrs_tspfdom assms)
+  by (simp add: medrs_tsb_dom ubcldom_least_cs)
+
+
+  (* now special lemmata for TSPS instantiation *)
+
+lemma medrs_well2 [simp]: assumes "#({True} \<ominus> bst) = \<infinity>"
+  shows "ufWell (\<Lambda> (x::'a MABP tstream\<^sup>\<Omega>). (ubclDom\<cdot>x = {c_ar})
+                           \<leadsto> Abs_ubundle([c_as \<mapsto> (tsMap::(bool \<Rightarrow> 'a MABP) \<Rightarrow> bool tstream \<rightarrow> 'a MABP tstream)
+                                Bool\<cdot>(tsMed\<cdot>(tsMap invBool\<cdot>(x . c_ar))\<cdot>bst)]))"
+proof -
+   have "#bst = \<infinity>"
+     by (simp add: med_ora_length assms(1))
+   thus ?thesis  
+     by (simp add: medrs_tspfdom)
+qed
+  
+
+lemma medrs_tspfdom2: assumes "#({True} \<ominus> bst) = \<infinity>"
+  shows "ufclDom\<cdot>(medRS_TSPF bst) = {c_ar}"
+proof -
+  have "#bst = \<infinity>"
+    by (simp add: med_ora_length assms(1))
+  thus ?thesis
+    by (simp add: medrs_tspfdom ufclDom_ufun_def)
+qed
+  
+lemma medrs_tspfran2: assumes "#({True} \<ominus> bst) = \<infinity>"
+  shows "ufRan\<cdot>(medRS_TSPF bst) = {c_as}"
+proof -
+  have "#bst = \<infinity>"
+    by (simp add: med_ora_length assms(1))
+  thus ?thesis
+    by (simp add: medrs_tspfran)
+qed
+
+  (* necessary for TSPS instantiation *)
+lemma medrs_tsps_dom1 [simp]: "f = medRS_TSPF ora \<and> #({True} \<ominus> ora) = \<infinity> \<Longrightarrow> ufDom\<cdot>f = {c_ar}"
+  by (metis medrs_tspfdom2 ufclDom_ufun_def)
+
+lemma medrs_tsps_dom2 [simp]: "\<exists>ora::bool stream. f = medRS_TSPF ora \<and> #({True} \<ominus> ora) = \<infinity> 
+                               \<Longrightarrow> ufDom\<cdot>f = {c_ar}"
+  using medrs_tsps_dom1  by auto
+ 
+lemma medrs_tsps_ran1 [simp]: "f = medRS_TSPF ora \<and> #({True} \<ominus> ora) = \<infinity> \<Longrightarrow> ufRan\<cdot>f = {c_as}"
+  by (simp add: medrs_tspfran2)
+
+lemma medrs_tsps_ran2 [simp]: "\<exists>ora::bool stream. f = medRS_TSPF ora \<and> #({True} \<ominus> ora) = \<infinity> 
+                               \<Longrightarrow> ufRan\<cdot>f = {c_as}"
+  using medrs_tsps_ran1 by auto
+
+
+      
+  subsection \<open>medium_sr\<close>     
+
+subsubsection \<open>defs\<close>
+
+definition medSRH :: "bool stream \<Rightarrow> 'a MABP TSB \<Rightarrow> 'a MABP tstream"  where
+"medSRH bst \<equiv> (\<lambda> x. (tsMap:: ('a \<times> bool \<Rightarrow> 'a MABP) \<Rightarrow> ('a \<times> bool) tstream \<rightarrow> 'a MABP tstream) 
+            BoolPair\<cdot>(tsMed\<cdot>(tsMap invBoolPair\<cdot>(x . c_ds))\<cdot>bst))"
+
+lemma medsrh_cont [simp]: "cont (medSRH bst)"
+  by (simp add: medSRH_def)
+
+lemma medsrh_contlub: assumes "chain Y"
+  shows "(medSRH bst) ((\<Squnion>i. Y i)) = (\<Squnion>i. ((medSRH bst) ((Y i))))"
+  apply (rule cont2contlubE)
+  by (simp_all add: assms)
+
+lemma to_medsrh: "tsMap BoolPair\<cdot>(tsMed\<cdot>(tsMap invBoolPair\<cdot>(x  .  c_ds))\<cdot>bst)
+                  = ((medSRH :: bool stream \<Rightarrow> 'a MABP TSB \<Rightarrow> 'a MABP tstream) bst) x"
+  by (simp add: medSRH_def)
+
+subsubsection \<open>pre\<close>
+(*
+lemma tsmed_input_cont [simp]: "cont (\<lambda> x. tsMed\<cdot>x\<cdot>bst)"
+  by simp
+
+lemma tsmed_input_mono [simp]: "monofun (\<lambda> x. tsMed\<cdot>x\<cdot>bst)"
+  using cont2mono tsmed_input_cont by blast
+*)
+
+lemma medsr_tsb_well[simp]: "tsb_well [c_dr \<mapsto> tsMap BoolPair\<cdot>(tsMed\<cdot>(tsMap invBoolPair\<cdot>(x . c_ds))\<cdot>bst)]"
+  apply (rule tsb_wellI)
+  by (simp add: tsmap_tsdom_range)
+
+lemma medsr_tsb_dom: "tsbDom\<cdot>([c_dr \<mapsto> tsMap BoolPair\<cdot>(tsMed\<cdot>(tsMap invBoolPair\<cdot>(x . c_ds))\<cdot>bst)]\<Omega>) = {c_dr}"
+  by (simp add: tsbdom_rep_eq)
+    
+  subsubsection \<open>cont\<close>
+    
+(* definition tsMedSRTSPF :: "bool stream \<Rightarrow> 'a MABP TSPF" where
+"tsMedSRTSPF bst\<equiv> Abs_CTSPF (\<lambda> x. (tsbDom\<cdot>x = {c_ds})
+  \<leadsto> [c_dr \<mapsto> (tsMap:: ('a \<times> bool \<Rightarrow> 'a MABP) \<Rightarrow> ('a \<times> bool) tstream \<rightarrow> 'a MABP tstream) 
+            BoolPair\<cdot>(tsMed\<cdot>(tsMap invBoolPair\<cdot>(x . c_ds))\<cdot>bst)]\<Omega>)" *)
+
+(* this can be shown analogue to before *)
+lemma medsr_cont [simp]: "cont (\<lambda> x::'a MABP TSB. (tsbDom\<cdot>x = {c_ds})
+  \<leadsto> [c_dr \<mapsto> (tsMap:: ('a \<times> bool \<Rightarrow> 'a MABP) \<Rightarrow> ('a \<times> bool) tstream \<rightarrow> 'a MABP tstream) 
+            BoolPair\<cdot>(tsMed\<cdot>(tsMap invBoolPair\<cdot>(x . c_ds))\<cdot>bst)]\<Omega>)"
+  sorry
+    
+ 
+  subsubsection \<open>tspf_well\<close>
+
+lemma medsr_tick: assumes "tsbDom\<cdot>b = {c_ds}" and "(#\<surd>tsb b) = n" and "#bst=\<infinity>"
+  shows "n \<le> (#\<surd>tsb [c_dr \<mapsto> (tsMap:: ('a \<times> bool \<Rightarrow> 'a MABP) \<Rightarrow> ('a \<times> bool) tstream \<rightarrow> 'a MABP tstream) 
+            BoolPair\<cdot>(tsMed\<cdot>(tsMap invBoolPair\<cdot>(b . c_ds))\<cdot>bst)]\<Omega>)"
+proof -
+  have "(#\<surd>tsb b) = #\<surd>(b . c_ds)"
+    apply (rule tsbtick_single_ch2)
+    by (simp add: assms(1))
+  hence f1: "n = #\<surd>(b . c_ds)"
+    using assms(2) by blast
+  hence f2: "n \<le> #\<surd>((tsMap:: ('a \<times> bool \<Rightarrow> 'a MABP) \<Rightarrow> ('a \<times> bool) tstream \<rightarrow> 'a MABP tstream) 
+            BoolPair\<cdot>(tsMed\<cdot>(tsMap invBoolPair\<cdot>(b . c_ds))\<cdot>bst))"
+    by (simp add: assms(3))
+  show ?thesis
+    apply (rule tsbtick_geI)
+    apply (simp add: medsr_tsb_dom tsbgetch_rep_eq)
+    using f2 by force
+qed    
+    
+  (* a medium is a tspf if the oracle bool stream bst is infinitly long*)
+lemma medsr_well [simp]: assumes "#bst=\<infinity>"
+  shows "tspf_well (\<Lambda> x.(tsbDom\<cdot>x = {c_ds})
+  \<leadsto> [c_dr \<mapsto> (tsMap:: ('a \<times> bool \<Rightarrow> 'a MABP) \<Rightarrow> ('a \<times> bool) tstream \<rightarrow> 'a MABP tstream) 
+            BoolPair\<cdot>(tsMed\<cdot>(tsMap invBoolPair\<cdot>(x . c_ds))\<cdot>bst)]\<Omega>)"
+  apply (rule tspf_wellI)
+    apply (simp_all add: domIff2 medsr_tsb_dom)
+    apply (subst tsbtick_single_ch1, simp)
+    by (simp add: assms tsbtick_single_ch2)    
+ 
+lemma medsr_revsubst: "Abs_CTSPF (medSR_TSPFAbb bst) = (medSR_TSPF bst)"
+  by (simp add: medSR_TSPF_def)
+    
+lemma medsr_tspfdom: assumes "#bst =\<infinity>"
+  shows "tspfDom\<cdot>(medSR_TSPF bst) = {c_ds}"
+    apply (simp add: medSR_TSPF_def)
+    apply (simp add: tspf_dom_insert assms)
+    apply (simp add: domIff2)
+    by (meson tsbleast_tsdom someI)
+   
+lemma medsr_tspfran: assumes "#bst =\<infinity>"
+  shows "tspfRan\<cdot>(medSR_TSPF bst) = {c_dr}"   
+    apply (simp add: medSR_TSPF_def)
+    apply (simp add: tspfran_least medsr_tspfdom assms)
+    apply (simp add: medsr_revsubst medsr_tspfdom assms)
+    by (metis singletonI tsb_newMap_id tsbleast_getch tsbleast_tsdom)
+
+  (* now special lemmata for TSPS instantiation *)
+
+lemma medsr_well2 [simp]: assumes "#({True} \<ominus> bst) = \<infinity>"
+  shows "tspf_well (\<Lambda> x.(tsbDom\<cdot>x = {c_ds})
+  \<leadsto> [c_dr \<mapsto> (tsMap:: ('a \<times> bool \<Rightarrow> 'a MABP) \<Rightarrow> ('a \<times> bool) tstream \<rightarrow> 'a MABP tstream) 
+            BoolPair\<cdot>(tsMed\<cdot>(tsMap invBoolPair\<cdot>(x . c_ds))\<cdot>bst)]\<Omega>)"
+proof -
+   have "#bst = \<infinity>"
+     by (simp add: med_ora_length assms(1))
+   thus ?thesis
+     by (simp add: medsr_tspfdom)
+qed
+  
+
+lemma medsr_tspfdom2: assumes "#({True} \<ominus> bst) = \<infinity>"
+  shows "tspfDom\<cdot>(medSR_TSPF bst) = {c_ds}"
+proof -
+  have "#bst = \<infinity>"
+    by (simp add: med_ora_length assms(1))
+  thus ?thesis
+    by (simp add: medsr_tspfdom)
+qed
+  
+lemma medsr_tspfran2: assumes "#({True} \<ominus> bst) = \<infinity>"
+  shows "tspfRan\<cdot>(medSR_TSPF bst) = {c_dr}"
+proof -
+  have "#bst = \<infinity>"
+    by (simp add: med_ora_length assms(1))
+  thus ?thesis
+    by (simp add: medsr_tspfran)
+qed
+
+  (* necessary for TSPS instantiation *)
+lemma medsr_tsps_dom1 [simp]: "f = medSR_TSPF ora \<and> #({True} \<ominus> ora) = \<infinity> \<Longrightarrow> tspfDom\<cdot>f = {c_ds}"
+  by (simp add: medsr_tspfdom2)
+
+lemma medsr_tsps_dom2 [simp]: "\<exists>ora::bool stream. f = medSR_TSPF ora \<and> #({True} \<ominus> ora) = \<infinity> 
+                               \<Longrightarrow> tspfDom\<cdot>f = {c_ds}"
+  using medsr_tsps_dom1  by auto
+ 
+lemma medsr_tsps_ran1 [simp]: "f = medSR_TSPF ora \<and> #({True} \<ominus> ora) = \<infinity> \<Longrightarrow> tspfRan\<cdot>f = {c_dr}"
+  by (simp add: medsr_tspfran2)
+
+lemma medsr_tsps_ran2 [simp]: "\<exists>ora::bool stream. f = medSR_TSPF ora \<and> #({True} \<ominus> ora) = \<infinity> 
+                               \<Longrightarrow> tspfRan\<cdot>f = {c_dr}"
+  using medsr_tsps_ran1 by auto
+      
+(* ----------------------------------------------------------------------- *)
+section \<open>Component Definitions\<close>
+(* ----------------------------------------------------------------------- *)
+  
+lift_definition RCV :: "('a MABP tstream\<^sup>\<Omega> , 'a MABP tstream\<^sup>\<Omega>) ufun uspec" is "Rev {recvTSPF}"
+  apply (simp add: inv_def)
+  by (simp add: uspecWell_def)
+    
+lift_definition MEDSR :: "'a MABP TSPS" is "{medSR_TSPF ora | ora. #({True} \<ominus> ora)=\<infinity>}"
+  apply (rule tsps_wellI)
+   by (simp_all)
+    
+lift_definition MEDRS :: "'a MABP TSPS" is "{medRS_TSPF ora | ora. #({True} \<ominus> ora)=\<infinity>}"
+  apply (rule tsps_wellI)
+   by (simp_all) (* proof uses the special medrs_tsps lemmata *)
+    
+lift_definition SND  :: "'a MABP TSPS" is "{senderTSPF s | s. s \<in> tsSender}"
+  apply (rule tsps_wellI)
+   apply (simp_all)
+    (* instantiation analogue to MEDRS *)
+    sorry
+
+abbreviation sendCompRecv :: "'a MABP TSPS" where 
+"sendCompRecv \<equiv> (SND::'a MABP TSPS) \<Otimes> (RCV::'a MABP TSPS)"
+  
+      
+abbreviation gencompABP :: "'a MABP TSPS" where
+"gencompABP \<equiv> ((SND \<Otimes> MEDSR) \<Otimes> RCV) \<Otimes> MEDRS"
+  
+  
+
+(* ----------------------------------------------------------------------- *)
+section \<open>More Lemmas\<close>
+(* ----------------------------------------------------------------------- *)
+  
+  (* Final lemma for general composition operator*)
+lemma abp_gencomp_final: assumes "f \<in> Rep_TSPS gencompABP"
+                            and "tsbDom\<cdot>tb = {c_abpIn}"
+  shows "tsAbs\<cdot>((f \<rightleftharpoons> tb) . c_abpOut) = tsAbs\<cdot>(tb . c_abpIn)"
+  oops                          
+      
+
+*)
